@prefix adms: <http://www.w3.org/ns/adms#> .  
@prefix rdf: <http://www.w3.org/1999/02/22-rdf-syntax-ns#> .  
@prefix epos: <https://www.epos-eu.org/epos-dcat-ap#> .  
@prefix dc: <http://purl.org/dc/elements/1.1/> .  
@prefix dct: <http://purl.org/dc/terms/> .  
@prefix vcard: <http://www.w3.org/2006/vcard/ns#> .  
@prefix hydra: <http://www.w3.org/ns/hydra/core#> .  
@prefix xsd: <http://www.w3.org/2001/XMLSchema#> .  
@prefix schema: <http://schema.org/> .  
@prefix dcat: <http://www.w3.org/ns/dcat#> .  
@prefix cnt: <http://www.w3.org/2011/content#> .  
@prefix locn: <http://www.w3.org/ns/locn#> .  
@prefix skos: <http://www.w3.org/2004/02/skos/core#> .  
@prefix rdfs: <http://www.w3.org/2000/01/rdf-schema#> .  
@prefix http: <http://www.w3.org/2006/http#> .  
@prefix owl: <http://www.w3.org/2002/07/owl#> .  
@prefix gsp: <http://www.opengis.net/ont/geosparql#> .  

<PIC:996625337> a schema:Organization;
	schema:identifier [ a schema:PropertyValue;
		schema:propertyID "pic";
		schema:value "996625337";
	]; 
	schema:legalName "Institute of Geophysics, Polish Academy of Sciences";
	schema:address [ a schema:PostalAddress;
		schema:streetAddress "Księcia Janusza 64";
		schema:addressLocality "Warszawa";
		schema:postalCode "01-452";
		schema:addressCountry "Poland";
	]; 
	schema:logo "http://igf.edu.pl/grafika/logo.png"^^xsd:anyURI;
	schema:url "http://igf.edu.pl/home.php"^^xsd:anyURI;
	schema:email "office@igf.edu.pl";
	schema:contactPoint <http://orcid.org/0000-0002-4801-4888/contactPoint>;
. 
<PIC:999844573> a schema:Organization;
	schema:identifier [ a schema:PropertyValue;
		schema:propertyID "pic";
		schema:value "999844573";
	]; 
	schema:legalName "Academic Computer Centre CYFRONET AGH";
	schema:address [ a schema:PostalAddress;
		schema:streetAddress "Nawojki 11";
		schema:addressLocality "Krakow";
		schema:postalCode "30-950";
		schema:addressCountry "Poland";
	]; 
	schema:logo "http://www.cyfronet.krakow.pl/en/for_press/13438,artykul,acc_cyfronet_agh_logo.html"^^xsd:anyURI;
	schema:url "http://www.cyfronet.krakow.pl/en/"^^xsd:anyURI;
	schema:email "cyfronet@cyfronet.krakow.pl";
	schema:contactPoint <mailto:m.sterzel@cyfronet.pl/contactPoint>;
. 
<PIC:999994341> a schema:Organization;
	schema:identifier [ a schema:PropertyValue;
		schema:propertyID "pic";
		schema:value "999994341";
	]; 
	schema:legalName "Helmholtz-Zentrum Potsdam, Deutsches GeoForschungsZentrum, GFZ";
	schema:address [ a schema:PostalAddress;
		schema:streetAddress "Telegrafenberg";
		schema:addressLocality "Potsdam";
		schema:postalCode "14473";
		schema:addressCountry "Germany";
	]; 
	#schema:logo "https://www.gfz-potsdam.de/fileadmin/_processed_/0/2/csm_LOGO-GFZ-de-mitFreistellungsraum_RGB_24bit_300dpi_546x390-jpg_06_f50928a495.jpg"^^xsd:anyURI;
	schema:url "http://www.gfz-potsdam.de/"^^xsd:anyURI;
	schema:email "info@gfz-potsdam.de";
	schema:contactPoint <http://orcid.org/0000-0003-1076-615X/contactPoint>;
	schema:contactPoint <mailto:a_blanke@gfz-potsdam.de/contactPoint>;
. 
<https://www.igp-vast.vn/> a schema:Organization;
	schema:identifier [ a schema:PropertyValue;
		schema:propertyID "URL";
		schema:value "https://www.igp-vast.vn/";
	]; 
	schema:legalName "Institute of Geophysics Vietnam Academy of Science and Technology";
	schema:address [ a schema:PostalAddress;
		schema:streetAddress "A8 Building - 18 Hoang Quoc Viet - Cau Giay";
		schema:addressLocality "Hanoi";
		schema:addressCountry "Vietnam";
	]; 
	schema:url "https://www.igp-vast.vn/"^^xsd:anyURI;
	schema:telephone "+84 24 37 564 380";
	schema:contactPoint <mailto:giangnv@igp-vast.vn/contactPoint>;
. 
<PIC:999516616> a schema:Organization;
	schema:identifier [ a schema:PropertyValue;
		schema:propertyID "pic";
		schema:value "999516616";
	]; 
	schema:legalName "Central Mining Institute";
	schema:address [ a schema:PostalAddress;
		schema:streetAddress "Plac Gwarków 1";
		schema:addressLocality "Katowice";
		schema:postalCode "40-166";
		schema:addressCountry "Poland";
	]; 
	schema:logo "https://www.gig.eu/sites/default/files/gig-logo.png"^^xsd:anyURI;
	schema:url "https://www.gig.eu"^^xsd:anyURI;
	schema:email "gmutke@gig.eu";
	schema:contactPoint <http://orcid.org/0000-0001-8181-0758/contactPoint>;
. 
<http://www.ineris.fr> a schema:Organization;
	schema:identifier [ a schema:PropertyValue;
		schema:propertyID "URL";
		schema:value "http://www.ineris.fr";
	]; 
	schema:legalName "INERIS, Institut National de l'Environnement Industriel et des Risques";
	schema:address [ a schema:PostalAddress;
		schema:streetAddress "Parc Technologique Alata, BP 2";
		schema:addressLocality "Verneuil-en-Halatte";
		schema:postalCode "60550";
		schema:addressCountry "France";
	]; 
	schema:url "http://www.ineris.fr/"^^xsd:anyURI;
	schema:email "emmanuelle.klein@ineris.fr";
	schema:contactPoint <mailto:jannes-l.kinscher@ineris.fr/contactPoint>;
. 
<mailto:university.of.oulu@oulu.fi> a schema:Organization;
	schema:identifier [ a schema:PropertyValue;
		schema:propertyID "mailto";
		schema:value "university.of.oulu@oulu.fi";
	]; 
	schema:legalName "University of Oulu (UoO)";
	schema:address [ a schema:PostalAddress;
		schema:streetAddress "P.O. BOX 8000";
		schema:addressLocality "Oulu";
		schema:postalCode "FI-90014";
		schema:addressCountry "Finland";
	]; 
	schema:url "http://www.oulu.fi/university/"^^xsd:anyURI;
	schema:email "university.of.oulu@oulu.fi";
	schema:contactPoint <mailto:jouni.nevalainen@oulu.fi/contactPoint>;
. 
<PIC:999472675> a schema:Organization;
	schema:identifier [ a schema:PropertyValue;
		schema:propertyID "pic";
		schema:value "999472675";
	]; 
	schema:legalName "Istituto Nazionale di Geofisica e Vulcanologia";
	schema:address [ a schema:PostalAddress;
		schema:streetAddress "Via di Vigna Murata 605";
		schema:addressLocality "Rome";
		schema:postalCode "00143";
		schema:addressCountry "Italy";
	]; 
	schema:logo "http://roma2.rm.ingv.it/userfiles/file/Logo/INGV_Logo-abbr_colore.jpg"^^xsd:anyURI;
	schema:url "http://www.ingv.it"^^xsd:anyURI;
	schema:email "ufficiostampa@ingv.it";
	schema:contactPoint <http://orcid.org/0000-0003-2915-1446/contactPoint>;
	schema:contactPoint <http://orcid.org/0000-0003-3844-5059/contactPoint>;
. 
<PIC:999862324> a schema:Organization;
	schema:identifier [ a schema:PropertyValue;
		schema:propertyID "pic";
		schema:value "999862324";
	]; 
	schema:legalName "Keele University";
	schema:address [ a schema:PostalAddress;
		schema:streetAddress "Staffordshire";
		schema:addressLocality "Keele";
		schema:postalCode "ST5 5BJ";
		schema:addressCountry "United Kingdom";
	]; 
	schema:logo "https://www.keele.ac.uk/media/keeleuniversity/styleassets/images/logo.png"^^xsd:anyURI;
	schema:url "https://www.keele.ac.uk/"^^xsd:anyURI;
	schema:email "chancellors.reception@keele.ac.uk";
	schema:contactPoint <http://orcid.org/0000-0002-0769-5277/contactPoint>;
. 
<https://isterre.fr> a schema:Organization;
	schema:identifier [ a schema:PropertyValue;
		schema:propertyID "URL";
		schema:value "https://isterre.fr";
	]; 
	schema:legalName "CNRS, ISTerre, Université Grenoble Alpes";
	schema:address [ a schema:PostalAddress;
		schema:streetAddress "38058 GRENOBLE Cedex 9";
		schema:addressLocality "Grenoble";
		schema:postalCode "CS 40700";
		schema:addressCountry "France";
	]; 
	schema:url "https://isterre.fr/"^^xsd:anyURI;
	schema:telephone "+33 (0)4 76 635 200";
	schema:contactPoint <http://orcid.org/0000-0002-9580-7864/contactPoint>;
	schema:contactPoint <mailto:abror.karimov@univ-grenoble-alpes.fr/contactPoint>;
. 
<PIC:999527286> a schema:Organization;
	schema:identifier [ a schema:PropertyValue;
		schema:propertyID "pic";
		schema:value "999527286";
	]; 
	schema:legalName "AMRA – Analysis and Monitoring of Environmental Risk";
	schema:address [ a schema:PostalAddress;
		schema:streetAddress "Via Nuova Agnano, 11";
		schema:addressLocality "Napoli";
		schema:postalCode "80125";
		schema:addressCountry "Italy";
	]; 
	schema:url "http://www.amracenter.com/"^^xsd:anyURI;
	schema:email "info@amracenter.com";
	schema:telephone "+390817685125";
	schema:contactPoint <https://orcid.org/0000-0001-8078-9416/contactPoint>;
. 
<PIC:999518944> a schema:Organization;
	schema:identifier [ a schema:PropertyValue;
		schema:propertyID "pic";
		schema:value "999518944";
	]; 
	schema:legalName "The Royal Netherlands Meteorological Institute, KNMI";
	schema:address [ a schema:PostalAddress;
		schema:streetAddress "Utrechtseweg 297";
		schema:addressLocality "De Bilt";
		schema:postalCode "3731 GA";
		schema:addressCountry "The Netherlands";
	]; 
	schema:logo "http://cdn.knmi.nl/assets/logo_large-1f49334b8856e16f352187f1b52d0edf258976c6329407b0b75f5f109ea012fb.png"^^xsd:anyURI;
	schema:url "http://www.knmi.nl"^^xsd:anyURI;
	schema:contactPoint <http://orcid.org/0000-0001-7153-5115/contactPoint>;
.
<PIC:974007459> a schema:Organization;
	schema:identifier [ a schema:PropertyValue;
		schema:propertyID "pic";
		schema:value "974007459";
	]; 
	schema:legalName "Reykjavik Energy";
	schema:address [ a schema:PostalAddress;
		schema:streetAddress "Bæjarháls 1";
		schema:addressLocality "Reykjavík";
		schema:addressCountry "Iceland";
	]; 
	schema:logo "https://www.or.is/english/about-or/logo"^^xsd:anyURI;
	schema:url "https://www.or.is"^^xsd:anyURI;
	schema:contactPoint <https://orcid.org/0000-0003-2989-1663/contactPoint>;
.
<https://www.sgsw.ch> a schema:Organization;
	schema:identifier [ a schema:PropertyValue;
		schema:propertyID "URL";
		schema:value "https://www.sgsw.ch";
	]; 
	schema:legalName "St.Galler Stadtwerke";
	schema:address [ a schema:PostalAddress;
		schema:streetAddress "Vadianstrasse 8";
		schema:addressLocality "St.Gallen";
		schema:postalCode "9001";
		schema:addressCountry "Switzerland";
	]; 
	schema:url "https://www.sgsw.ch"^^xsd:anyURI;
	schema:contactPoint <mailto:thomas.bloch@sgsw.ch/contactPoint>;
.
<https://eost.unistra.fr> a schema:Organization;
	schema:identifier [ a schema:PropertyValue;
		schema:propertyID "URL";
		schema:value "https://eost.unistra.fr";
	]; 
	schema:legalName "Ecole et Observatoire des Sciences de la Terre";
	schema:address [ a schema:PostalAddress;
		schema:streetAddress "5 Rue René Descartes";
		schema:addressLocality "Strasbourg";
		schema:postalCode "67084";
		schema:addressCountry "France";
	]; 
	schema:url "https://eost.unistra.fr"^^xsd:anyURI;
	schema:email "contact@eost.unistra.fr";
	schema:contactPoint <http://orcid.org/0000-0003-4017-4673/contactPoint>;
.
<http://en.isor.is/> a schema:Organization;
    schema:identifier [ a schema:PropertyValue;
        schema:propertyID "URL";
        schema:value "http://en.isor.is/";
    ]; 
    schema:legalName "Iceland Geosurvey";
    schema:address [ a schema:PostalAddress;
        schema:streetAddress "Grensásvegi 9";
        schema:addressLocality "Reykjavík";
        schema:postalCode "108";
        schema:addressCountry "Iceland";
    ]; 
    schema:logo "http://en.isor.is/sites/en.isor.is/files/logo.png"^^xsd:anyURI;
    schema:url "http://en.isor.is/"^^xsd:anyURI;
    schema:contactPoint <mailto:Egill.Arni.Gudnason@isor.is/contactPoint>;
.


<http://orcid.org/0000-0002-4801-4888> a schema:Person;
	schema:identifier [ a schema:PropertyValue;
		schema:propertyID "orcid";
		schema:value "0000-0002-4801-4888";
	]; 
	schema:familyName "Lizurek";
	schema:givenName "Grzegorz";
	schema:address [ a schema:PostalAddress;
		schema:streetAddress "Księcia Janusza 64";
		schema:addressLocality "Warszawa";
		schema:postalCode "01-452";
		schema:addressCountry "Poland";
	]; 
	schema:email "lizurek@igf.edu.pl";
	schema:telephone "+48226915777";
	schema:url "http://www.igf.edu.pl/grzegorz-lizurek-phd.php"^^xsd:anyURI;
	schema:affiliation <PIC:996625337>;
	schema:contactPoint <http://orcid.org/0000-0002-4801-4888/contactPoint>;
. 
<mailto:m.sterzel@cyfronet.pl> a schema:Person;
	schema:identifier [ a schema:PropertyValue;
		schema:propertyID "mailto";
		schema:value "mailto:m.sterzel@cyfronet.pl";
	]; 
	schema:familyName "Sterzel";
	schema:givenName "Mariusz";
	schema:address [ a schema:PostalAddress;
		schema:streetAddress "Nawojki 11";
		schema:addressLocality "Krakow";
		schema:postalCode "30-950";
		schema:addressCountry "Poland";
	]; 
	schema:email "m.sterzel@cyfronet.pl";
	schema:telephone "+48126323355";
	schema:affiliation <PIC:999844573>;
	schema:contactPoint <mailto:m.sterzel@cyfronet.pl/contactPoint>;
. 
<https://orcid.org/0000-0002-9824-7962> a schema:Person;
	schema:identifier [ a schema:PropertyValue;
		schema:propertyID "orcid";
		schema:value "0000-0002-9824-7962";
	]; 
	schema:familyName "Kocot";
	schema:givenName "Joanna";
	schema:address [ a schema:PostalAddress;
		schema:streetAddress "Nawojki 11";
		schema:addressLocality "Krakow";
		schema:postalCode "30-950";
		schema:addressCountry "Poland";
	]; 
	schema:email "j.kocot@cyfronet.pl";
	schema:telephone "+48126323355";
	schema:affiliation <PIC:999844573>;
	schema:contactPoint <https://orcid.org/0000-0002-9824-7962/contactPoint>;
. 
<mailto:a_blanke@gfz-potsdam.de> a schema:Person;
	schema:identifier [ a schema:PropertyValue;
		schema:propertyID "mailto";
		schema:value "a_blanke@gfz-potsdam.de";
	]; 
	schema:familyName "Blanke";
	schema:givenName "Aglaja";
	schema:address [ a schema:PostalAddress;
		schema:streetAddress "14473 Potsdam";
		schema:addressLocality "Potsdam";
		schema:postalCode "14473";
		schema:addressCountry "Germany";
	]; 
	schema:email "a_blanke@gfz-potsdam.de";
	schema:affiliation <PIC:999994341>;
. 
<http://orcid.org/0000-0003-1076-615X> a schema:Person;
	schema:identifier [ a schema:PropertyValue;
		schema:propertyID "orcid";
		schema:value "0000-0003-1076-615X";
	]; 
	schema:familyName "Kwiatek";
	schema:givenName "Grzegorz";
	schema:address [ a schema:PostalAddress;
		schema:streetAddress "14473 Potsdam";
		schema:addressLocality "Potsdam";
		schema:postalCode "14473";
		schema:addressCountry "Germany";
	]; 
	schema:email "kwiatek@gfz-potsdam.de";
	schema:affiliation <PIC:999994341>;
	schema:contactPoint <http://orcid.org/0000-0003-1076-615X/contactPoint>;
. 
<mailto:giangnv@igp-vast.vn> a schema:Person;
	schema:identifier [ a schema:PropertyValue;
		schema:propertyID "mailto";
		schema:value "giangnv@igp-vast.vn";
	]; 
	schema:familyName "Van Giang";
	schema:givenName "Nguyen";
	schema:address [ a schema:PostalAddress;
		schema:streetAddress "A8 Building - 18 Hoang Quoc Viet - Cau Giay - Hanoi - Vietnam";
		schema:addressLocality "Hanoi";
		schema:addressCountry "Vietnam";
	]; 
	schema:email "giangnv@igp-vast.vn";
	schema:affiliation <https://www.igp-vast.vn/>;
	schema:contactPoint <mailto:giangnv@igp-vast.vn/contactPoint>;
. 
<http://orcid.org/0000-0001-8181-0758> a schema:Person;
	schema:identifier [ a schema:PropertyValue;
		schema:propertyID "orcid";
		schema:value "0000-0001-8181-0758";
	]; 
	schema:familyName "Mutke";
	schema:givenName "Grzegorz";
	schema:address [ a schema:PostalAddress;
		schema:streetAddress "Plac Gwarków 1";
		schema:addressLocality "Katowice";
		schema:postalCode "40-166";
		schema:addressCountry "Poland";
	]; 
	schema:email "gmutke@gig.eu";
	schema:affiliation <PIC:999516616>;
	schema:contactPoint <http://orcid.org/0000-0001-8181-0758/contactPoint>;
. 
<mailto:jannes-l.kinscher@ineris.fr> a schema:Person;
	schema:identifier [ a schema:PropertyValue;
		schema:propertyID "mailto";
		schema:value "jannes-l.kinscher@ineris.fr";
	]; 
	schema:familyName "Kinscher";
	schema:givenName "Jannes L.";
	schema:address [ a schema:PostalAddress;
		schema:streetAddress "Parc Technologique Alata, BP 2";
		schema:addressLocality "Verneuil-en-Halatte";
		schema:postalCode "60550";
		schema:addressCountry "France";
	]; 
	schema:email "jannes-l.kinscher@ineris.fr";
	schema:affiliation <http://www.ineris.fr>;
	schema:contactPoint <mailto:jannes-l.kinscher@ineris.fr/contactPoint>;
. 
<mailto:jouni.nevalainen@oulu.fi> a schema:Person;
	schema:identifier [ a schema:PropertyValue;
		schema:propertyID "mailto";
		schema:value "jouni.nevalainen@oulu.fi";
	]; 
	schema:familyName "Nevalainen";
	schema:givenName "Jouni";
	schema:address [ a schema:PostalAddress;
		schema:streetAddress "P.O. BOX 8000";
		schema:addressLocality "Oulu";
		schema:postalCode "FI-90014";
		schema:addressCountry "Finland";
	]; 
	schema:email "jouni.nevalainen@oulu.fi";
	schema:affiliation <mailto:university.of.oulu@oulu.fi>;
	schema:contactPoint <mailto:jouni.nevalainen@oulu.fi/contactPoint>;
.
<http://orcid.org/0000-0003-2915-1446> a schema:Person;
	schema:identifier [ a schema:PropertyValue;
		schema:propertyID "orcid";
		schema:value "0000-0003-2915-1446";
	]; 
	schema:familyName "Saccorotti";
	schema:givenName "Gilberto";
	schema:address [ a schema:PostalAddress;
		schema:streetAddress "Via della Faggiola 32";
		schema:addressLocality "Pisa";
		schema:postalCode "56126";
		schema:addressCountry "Italy";
	]; 
	schema:email "gilberto.saccorotti@ingv.it";
	schema:affiliation <PIC:999472675>;
. 
<http://orcid.org/0000-0003-3844-5059> a schema:Person;
	schema:identifier [ a schema:PropertyValue;
		schema:propertyID "orcid";
		schema:value "0000-0003-3844-5059";
	]; 
	schema:familyName "Roselli";
	schema:givenName "Pamela";
	schema:address [ a schema:PostalAddress;
		schema:streetAddress "Via di Vigna Murata 605";
		schema:addressLocality "Rome";
		schema:postalCode "00143";
		schema:addressCountry "Italy";
	]; 
	schema:email "pamela.roselli@ingv.it";
	schema:affiliation <PIC:999472675>;
	schema:contactPoint <http://orcid.org/0000-0003-3844-5059/contactPoint>;
. 
<http://orcid.org/0000-0001-9196-8452> a schema:Person;
	schema:identifier [ a schema:PropertyValue;
		schema:propertyID "orcid";
		schema:value "0000-0001-9196-8452";
	]; 
	schema:familyName "Alexander";
	schema:givenName "Garcia";
	schema:address [ a schema:PostalAddress;
		schema:streetAddress "Via di Vigna Murata 605";
		schema:addressLocality "Rome";
		schema:postalCode "00143";
		schema:addressCountry "Italy";
	]; 
	schema:email "alexander.garcia@ingv.it";
	schema:affiliation <PIC:999472675>;
	schema:contactPoint <http://orcid.org/0000-0001-9196-8452/contactPoint>;
. 
<http://orcid.org/0000-0002-0769-5277> a schema:Person;
	schema:identifier [ a schema:PropertyValue;
		schema:propertyID "orcid";
		schema:value "0000-0002-0769-5277";
	]; 
	schema:familyName "Jones";
	schema:givenName "Glenda";
	schema:address [ a schema:PostalAddress;
		schema:streetAddress "Staffordshire";
		schema:addressLocality "Keele";
		schema:postalCode "ST5 5BJ";
		schema:addressCountry "United Kingdom";
	]; 
	schema:email "g.m.jones@keele.ac.uk";
	schema:affiliation <PIC:999862324>;
	schema:contactPoint <http://orcid.org/0000-0002-0769-5277/contactPoint>;
. 
<http://orcid.org/0000-0002-9580-7864> a schema:Person;
	schema:identifier [ a schema:PropertyValue;
		schema:propertyID "orcid";
		schema:value "0000-0002-9580-7864";
	]; 
	schema:familyName "Grasso";
	schema:givenName "Jean-Robert";
	schema:address [ a schema:PostalAddress;
		schema:streetAddress "38058 GRENOBLE Cedex 9";
		schema:addressLocality "Grenoble";
		schema:postalCode "CS 40700";
		schema:addressCountry "France";
	]; 
	schema:email "jean-robert.grasso@univ-grenoble-alpes.fr";
	schema:affiliation <https://isterre.fr>;
	schema:contactPoint <http://orcid.org/0000-0002-9580-7864/contactPoint>;
. 
<mailto:abror.karimov@univ-grenoble-alpes.fr> a schema:Person;
	schema:identifier [ a schema:PropertyValue;
		schema:propertyID "mailto";
		schema:value "abror.karimov@univ-grenoble-alpes.fr";
	]; 
	schema:familyName "Karimov";
	schema:givenName "Abror";
	schema:address [ a schema:PostalAddress;
		schema:streetAddress "38058 GRENOBLE Cedex 9";
		schema:addressLocality "Grenoble";
		schema:postalCode "CS 40700";
		schema:addressCountry "France";
	]; 
	schema:email "abror.karimov@univ-grenoble-alpes.fr";
	schema:affiliation <https://isterre.fr>;
	schema:contactPoint <mailto:abror.karimov@univ-grenoble-alpes.fr/contactPoint>;
. 
<https://orcid.org/0000-0001-8078-9416> a schema:Person;
	schema:identifier [ a schema:PropertyValue;
		schema:propertyID "orcid";
		schema:value "0000-0001-8078-9416";
	]; 
	schema:familyName "Picozzi";
	schema:givenName "Matteo";
	schema:address [ a schema:PostalAddress;
		schema:streetAddress "Via Nuova Agnano, 11";
		schema:addressLocality "Naples";
		schema:postalCode "80125";
		schema:addressCountry "Italy";
	]; 
	schema:email "matteo.picozzi@unina.it";
	schema:affiliation <PIC:999527286>;
	schema:contactPoint <https://orcid.org/0000-0001-8078-9416/contactPoint>;
. 
<http://orcid.org/0000-0001-7153-5115> a schema:Person;
	schema:identifier [ a schema:PropertyValue;
		schema:propertyID "orcid";
		schema:value "0000-0001-7153-5115";
	]; 
	schema:familyName "Ruigrok";
	schema:givenName "Elmer";
	schema:address [ a schema:PostalAddress;
		schema:streetAddress "Utrechtseweg 297";
		schema:addressLocality "De Bilt";
		schema:postalCode "3731 GA";
		schema:addressCountry "The Netherlands";
	]; 
	schema:email "E.N.Ruigrok@uu.nl";
	schema:affiliation <PIC:999518944>;
	schema:contactPoint <http://orcid.org/0000-0001-7153-5115/contactPoint>;
. 
<https://orcid.org/0000-0003-2989-1663> a schema:Person;
	schema:identifier [ a schema:PropertyValue;
		schema:propertyID "orcid";
		schema:value "0000-0003-2989-1663";
	]; 
	schema:familyName "Snæbjörnsdóttir";
	schema:givenName "Sandra Ósk";
	schema:address [ a schema:PostalAddress;
		schema:streetAddress "Bæjarháls 1";
		schema:addressLocality "Reykjavík";
		schema:addressCountry "Iceland";
	];
	schema:email "sandra.osk.snaebjornsdottir@or.is";
	schema:affiliation <PIC:974007459>;
	schema:contactPoint <https://orcid.org/0000-0003-2989-1663/contactPoint>;
. 
<mailto:thomas.bloch@sgsw.ch> a schema:Person;
	schema:identifier [ a schema:PropertyValue;
		schema:propertyID "mailto";
		schema:value "thomas.bloch@sgsw.ch";
	]; 
	schema:familyName "Bloch";
	schema:givenName "Thomas";
	schema:address [ a schema:PostalAddress;
		schema:streetAddress "Vadianstrasse 8";
		schema:addressLocality "St.Gallen";
		schema:postalCode "9001";
		schema:addressCountry "Switzerland";
	];
	schema:email "thomas.bloch@sgsw.ch";
	schema:affiliation <https://www.sgsw.ch>;
	schema:contactPoint <mailto:thomas.bloch@sgsw.ch/contactPoint>;
. 
<http://orcid.org/0000-0003-4017-4673> a schema:Person;
	schema:identifier [ a schema:PropertyValue;
		schema:propertyID "orcid";
		schema:value "0000-0003-4017-4673";
	]; 
	schema:familyName "Schaming";
	schema:givenName "Marc";
	schema:address [ a schema:PostalAddress;
		schema:streetAddress "5 Rue René Descartes";
		schema:addressLocality "Strasbourg";
		schema:postalCode "67084";
		schema:addressCountry "France";
	]; 
	schema:email "Marc.Schaming@unistra.fr";
	schema:telephone "+33368850093";
	schema:affiliation <https://eost.unistra.fr>;
	schema:contactPoint <http://orcid.org/0000-0003-4017-4673/contactPoint>;
. 
<mailto:Egill.Arni.Gudnason@isor.is> a schema:Person;
    schema:identifier [ a schema:PropertyValue;
        schema:propertyID "mailto";
        schema:value "Egill.Arni.Gudnason@isor.is";
    ]; 
    schema:familyName "Gudnason";
    schema:givenName "Egil Arni";
    schema:address [ a schema:PostalAddress;
        schema:streetAddress "Grensásvegi 9";
        schema:addressLocality "Reykjavík";
        schema:postalCode "108";
        schema:addressCountry "Iceland";
    ];
    schema:email "Egill.Arni.Gudnason@isor.is";
    schema:affiliation <http://en.isor.is/>;
    schema:contactPoint <mailto:Egill.Arni.Gudnason@isor.is/contactPoint>;
.

	<epos:Anthropogenichazards> a skos:ConceptScheme;
		dct:title "Anthropogenic hazards";
		dct:description "It contains the concepts of anthropogenic hazards";
. 
	<epos:Reservoirimpoundment> a skos:Concept;
		skos:inScheme <epos:Anthropogenichazards>;
		skos:prefLabel "reservoir impoundment";
. 
	<epos:Geothermalenergyproduction> a skos:Concept;
		skos:inScheme <epos:Anthropogenichazards>;
		skos:prefLabel "geothermal energy production";
. 
	<epos:Hardrockmining> a skos:Concept;
		skos:inScheme <epos:Anthropogenichazards>;
		skos:prefLabel "hard rock mining";
. 
	<epos:Coalmining> a skos:Concept;
		skos:inScheme <epos:Anthropogenichazards>;
		skos:prefLabel "coal mining";
. 
	<epos:Saltsolutionsmining> a skos:Concept;
		skos:inScheme <epos:Anthropogenichazards>;
		skos:prefLabel "salt solutions mining";
. 
	<epos:Unconventionalhydrocarbonextraction> a skos:Concept;
		skos:inScheme <epos:Anthropogenichazards>;
		skos:prefLabel "unconventional hydrocarbon extraction";
. 
	<epos:Conventionalhydrocarbonextraction> a skos:Concept;
		skos:inScheme <epos:Anthropogenichazards>;
		skos:prefLabel "conventional hydrocarbon extraction";
. 

	<epos:CollectivePropertiesOfSeismicityAnalysis> a skos:Concept;
		skos:inScheme <epos:Anthropogenichazards>;
		skos:prefLabel "collective properties of seismicity analysis";
. 
	<epos:Converters> a skos:Concept;
		skos:inScheme <epos:Anthropogenichazards>;
		skos:prefLabel "converters";
. 
	<epos:CorrelationAnalysis> a skos:Concept;
		skos:inScheme <epos:Anthropogenichazards>;
		skos:prefLabel "correlation analysis";
. 
	<epos:Dataprocessingapplications> a skos:Concept;
		skos:inScheme <epos:Anthropogenichazards>;
		skos:prefLabel "data processing applications";
. 
	<epos:DownloadTools> a skos:Concept;
		skos:inScheme <epos:Anthropogenichazards>;
		skos:prefLabel "download tools";
. 
	<epos:EarthquakeInteractionsAnalysis> a skos:Concept;
		skos:inScheme <epos:Anthropogenichazards>;
		skos:prefLabel "earthquake interactions analysis";
. 
	<epos:EventDetectionAlgorithms> a skos:Concept;
		skos:inScheme <epos:Anthropogenichazards>;
		skos:prefLabel "event detection algorithms";
. 
	<epos:FilteringTools> a skos:Concept;
		skos:inScheme <epos:Anthropogenichazards>;
		skos:prefLabel "filtering tools";
. 
	<epos:ProbabilisticSeismicHazardAnalysis> a skos:Concept;
		skos:inScheme <epos:Anthropogenichazards>;
		skos:prefLabel "probabilistic seismic hazard analysis";
. 
	<epos:SeismogramAnalysisTools> a skos:Concept;
		skos:inScheme <epos:Anthropogenichazards>;
		skos:prefLabel "seismogram analysis tools";
. 
	<epos:SourceParameterEstimation> a skos:Concept;
		skos:inScheme <epos:Anthropogenichazards>;
		skos:prefLabel "source parameter estimation";
.
	<epos:StressFieldModeling> a skos:Concept;
		skos:inScheme <epos:Anthropogenichazards>;
		skos:prefLabel "stress field modeling";
.
	<epos:Visualizations> a skos:Concept;
		skos:inScheme <epos:Anthropogenichazards>;
		skos:prefLabel "visualizations";
.


	<anthropogenic_hazards/dataset/virtual_access> a dcat:Dataset;
		dct:title "Virtual access to IS-EPOS Platform";
		dct:identifier "anthropogenic_hazards/dataset/virtual_access";
		adms:identifier [ a adms:Identifier;
			adms:schemaAgency "DDSS-ID";
			skos:notation "WP14-DDSS-001";
		];
  	adms:identifier [ a adms:Identifier;
      adms:schemaAgency "DOI";
      skos:notation "10.1007/s11600-018-0209-z";
    ];
		dct:description "Virtual access to IS-EPOS Platform";
		dct:created "2015-10-20"^^xsd:date;
		dct:modified "2018-07-30"^^xsd:date;
		dct:temporal [ a dct:PeriodOfTime; 
      schema:startDate "1956-06-01T00:00:00Z"^^xsd:dateTime;
    ];
		dcat:theme <epos:Reservoirimpoundment>;
		dcat:theme <epos:Geothermalenergyproduction>;
		dcat:theme <epos:Hardrockmining>;
		dcat:theme <epos:Coalmining>;
		dcat:theme <epos:Saltsolutionsmining>;
		dcat:theme <epos:Conventionalhydrocarbonextraction>;
		dcat:theme <epos:Unconventionalhydrocarbonextraction>;
		dcat:theme <epos:CollectivePropertiesOfSeismicityAnalysis>;
    dcat:theme <epos:Converters>;
    dcat:theme <epos:CorrelationAnalysis>;
    dcat:theme <epos:Dataprocessingapplications>;
    dcat:theme <epos:DownloadTools>;
    dcat:theme <epos:EarthquakeInteractionsAnalysis>;
    dcat:theme <epos:EventDetectionAlgorithms>;
    dcat:theme <epos:FilteringTools>;
    dcat:theme <epos:ProbabilisticSeismicHazardAnalysis>;
    dcat:theme <epos:SeismogramAnalysisTools>;
    dcat:theme <epos:SourceParameterEstimation>;
    dcat:theme <epos:StressFieldModeling>;
    dcat:theme <epos:Visualizations>;
		dcat:keyword "anthropogenic hazards","TCS AH","IS-EPOS platform","web platform","multiservice","research environment","workspace","applications","episode","document repository";
		dct:publisher <PIC:996625337>;
		dcat:contactPoint <mailto:m.sterzel@cyfronet.pl/contactPoint>;
		dcat:distribution <anthropogenic_hazards/distribution/episodes>;
		dcat:distribution <anthropogenic_hazards/distribution/apps>;
. 
	<anthropogenic_hazards/dataset/episode/CZORSZTYN> a dcat:Dataset;
		dct:title "CZORSZTYN: shallow water reservoir";
		dct:identifier "anthropogenic_hazards/dataset/episode/CZORSZTYN";
		adms:identifier [ a adms:Identifier;
			adms:schemaAgency "DDSS-ID";
			skos:notation "WP14-DDSS-002";
		]; 
		adms:identifier [ a adms:Identifier;
      adms:schemaAgency "DOI";
      skos:notation "10.25171/InstGeoph_PAS_ISEPOS-2017-004";
    ];
    dct:description "Seismic activity linked to the impoundment of Czorsztyn artificial lake. The lake was created by backing up water by an earth dam of the hydropower plant Niedzica on Dunajec river in south of Poland. Its filling ended in 1997. The reservoir of 234.5 milion cubic meters capacity is shallow, on average between 20 to 50 m of water column. Seismic activity began in 2011.  Episode integrated in the framework of: IS-EPOS project, Digital Research Space of Induced Seismicity for EPOS Purposes No. POIG.02.03.00-14-090/13. How to cite: IS EPOS (2017), Episode: CZORSZTYN, https://tcs.ah-epos.eu/#episode:CZORSZTYN, doi:10.25171/InstGeoph_PAS_ISEPOS-2017-004";
		dct:accrualPeriodicity "http://purl.org/cld/freq/quarterly"^^xsd:anyURI ;
		dct:created "2015-10-20"^^xsd:date;
		dct:modified "2018-06-27"^^xsd:date;
		dct:issued "2017-08-03"^^xsd:date;
		dct:temporal [ a dct:PeriodOfTime; 
			schema:startDate "2013-08-25T00:00:00Z"^^xsd:dateTime;
		];
		dct:spatial [ a dct:Location;
	        locn:geometry "POINT(20.323325 49.419624)"^^gsp:wktLiteral;
	    ];
		dcat:theme <epos:Reservoirimpoundment>;
		dcat:keyword "anthropogenic hazards","TCS AH","IS-EPOS platform", "episode", "reservoir impoundment", "anthropogenic seismicity", "catalogue", "seismic waveform", "station information", "reservoir industrial data", "water level", "velocity model";
		dct:publisher <PIC:996625337>;
		dcat:contactPoint <http://orcid.org/0000-0002-4801-4888/contactPoint>;
		dcat:distribution <anthropogenic_hazards/distribution/episode-elements/CZORSZTYN>;
. 
	<anthropogenic_hazards/dataset/episode/GS> a dcat:Dataset;
		dct:title "GROSS SCHOENEBECK: geothermal energy production experiment";
		dct:identifier "anthropogenic_hazards/dataset/episode/GS";
		adms:identifier [ a adms:Identifier;
			adms:schemaAgency "DDSS-ID";
			skos:notation "WP14-DDSS-003";
		]; 
		adms:identifier [ a adms:Identifier;
      adms:schemaAgency "DOI";
      skos:notation "10.25171/InstGeoph_PAS_ISEPOS-2017-005";
    ];
    dct:description "An injection deep well and a doublet of production wells were established in this area reaching the reservoir rocks like red bed sandstone and andesitic volcanic rock at the 4200m depth. Injection performed from 9th to 14th August 2007 was used for repeated stimulation treatments to investigate scenarios of enhancing productivity of thermal fluid recovery from the underground. A total amount of 13.000 m^3 of water was injected. The maximum injection well-head pressure reached 58.6 MPa.  Episode integrated in the framework of: IS-EPOS project, Digital Research Space of Induced Seismicity for EPOS Purposes No. POIG.02.03.00-14-090/13 • SHEER project, SHale gas Exploration and Exploitation induced Risks project has received funding from the European Union's Horizon 2020 research and innovation programme under grant agreement No 640896 • EPOS IP project, European Plate Observing System Implementation Phase. This project has received funding from the European Union’s Horizon 2020 research and innovation programme under grant agreement No 676564.  How to cite: IS EPOS (2017), Episode: GROSS SCHOENEBECK, https://tcs.ah-epos.eu/#episode:GS, doi:10.25171/InstGeoph_PAS_ISEPOS-2017-005";
		dct:created "2015-10-20"^^xsd:date;
		dct:modified "2018-05-01"^^xsd:date;
		dct:issued "2017-08-03"^^xsd:date;
		dct:temporal [ a dct:PeriodOfTime; 
			schema:startDate "2007-08-09T00:00:00Z"^^xsd:dateTime; 
			schema:endDate "2007-08-19T00:00:00Z"^^xsd:dateTime; 
		];
		dct:spatial [ a dct:Location;
	        locn:geometry "POINT(13.653131 52.915086)"^^gsp:wktLiteral;
	    ];
		dcat:theme <epos:Geothermalenergyproduction>;
		dcat:keyword "anthropogenic hazards","TCS AH","IS-EPOS platform", "episode", "geothermal energy production", "anthropogenic seismicity", "catalogue", "seismic waveform", "station information", "injection industrial data", "velocity model";
		dct:publisher <PIC:999994341>;
		dcat:contactPoint <http://orcid.org/0000-0003-1076-615X/contactPoint>;
		dcat:contactPoint <mailto:a_blanke@gfz-potsdam.de/contactPoint>;
		dcat:distribution <anthropogenic_hazards/distribution/episode-elements/GS>;
. 
	<anthropogenic_hazards/dataset/episode/LGCD> a dcat:Dataset;
		dct:title "LGCD: regional seismicity and ground motion associating underground hard rock mining";
		dct:identifier "anthropogenic_hazards/dataset/episode/LGCD";
		adms:identifier [ a adms:Identifier;
			adms:schemaAgency "DDSS-ID";
			skos:notation "WP14-DDSS-004";
		]; 
		adms:identifier [ a adms:Identifier;
      adms:schemaAgency "DOI";
      skos:notation "10.25171/InstGeoph_PAS_ISEPOS-2017-006";
    ];
    dct:description "Seismicity induced by underground copper ore exploitation in mines located in the Legnica-Glogow Copper District (LGCD), southwestern Poland. Mines use a room and pillar exploitation system at the level from 0.6 to 1.3 km below surface. Episode LGCD contains only seismic events recorded inside the seismic network.  Episode integrated in the framework of: IS-EPOS project, Digital Research Space of Induced Seismicity for EPOS Purposes No. POIG.02.03.00-14-090/13.  How to cite: IS EPOS (2017), Episode: LGCD, https://tcs.ah-epos.eu/#episode:LGCD, doi:10.25171/InstGeoph_PAS_ISEPOS-2017-006";
		dct:accrualPeriodicity "http://purl.org/cld/freq/quarterly"^^xsd:anyURI ;
		dct:created "2015-10-20"^^xsd:date;
		dct:modified "2018-08-23"^^xsd:date;
		dct:issued "2018-08-03"^^xsd:date;
		dct:temporal [ a dct:PeriodOfTime; 
			schema:startDate "2013-12-10T00:00:00Z"^^xsd:dateTime;
		];
		dct:spatial [ a dct:Location;
	        locn:geometry "POINT(16.106551 51.501023)"^^gsp:wktLiteral;
	    ];
		dcat:theme <epos:Hardrockmining>;
		dcat:keyword "anthropogenic hazards","TCS AH","IS-EPOS platform", "episode", "underground mining", "anthropogenic seismicity", "catalogue", "seismic waveform", "ground motion parameters", "station information", "mine industrial data", "velocity model";
		dct:publisher <PIC:996625337>;
		dcat:contactPoint <http://orcid.org/0000-0002-4801-4888/contactPoint>;
		dcat:distribution <anthropogenic_hazards/distribution/episode-elements/LGCD>;
. 
	<anthropogenic_hazards/dataset/episode/SONG_TRANH> a dcat:Dataset;
		dct:title "SONG TRANH: deep water reservoir";
		dct:identifier "anthropogenic_hazards/dataset/episode/SONG_TRANH";
		adms:identifier [ a adms:Identifier;
			adms:schemaAgency "DDSS-ID";
			skos:notation "WP14-DDSS-005";
		]; 
		adms:identifier [ a adms:Identifier;
      adms:schemaAgency "DOI";
      skos:notation "10.25171/InstGeoph_PAS_ISEPOS-2017-002";
    ];
    dct:description "Seismic activity linked to Song Tranh 2 hydropower plant and the reservoir containing backed up water of Tranh river in central Vietnam. The reservoir volume is 740 million cubic meters and the water level varies between 140 and 175 m. Seismic activity in the reservoir region, previously known as aseismic, began in 2011, soon after filling of the reservoir.  Episode integrated in the framework of: IS-EPOS project, Digital Research Space of Induced Seismicity for EPOS Purposes No. POIG.02.03.00-14-090/13; EPOS IP project, European Plate Observing System Implementation Phase. This project has received funding from the European Union’s Horizon 2020 research and innovation programme under grant agreement No 676564.  How to cite: IS EPOS (2017), Episode: SONG TRANH, https://tcs.ah-epos.eu/#episode:SONG_TRANH, doi:10.25171/InstGeoph_PAS_ISEPOS-2017-002";
		dct:accrualPeriodicity "http://purl.org/cld/freq/quarterly"^^xsd:anyURI ;
		dct:created "2015-10-20"^^xsd:date;
		dct:modified "2018-03-05"^^xsd:date;
		dct:issued "2017-08-03"^^xsd:date;
		dct:temporal [ a dct:PeriodOfTime; 
			schema:startDate "2011-01-01T00:00:00Z"^^xsd:dateTime;
		];
		dct:spatial [ a dct:Location;
	        locn:geometry "POINT(108.148 15.331)"^^gsp:wktLiteral;
	    ];
		dcat:theme <epos:Reservoirimpoundment>;
		dcat:keyword "anthropogenic hazards","TCS AH","IS-EPOS platform", "episode", "reservoir impoundment", "anthropogenic seismicity", "catalogue", "seismic waveform", "station information", "reservoir industrial data", "water level", "fault", "velocity model";
		dct:publisher <PIC:996625337>;
		dcat:contactPoint <http://orcid.org/0000-0002-4801-4888/contactPoint>;
		dcat:contactPoint <mailto:giangnv@igp-vast.vn/contactPoint>;
		dcat:distribution <anthropogenic_hazards/distribution/episode-elements/SONG_TRANH>;
. 
	<anthropogenic_hazards/dataset/episode/USCB> a dcat:Dataset;
		dct:title "USCB: regional seismicity and ground motion associating underground coal mining";
		dct:identifier "anthropogenic_hazards/dataset/episode/USCB";
		adms:identifier [ a adms:Identifier;
			adms:schemaAgency "DDSS-ID";
			skos:notation "WP14-DDSS-006";
		]; 
		adms:identifier [ a adms:Identifier;
      adms:schemaAgency "DOI";
      skos:notation "10.25171/InstGeoph_PAS_ISEPOS-2017-007";
    ];
    dct:description "Seismic activity linked to underground coal mining in Upper Silesia Coal Basin (USCB) in Poland. Multilevel mine operations have been conducted for more than 200 years. Presently (2016), there are more than 20 seismically active mines.  Episode integrated in the framework of: IS-EPOS project, Digital Research Space of Induced Seismicity for EPOS Purposes No. POIG.02.03.00-14-090/13.  How to cite: IS EPOS (2017), Episode: USCB, https://tcs.ah-epos.eu/#episode:USCB, doi:10.25171/InstGeoph_PAS_ISEPOS-2017-007";
		dct:accrualPeriodicity "http://purl.org/cld/freq/quarterly"^^xsd:anyURI ;
		dct:created "2015-10-20"^^xsd:date;
		dct:modified "2019-08-06"^^xsd:date;
		dct:issued "2017-08-03"^^xsd:date;
		dct:temporal [ a dct:PeriodOfTime; 
			schema:startDate "2014-01-02T00:00:00Z"^^xsd:dateTime;
		];
		dct:spatial [ a dct:Location;
	        locn:geometry "POINT(19.080085 50.244433)"^^gsp:wktLiteral;
	    ];
		dcat:theme <epos:Coalmining>;
		dcat:keyword "anthropogenic hazards","TCS AH","IS-EPOS platform", "episode", "underground mining", "anthropogenic seismicity", "catalogue", "seismic waveform", "station information", "ground motion parameters", "mine industrial data", "fault", "shear wave velocity", "velocity model";
		dct:publisher <PIC:999516616>;
		dcat:contactPoint <http://orcid.org/0000-0001-8181-0758/contactPoint>;
		dcat:distribution <anthropogenic_hazards/distribution/episode-elements/USCB>;
. 
	<anthropogenic_hazards/dataset/episode/BOBREK> a dcat:Dataset;
		dct:title "BOBREK MINE: local seismicity linked to longwall mining";
		dct:identifier "anthropogenic_hazards/dataset/episode/BOBREK";
		adms:identifier [ a adms:Identifier;
			adms:schemaAgency "DDSS-ID";
			skos:notation "WP14-DDSS-007";
		]; 
		adms:identifier [ a adms:Identifier;
      adms:schemaAgency "DOI";
      skos:notation "10.25171/InstGeoph_PAS_ISEPOS-2017-003";
    ];
    dct:description "Bobrek Mine: local seismicity linked to longwall mining is the Laboratory for Monitoring Mining Induced Seismicity (LMMIS) of passive seismic records of seismicity induced and triggered by underground coal mining. The episode relates to seismic activity linked to longwall mining of panel 3 in coal seam 503 in Bobrek colliery in Upper Silesia Coal Basin in Poland. The coal seam no. 503 was 3.0 to 3.5 m thick in the area of longwall panel no. 3 and at the depth of 700 m below surface. The coal extraction was carried on in the period 1/04/2009-8/07/2010.  Episode integrated in the framework of: IS-EPOS project, Digital Research Space of Induced Seismicity for EPOS Purposes No. POIG.02.03.00-14-090/13.  How to cite: IS EPOS (2017), Episode: BOBREK, https://tcs.ah-epos.eu/#episode:BOBREK, doi:10.25171/InstGeoph_PAS_ISEPOS-2017-003";
		dct:created "2015-10-20"^^xsd:date;
		dct:modified "2018-02-02"^^xsd:date;
		dct:issued "2017-08-03"^^xsd:date;
		dct:temporal [ a dct:PeriodOfTime; 
			schema:startDate "2009-04-12T00:00:00Z"^^xsd:dateTime; 
			schema:endDate "2010-07-07T00:00:00Z"^^xsd:dateTime; 
		];
		dct:spatial [ a dct:Location;
	        locn:geometry "POINT(18.867014 50.351483)"^^gsp:wktLiteral;
	    ];
		dcat:theme <epos:Coalmining>;
		dcat:keyword "anthropogenic hazards","TCS AH","IS-EPOS platform", "episode", "underground mining", "anthropogenic seismicity", "catalogue", "seismic waveform", "station information", "mine industrial data", "velocity model";
		dct:publisher <PIC:999516616>;
		dcat:contactPoint <http://orcid.org/0000-0001-8181-0758/contactPoint>;
		dcat:distribution <anthropogenic_hazards/distribution/episode-elements/BOBREK>;
. 
	<anthropogenic_hazards/dataset/episode/PYHASALMI_MINE> a dcat:Dataset;
		dct:title "PYHASALMI MINE: in situ underground laboratory";
		dct:identifier "anthropogenic_hazards/dataset/episode/PYHASALMI_MINE";
		adms:identifier [ a adms:Identifier;
			adms:schemaAgency "DDSS-ID";
			skos:notation "WP14-DDSS-009";
		]; 
		adms:identifier [ a adms:Identifier;
      adms:schemaAgency "DOI";
      skos:notation "10.25171/InstGeoph_PAS_ISEPOS-2017-015";
    ];
    dct:description "Pyhasalmi mine, Central Finland, is an underground mine which produces copper, zinc and pyrite. A seismic network was installed underground in 2002 to monitor and locate frequently occurring microseismic scale events. Main target in Pyhasalmi episode is to: 1. Compare microseismic networks detected events with observations with national permanent seismic stations observations. 2. Correlate mining related microseismic events with the production data of the Pyhasalmi mine. 3. Analyze regions, where events concentrate and compare the locations with known geology. Pyhasalmi Episode consists of various data in order to track relation between seismicity and Pyhasalmi mine production. Data consists of seismic waverform and catalog, borehole information and basemaps.  Episode integrated in the framework of: EPOS IP project, European Plate Observing System Implementation Phase. This project has received funding from the European Union’s Horizon 2020 research and innovation programme under grant agreement No 676564.  How to cite: IS EPOS (2017), Episode: PYHASALMI MINE, https://tcs.ah-epos.eu/#episode:PYHASALMI_MINE, doi:10.25171/InstGeoph_PAS_ISEPOS-2017-015";
		dct:created "2017-09-12"^^xsd:date;
		dct:modified "2018-02-02"^^xsd:date;
		dct:issued "2017-09-12"^^xsd:date;
		dct:temporal [ a dct:PeriodOfTime; 
			schema:startDate "2010-10-01T00:00:00Z"^^xsd:dateTime; 
			schema:endDate "2011-03-31T00:00:00Z"^^xsd:dateTime; 
		];
		dct:spatial [ a dct:Location;
	        locn:geometry "POINT(26.042500 63.658889)"^^gsp:wktLiteral;
	    ];
		dcat:theme <epos:Hardrockmining>;
		dcat:keyword "anthropogenic hazards","TCS AH","IS-EPOS platform", "episode", "underground mining", "anthropogenic seismicity", "catalogue", "seismic waveform", "station information", "mine industrial data", "geology", "velocity model";
		dct:publisher <mailto:university.of.oulu@oulu.fi>;
		dcat:contactPoint <mailto:jouni.nevalainen@oulu.fi/contactPoint>;
		dcat:distribution <anthropogenic_hazards/distribution/episode-elements/PYHASALMI_MINE>;
. 
	<anthropogenic_hazards/dataset/episode/LGF> a dcat:Dataset;
		dct:title "LACQ GAS FIELD: conventional hydrocarbon extraction";
		dct:identifier "anthropogenic_hazards/dataset/episode/LGF";
		adms:identifier [ a adms:Identifier;
			adms:schemaAgency "DDSS-ID";
			skos:notation "WP14-DDSS-010";
		]; 
		adms:identifier [ a adms:Identifier;
      adms:schemaAgency "DOI";
      skos:notation "10.25171/InstGeoph_PAS_ISEPOS-2018-005";
    ];
    dct:description "The episode is related to a seismic swarm that developed contemporary to and in the vicinity of a deep conventional gas extraction, Lacq gas Field, Aquitaine, France. Onset of Lacq gas field production is 1958, when the first local M3 event occurred in 1969. Since this time, hundreds of shallow, small to moderate earthquakes (Mmax=4) have occurred near the Lacq deep gas field. These earthquakes are clearly separated from tectonic seismicity occurring in the Pyrenees, 25 km to the southwest. The induced seismicity began when the reservoir pressure had declined by 30 MPa. Repeated leveling over the field shows localized subsidence reaching a maximum of 60 mm in 1989. Episode data are (i) regional seismicity catalogue on the 1962-2009 period, local catalogue 1976-1995 period, respectively; (ii) yearly production volume, 1958-2016; (iii) yearly reservoir pressure drop, 1958-2016; (iv) yearly injected volume, 1958-2016. Episode integrated in the framework of: EPOS IP project, European Plate Observing System Implementation Phase. This project has received funding from the European Union’s Horizon 2020 research and innovation programme under grant agreement No 676564. How to cite: IS EPOS (2018), Episode: LACQ GAS FIELD, https://tcs.ah-epos.eu/#episode:LGF, doi:10.25171/InstGeoph_PAS_ISEPOS-2018-005.";
		dct:temporal [ a dct:PeriodOfTime; 
			schema:startDate "1977-12-31T00:00:00Z"^^xsd:dateTime; 
			schema:endDate "2016-12-31T00:00:00Z"^^xsd:dateTime; 
		];
		dct:spatial [ a dct:Location;
	        locn:geometry "POINT(0 43.5)"^^gsp:wktLiteral;
	    ];
		dcat:theme <epos:Conventionalhydrocarbonextraction>;
		dcat:keyword "anthropogenic hazards","TCS AH","IS-EPOS platform", "episode", "conventional hydrocarbon extraction", "anthropogenic seismicity", "catalogue", "station information", "reservoir industrial data", "injection industrial data", "hydrocarbon production data", "velocity model";
		dct:publisher <https://isterre.fr>;
		dcat:contactPoint <http://orcid.org/0000-0002-9580-7864/contactPoint>;
		dcat:contactPoint <mailto:abror.karimov@univ-grenoble-alpes.fr/contactPoint>;
		dcat:distribution <anthropogenic_hazards/distribution/episode-elements/LGF>;
. 
	<anthropogenic_hazards/dataset/episode/MONTEYNARD> a dcat:Dataset;
		dct:title "MONTEYNARD: water reservoir";
		dct:identifier "anthropogenic_hazards/dataset/episode/MONTEYNARD";
		adms:identifier [ a adms:Identifier;
			adms:schemaAgency "DDSS-ID";
			skos:notation "WP14-DDSS-011";
		]; 
		adms:identifier [ a adms:Identifier;
      adms:schemaAgency "DOI";
      skos:notation "10.25171/InstGeoph_PAS_ISEPOS-2018-003";
    ];
    dct:description "The episode describes the seismicity sequence around Monteynard dam, caused by reservoir impoundment in France. The seismic sequence, April 1962, M=5.5, April 1963, M=4.9, November 1979, M=4.5 is located is the near field of the reservoir, i.e. within 1-3 reservoir lake length. Monteynard reservoir situated in moderate seismic zone of western Alps. Initially within first few years, six earthquakes (ML higher than 3.5) occurred in quick succession in close vicinity of the reservoir (less than 15 km) thereby supporting the hypothesis of reservoir induced earthquakes at Monteynard. The first significant earthquake (M5.2) occurred near the reservoir when the reservoir was only one third full (40 m deep). The two other earthquakes (ML bigger than 4.5) in 1963 and 1979 occurred when the reservoir level peaked to its maximum value (115 m). The episode data correspond to (i) seismicity catalogues (1962,2009) around the reservoir up to a 10L distance to reservoir (L being the reservoir lake length). The users can select catalogue for seismicity either in 1L or 3L or 10L distance to lake reservoir; (ii) Yearly values for reservoir lake level are provided on the 1961-1992 period as mean, maximum and minimum values; monthly values being only available on the 1961-1964 period. Episode integrated in the framework of: EPOS IP project, European Plate Observing System Implementation Phase. This project has received funding from the European Union’s Horizon 2020 research and innovation programme under grant agreement No 676564. How to cite: IS EPOS (2018), Episode: MONTEYNARD, https://tcs.ah-epos.eu/#episode:MONTEYNARD, doi:10.25171/InstGeoph_PAS_ISEPOS-2018-003.";
		dct:created "2018-07-24"^^xsd:date;
		dct:modified "2018-07-24"^^xsd:date;
		dct:issued "2018-07-24"^^xsd:date;
		dct:temporal [ a dct:PeriodOfTime; 
			schema:startDate "1962-04-12T00:00:00Z"^^xsd:dateTime; 
			schema:endDate "2009-12-29T00:00:00Z"^^xsd:dateTime; 
		];
		dct:spatial [ a dct:Location;
	        locn:geometry "POINT(5.67766 44.90027)"^^gsp:wktLiteral;
	    ];
		dcat:theme <epos:Reservoirimpoundment>;
		dcat:keyword "anthropogenic hazards","TCS AH","IS-EPOS platform", "episode", "reservoir impoundment", "anthropogenic seismicity", "catalogue", "water level", "reservoir industrial data";
		dct:publisher <https://isterre.fr>;
		dcat:contactPoint <http://orcid.org/0000-0002-9580-7864/contactPoint>;
		dcat:contactPoint <mailto:abror.karimov@univ-grenoble-alpes.fr/contactPoint>;
		dcat:distribution <anthropogenic_hazards/distribution/episode-elements/MONTEYNARD>;
. 
	<anthropogenic_hazards/dataset/episode/SSFS1993> a dcat:Dataset;
		dct:title "1993 Soultz-sous-Forêts Stimulation";
		dct:identifier "anthropogenic_hazards/dataset/episode/SSFS1993";
		adms:identifier [ a adms:Identifier;
			adms:schemaAgency "DDSS-ID";
			skos:notation "WP14-DDSS-012";
		]; 
		adms:identifier [ a adms:Identifier;
      adms:schemaAgency "DOI";
      skos:notation "10.25577/SSFS1993";
    ];
    dct:description "In 1993, during the development of the european enhanced geothermal system field of Soultz-sous-Forêts (Alsace), 44000 m3 of water have been injected to create the reservoir by stimulating the natural fracture system of the granitic rock mass. Some 16000 microseismic events have been recorded by a network consisting of a hydrophone and 3 four-component accelerometers, cemented in the granite at the bottom of observation wells. Episode integrated in the framework of: EPOS IP project, European Plate Observing System Implementation Phase. This project has received funding from the European Union’s Horizon 2020 research and innovation programme under grant agreement No 676564. How to cite: EOST & GEIE EMC. (2017). Episode: 1993 stimulation Soultz-sous-Forêts [Collection]. EOST - CDGP. https://doi.org/10.25577/SSFS1993";
		dct:created "2018-09-28"^^xsd:date;
		dct:modified "2019-08-06"^^xsd:date;
		dct:issued "2018-09-28"^^xsd:date;
		dct:temporal [ a dct:PeriodOfTime; 
			schema:startDate "1993-09-01T00:00:00Z"^^xsd:dateTime;
			schema:endDate "1993-10-25T00:00:00Z"^^xsd:dateTime;
		];
		dct:spatial [ a dct:Location;
	        locn:geometry "POLYGON((7.86 48.93, 7.86 48.94, 7.87 48.94, 7.87 48.93, 7.86 48.93))"^^gsp:wktLiteral;
	    ];
		dcat:theme <epos:Geothermalenergyproduction>;
		dcat:keyword "anthropogenic hazards","TCS AH","IS-EPOS platform", "episode", "geothermal energy production", "anthropogenic seismicity", "catalogue", "seismic waveform", "station information", "injection industrial data", "velocity model";
		dct:publisher <https://eost.unistra.fr>;
		dcat:contactPoint <http://orcid.org/0000-0003-4017-4673/contactPoint>;
		dcat:distribution <anthropogenic_hazards/distribution/episode-elements/SSFS1993>;
. 
	<anthropogenic_hazards/dataset/episode/SSFS2000> a dcat:Dataset;
		dct:title "2000 Soultz-sous-Forêts Stimulation";
		dct:identifier "anthropogenic_hazards/dataset/episode/SSFS2000";
		adms:identifier [ a adms:Identifier;
			adms:schemaAgency "DDSS-ID";
			skos:notation "WP14-DDSS-013";
		]; 
		adms:identifier [ a adms:Identifier;
      adms:schemaAgency "DOI";
      skos:notation "10.25577/SSFS2000";
    ];
    dct:description "During June/July 2000 a hydraulic stimulation program was conducted in the well GPK2. The stimulation was performed over the open hole section of GPK2 from 4431 m (measured depth) to the bottom of the well at around 5084 m. A total of 27 800 m3 of water were injected. At the start of the stimulation 700m3 of brine were injected in an effort to encourage downward growth of the stimulated region. The stimulation covered a period of six days. After a break of seven days a post-stimulation injection test was performed. Microseismic emissions have been monitored and recorded throughout the experiment and continued for a further 11 days after the injection test. Episode integrated in the framework of: EPOS IP project, European Plate Observing System Implementation Phase. This project has received funding from the European Union’s Horizon 2020 research and innovation programme under grant agreement No 676564. How to cite: EOST & GEIE EMC. (2018). Episode: 2000 stimulation Soultz-sous-Forêts [Collection]. EOST - CDGP. https://doi.org/10.25577/SSFS2000";
		dct:created "2019-03-26"^^xsd:date;
		dct:modified "2019-03-26"^^xsd:date;
		dct:issued "2019-03-26"^^xsd:date;
		dct:temporal [ a dct:PeriodOfTime; 
			schema:startDate "2000-06-28T22:00:00Z"^^xsd:dateTime;
			schema:endDate "2000-07-16T22:00:00Z"^^xsd:dateTime;
		];
		dct:spatial [ a dct:Location;
	        locn:geometry "POLYGON((7.86 48.93, 7.86 48.94, 7.87 48.94, 7.87 48.93, 7.86 48.93))"^^gsp:wktLiteral;
	    ];
		dcat:theme <epos:Geothermalenergyproduction>;
		dcat:keyword "anthropogenic hazards","TCS AH","IS-EPOS platform", "episode", "geothermal energy production", "anthropogenic seismicity", "catalogue", "station information", "injection industrial data";
		dct:publisher <https://eost.unistra.fr>;
		dcat:contactPoint <http://orcid.org/0000-0003-4017-4673/contactPoint>;
		dcat:distribution <anthropogenic_hazards/distribution/episode-elements/SSFS2000>;
. 
	<anthropogenic_hazards/dataset/episode/SSFS2003> a dcat:Dataset;
		dct:title "2003 Soultz-sous-Forêts Stimulation";
		dct:identifier "anthropogenic_hazards/dataset/episode/SSFS2003";
		adms:identifier [ a adms:Identifier;
			adms:schemaAgency "DDSS-ID";
			skos:notation "WP14-DDSS-014";
		]; 
		adms:identifier [ a adms:Identifier;
      adms:schemaAgency "DOI";
      skos:notation "10.25577/SSFS2003";
    ];
    dct:description "The stimulation was performed in 2003 mainly by massive injection into the well GPK3. The stimulation strategy can be divided in five parts: - Injection into GPK3 - Injection into both GPK2 and GPK3 (“dual” or “focused” stimulation, Baria et al., 2004) - Shut in GPK2 - Shut in both GPK2 and GPK3 and production from GPK2 - Circulation test GPK2-GPK3 following stimulation. Episode integrated in the framework of: EPOS IP project, European Plate Observing System Implementation Phase. This project has received funding from the European Union’s Horizon 2020 research and innovation programme under grant agreement No 676564. How to cite: EOST, & GEIE EMC. (2018). Episode: 2003 stimulation Soultz-sous-Forêts [Collection]. EOST - CDGP. https://doi.org/10.25577/SSFS2003";
		dct:created "2019-04-08"^^xsd:date;
		dct:modified "2019-08-06"^^xsd:date;
		dct:issued "2019-04-08"^^xsd:date;
		dct:temporal [ a dct:PeriodOfTime; 
			schema:startDate "2003-01-22T23:00:00Z"^^xsd:dateTime;
			schema:endDate "2003-03-19T23:00:00Z"^^xsd:dateTime;
		];
		dct:spatial [ a dct:Location;
	        locn:geometry "POLYGON((7.86 48.93, 7.86 48.94, 7.87 48.94, 7.87 48.93, 7.86 48.93))"^^gsp:wktLiteral;
	    ];
		dcat:theme <epos:Geothermalenergyproduction>;
		dcat:keyword "anthropogenic hazards","TCS AH","IS-EPOS platform", "episode", "geothermal energy production", "anthropogenic seismicity", "catalogue", "station information", "injection industrial data";
		dct:publisher <https://eost.unistra.fr>;
		dcat:contactPoint <http://orcid.org/0000-0003-4017-4673/contactPoint>;
		dcat:distribution <anthropogenic_hazards/distribution/episode-elements/SSFS2003>;
. 
	<anthropogenic_hazards/dataset/episode/SSFS2004> a dcat:Dataset;
		dct:title "2004 Soultz-sous-Forêts Stimulation";
		dct:identifier "anthropogenic_hazards/dataset/episode/SSFS2004";
		adms:identifier [ a adms:Identifier;
			adms:schemaAgency "DDSS-ID";
			skos:notation "WP14-DDSS-046";
		]; 
		adms:identifier [ a adms:Identifier;
      adms:schemaAgency "DOI";
      skos:notation "10.25577/SSFS2004";
    ];
    dct:description "The 2004 stimulation was aimed at improving the hydraulic performances of the well GPK4. This borehole was stimulated twice. The present test corresponds to the first stimulation of GPK4. The data from a pre-stimulation low flow injection test performed to evaluate the initial injectivity of GPK4 are included. Episode integrated in the framework of: EPOS IP project, European Plate Observing System Implementation Phase. This project has received funding from the European Union’s Horizon 2020 research and innovation programme under grant agreement No 676564. How to cite: EOST & GEIE EMC. (2018). Episode: 2004 stimulation Soultz-sous-Forêts [Collection]. EOST - CDGP. https://doi.org/10.25577/SSFS2004";
		dct:created "2019-08-07"^^xsd:date;
		dct:modified "2019-08-07"^^xsd:date;
		dct:issued "2019-08-07"^^xsd:date;
		dct:temporal [ a dct:PeriodOfTime; 
			schema:startDate "2004-09-06T22:00:00Z"^^xsd:dateTime;
			schema:endDate "2004-10-01T22:00:00Z"^^xsd:dateTime;
		];
		dct:spatial [ a dct:Location;
	        locn:geometry "POINT(7.86 48.93)"^^gsp:wktLiteral;
	    ];
		dcat:theme <epos:Geothermalenergyproduction>;
		dcat:keyword "anthropogenic hazards","TCS AH","IS-EPOS platform", "episode", "geothermal energy production", "anthropogenic seismicity", "catalogue", "station information", "injection industrial data";
		dct:publisher <https://eost.unistra.fr>;
		dcat:contactPoint <http://orcid.org/0000-0003-4017-4673/contactPoint>;
		dcat:distribution <anthropogenic_hazards/distribution/episode-elements/SSFS2004>;
. 
	<anthropogenic_hazards/dataset/episode/SSFS2005> a dcat:Dataset;
		dct:title "2005 Soultz-sous-Forêts Stimulation";
		dct:identifier "anthropogenic_hazards/dataset/episode/SSFS2005";
		adms:identifier [ a adms:Identifier;
			adms:schemaAgency "DDSS-ID";
			skos:notation "WP14-DDSS-047";
		]; 
		adms:identifier [ a adms:Identifier;
      adms:schemaAgency "DOI";
      skos:notation "10.25577/SSFS2005";
    ];
    dct:description "The 2005 stimulation is the second stimulation of GPK4, after the previous one, performed in September 2004. The stimulation was followed a few days later by a program of chemical stimulation (injection of diluted HCl). This program involved the chemical stimulation itself and two identical step-rate injection tests: the first was performed before the chemical stimulation and the second after, in order to observe the efficiency of the chemical stimulation. The program was in the following order: - Second hydraulic stimulation of GPK4, - First step-rate test, - Chemical stimulation of GPK4 with HCl, - Second step-rate test. Episode integrated in the framework of: EPOS IP project, European Plate Observing System Implementation Phase. This project has received funding from the European Union’s Horizon 2020 research and innovation programme under grant agreement No 676564. How to cite: EOST, & GEIE EMC. (2018). Episode: 2005 stimulation Soultz-sous-Forêts [Data set]. EOST - CDGP";
		dct:created "2019-08-07"^^xsd:date;
		dct:modified "2019-08-07"^^xsd:date;
		dct:issued "2019-08-07"^^xsd:date;
		dct:temporal [ a dct:PeriodOfTime; 
			schema:startDate "2005-02-03T23:00:00Z"^^xsd:dateTime;
			schema:endDate "2005-04-02T23:00:00Z"^^xsd:dateTime;
		];
		dct:spatial [ a dct:Location;
	        locn:geometry "POINT(7.86 48.93)"^^gsp:wktLiteral;
	    ];
		dcat:theme <epos:Geothermalenergyproduction>;
		dcat:keyword "anthropogenic hazards","TCS AH","IS-EPOS platform", "episode", "geothermal energy production", "anthropogenic seismicity", "catalogue", "station information", "injection industrial data";
		dct:publisher <https://eost.unistra.fr>;
		dcat:contactPoint <http://orcid.org/0000-0003-4017-4673/contactPoint>;
		dcat:distribution <anthropogenic_hazards/distribution/episode-elements/SSFS2005>;
. 
	<anthropogenic_hazards/dataset/episode/GISOS-CERVILLE> a dcat:Dataset;
		dct:title "GISOS-CERVILLE: underground solution mining";
		dct:identifier "anthropogenic_hazards/dataset/episode/GISOS-CERVILLE";
		adms:identifier [ a adms:Identifier;
			adms:schemaAgency "DDSS-ID";
			skos:notation "WP14-DDSS-015";
		]; 
		adms:identifier [ a adms:Identifier;
      adms:schemaAgency "DOI";
      skos:notation "10.25171/InstGeoph_PAS_ISEPOS-2017-013";
    ];
    dct:description "Ground failures, caving processes and collapses of large natural or man-made underground cavities can produce significant socio-economic damages and represent a serious risk envisaged by the stakeholders and municipalities. In order to improve our understanding of the mechanisms governing such a geohazard and to test the potential of geophysical methods to prevent them, the development and collapse of a salt solution mining cavity (channel and drilling exploitation technique) was monitored. This experiment was conducted by the research “Groupement d’Intérêt Scientifique sur l’impact et la Sécurité des Ouvrages Souterrains” (GISOS), at the SOLVAY exploitation site of Cerville-Buissoncourt (Lorraine basin, France). During the experiment, an important seismic catalogue (ten thousands of events) was recorded by a local high frequency microseismic network, installed by INERIS, which provides a unique opportunity to study in detail the microseismic response of a caving and collapsing underground cavity. In addition, several geotechnical measurements such as GPS, extensometer have been perfomed to measure local insitu deformation and to visualize the evolving cavity structure from sonar campaign.  Episode integrated in the framework of: EPOS IP project, European Plate Observing System Implementation Phase. This project has received funding from the European Union’s Horizon 2020 research and innovation programme under grant agreement No 676564.  How to cite: IS EPOS (2017), Episode: GISOS-CERVILLE, https://tcs.ah-epos.eu/#episode:GISOS-CERVILLE, doi:10.25171/InstGeoph_PAS_ISEPOS-2017-013";
		dct:created "2017-08-03"^^xsd:date;
		dct:modified "2019-08-06"^^xsd:date;
		dct:issued "2017-08-03"^^xsd:date;
		dct:temporal [ a dct:PeriodOfTime; 
			schema:startDate "2008-03-06T00:00:00Z"^^xsd:dateTime; 
			schema:endDate "2009-02-12T00:00:00Z"^^xsd:dateTime; 
		];
		dct:spatial [ a dct:Location;
	        locn:geometry "POINT(6.321185 48.676043)"^^gsp:wktLiteral;
	    ];
		dcat:theme <epos:Saltsolutionsmining>;
		dcat:keyword "anthropogenic hazards","TCS AH","IS-EPOS platform", "episode", "underground mining", "anthropogenic seismicity", "catalogue", "seismic waveform", "station information", "water level", "ground water", "mine industrial data", "deformation", "velocity model";
		dct:publisher <http://www.ineris.fr>;
		dcat:contactPoint <mailto:jannes-l.kinscher@ineris.fr/contactPoint>;
		dcat:distribution <anthropogenic_hazards/distribution/episode-elements/GISOS-CERVILLE>;
. 
	<anthropogenic_hazards/dataset/episode/STARFISH> a dcat:Dataset;
		dct:title "STARFISH: underground gas storage";
		dct:identifier "anthropogenic_hazards/dataset/episode/STARFISH";
		adms:identifier [ a adms:Identifier;
			adms:schemaAgency "DDSS-ID";
			skos:notation "WP14-DDSS-016";
		]; 
		adms:identifier [ a adms:Identifier;
      adms:schemaAgency "DOI";
      skos:notation "10.25171/InstGeoph_PAS_ISEPOS-2017-014";
    ];
    dct:description "An experiment was undertaken in an underground salt mine to assess the influence of thermal loading of high-frequency gas storage operations cycles on the stability of salt cavities. A footwall salt block was exposed to repetitive rapid cooling cycles while its thermo-mechanical and acoustic response was recorded by multi-parameter geotechnical monitoring approach performed by different project partners (SMRI, BGR, Ecole de mines Paris). The cooling system allowed cooling with maximum temperature drops of 25 °C. Data of this episode was recorded by a multi parameter monitoring system set up by INERIS, comprising 16 high-resolution acoustic sensors, thermal sensors as well as strain cells, at different depths. Results of data analysis indicate that the nature of the first cooling cycle seems to be a crucial factor for the following mechanical behavior of salt rocks to successive cooling cycles.  Episode integrated in the framework of: EPOS IP project, European Plate Observing System Implementation Phase. This project has received funding from the European Union’s Horizon 2020 research and innovation programme under grant agreement No 676564.  How to cite: IS EPOS (2017), Episode: STARFISH, https://tcs.ah-epos.eu/#episode:STARFISH, doi:10.25171/InstGeoph_PAS_ISEPOS-2017-014";
		dct:created "2017-08-04"^^xsd:date;
		dct:modified "2019-08-06"^^xsd:date;
		dct:issued "2017-08-04"^^xsd:date;
		dct:temporal [ a dct:PeriodOfTime; 
			schema:startDate "2014-04-09T00:00:00Z"^^xsd:dateTime; 
			schema:endDate "2015-02-25T00:00:00Z"^^xsd:dateTime; 
		];
		dct:spatial [ a dct:Location;
	        locn:geometry "POINT(6.30884 48.63829)"^^gsp:wktLiteral;
	    ];
		dcat:theme <epos:Unconventionalhydrocarbonextraction>;
		dcat:keyword "anthropogenic hazards","TCS AH","IS-EPOS platform", "episode", "underground gas storage", "anthropogenic seismicity", "catalogue", "station information", "temperature", "strainmeter";
		dct:publisher <http://www.ineris.fr>;
		dcat:contactPoint <mailto:jannes-l.kinscher@ineris.fr/contactPoint>;
		dcat:distribution <anthropogenic_hazards/distribution/episode-elements/STARFISH>;
. 
	<anthropogenic_hazards/dataset/episode/THE_GEYSERS_Prati_9_and_Prati_29_cluster> a dcat:Dataset;
		dct:title "THE GEYSERS Prati 9 and Prati 29 cluster: Treated wastewater injection for geothermal power production";
		dct:identifier "anthropogenic_hazards/dataset/episode/THE_GEYSERS_Prati_9_and_Prati_29_cluster";
		adms:identifier [ a adms:Identifier;
			adms:schemaAgency "DDSS-ID";
			skos:notation "WP14-DDSS-017";
		]; 
		adms:identifier [ a adms:Identifier;
      adms:schemaAgency "DOI";
      skos:notation "10.25171/InstGeoph_PAS_ISEPOS-2017-011";
    ];
    dct:description "The Geysers is the world's largest geothermal (hydrothermal) field located 116km north of San Francisco, California. The injection of treated wastewater leads to occurrence of significant seismic activity with thousands of earthquakes above the magnitude of completeness of 1.4 occurring every year. This episode contains high quality seismic catalogs and other associated data from a cluster of seismicity related to fluid injection in the vicinity of Prati 9 and Prati 29 injection wells located in the north-western part of the field. The first catalog contains source parameters (including high quality static stress drop) estimated using mesh spectral ratio technique. The second catalog contains refined focal mechanism derived using HASH software. The catalog data are accompanied by technological data (injection rates) as well as supplementary information (well traces).  Episode integrated in the framework of: EPOS IP project, European Plate Observing System Implementation Phase. This project has received funding from the European Union’s Horizon 2020 research and innovation programme under grant agreement No 676564.  How to cite: • Kwiatek, Grzegorz and Martinez-Garzon, Patricia and Dresen, Georg and Bohnhoff, Marco and Sone, Hiroki and Hartline, Craig (2015) Effects of long-term fluid injection on induced seismicity parameters and maximum magnitude in northwestern part of The Geysers geothermal field. Journal of Geophysical Research: Solid Earth, 120 (10). pp. 7085-7101. DOI: 10.1002/2015JB012362 • Martinez-Garzon, Patricia and Kwiatek, Grzegorz and Sone, Hiroki and Bohnhoff, Marco and Dresen, Georg and Hartline, Craig (2014) Spatiotemporal changes, faulting regimes, and source parameters of induced seismicity: A case study from The Geysers geothermal field. Journal of Geophysical Research: Solid Earth, 119 (11). pp. 8378-8396. DOI: 10.1002/2014JB011385 • IS EPOS (2017), Episode: THE GEYSERS Prati 9 and Prati 29 cluster, https://tcs.ah-epos.eu/#episode:THE_GEYSERS_Prati_9_and_Prati_29_cluster, doi:10.25171/InstGeoph_PAS_ISEPOS-2017-011";
		dct:created "2017-06-26"^^xsd:date;
		dct:modified "2018-05-07"^^xsd:date;
		dct:issued "2017-06-26"^^xsd:date;
		dct:temporal [ a dct:PeriodOfTime; 
			schema:startDate "2007-12-10T00:00:00Z"^^xsd:dateTime; 
			schema:endDate "2014-08-23T00:00:00Z"^^xsd:dateTime; 
		];
		dct:spatial [ a dct:Location;
	        locn:geometry "POINT(-122.8278 38.8404)"^^gsp:wktLiteral;
	    ];
		dcat:theme <epos:Geothermalenergyproduction>;
		dcat:keyword "anthropogenic hazards","TCS AH","IS-EPOS platform", "episode", "geothermal energy production", "anthropogenic seismicity", "catalogue", "injection industrial data";
		dct:publisher <PIC:999994341>;
		dcat:contactPoint <http://orcid.org/0000-0003-1076-615X/contactPoint>;
		dcat:contactPoint <mailto:a_blanke@gfz-potsdam.de/contactPoint>;
		dcat:distribution <anthropogenic_hazards/distribution/episode-elements/THE_GEYSERS_Prati_9_and_Prati_29_cluster>;
. 
	<anthropogenic_hazards/dataset/episode/THE_GEYSERS> a dcat:Dataset;
		dct:title "THE GEYSERS: geothermal energy production";
		dct:identifier "anthropogenic_hazards/dataset/episode/THE_GEYSERS";
		adms:identifier [ a adms:Identifier;
			adms:schemaAgency "DDSS-ID";
			skos:notation "WP14-DDSS-018";
		]; 
		adms:identifier [ a adms:Identifier;
      adms:schemaAgency "DOI";
      skos:notation "10.25171/InstGeoph_PAS_ISEPOS-2018-001";
    ];
    dct:description "The Geysers geothermal field is one of the largest geothermal fields worldwide in terms of steam production. The Geysers is a vapor-dominated reservoir, located 116km north of San Francisco, California. It has been in operation for more than 50 years resulting in the occurrence of several hundred thousand induced seismic events. Over the years, field exploitation resulted in a long-term reduction of reservoir pressure and a decrease in steam production. Episode consists of the various data describing the seismicity connected with fluid injection at this geothermal site. The seismicity data are accompanied by technological data (injection volumes, steam production) as well as supplementary information (well positions and location of power plants). Episode integrated in the framework of: SHEER project, SHale gas Exploration and Exploitation induced Risks project has received funding from the European Union's Horizon 2020 research and innovation programme under grant agreement No 640896. How to cite: IS EPOS (2018), Episode: THE GEYSERS, https://tcs.ah-epos.eu/#episode:THE_GEYSERS, doi:10.25171/InstGeoph_PAS_ISEPOS-2018-001";
		dct:created "2018-04-20"^^xsd:date;
		dct:modified "2019-08-06"^^xsd:date;
		dct:issued "2018-04-20"^^xsd:date;
		dct:temporal [ a dct:PeriodOfTime; 
			schema:startDate "1970-04-01T00:00:00Z"^^xsd:dateTime; 
			schema:endDate "2011-10-31T00:00:00Z"^^xsd:dateTime; 
		];
		dct:spatial [ a dct:Location;
	        locn:geometry "POINT(-122.83268669938 38.798401622883)"^^gsp:wktLiteral;
	    ];
		dcat:theme <epos:Geothermalenergyproduction>;
		dcat:keyword "anthropogenic hazards","TCS AH","IS-EPOS platform", "episode", "geothermal energy production", "anthropogenic seismicity", "catalogue", "seismic waveform", "station information", "injection industrial data", "geothermal industrial data", "fault";
		dct:publisher <PIC:999527286>;
		dcat:contactPoint <https://orcid.org/0000-0001-8078-9416/contactPoint>;
		dcat:distribution <anthropogenic_hazards/distribution/episode-elements/THE_GEYSERS>;
. 
	<anthropogenic_hazards/dataset/episode/VDF> a dcat:Dataset;
		dct:title "VAL D'AGRI FIELD: conventional hydrocarbon extraction";
		dct:identifier "anthropogenic_hazards/dataset/episode/VDF";
		adms:identifier [ a adms:Identifier;
			adms:schemaAgency "DDSS-ID";
			skos:notation "WP14-DDSS-019";
		]; 
		adms:identifier [ a adms:Identifier;
      adms:schemaAgency "DOI";
      skos:notation "10.25171/InstGeoph_PAS_ISEPOS-2017-017";
    ];
    dct:description "Seismic monitoring of the initial stage of wastewater injection into a disposal well of the Val d'Agri oil field. The monitoring unraveled a low magnitude swarm induced by disposal operations that initiated just a few hours after the beginning of injection. Main objective is to provide seismic data to be analyzed with advanced techniques for a better understanding of the mechanisms of injection-linked seismicity and of physical properties of the reservoir.  Episode integrated in the framework of: EPOS IP project, European Plate Observing System Implementation Phase. This project has received funding from the European Union’s Horizon 2020 research and innovation programme under grant agreement No 676564.  How to cite: IS EPOS (2017), Episode: VDF, https://tcs.ah-epos.eu/#episode:VDF, doi:10.25171/InstGeoph_PAS_ISEPOS-2017-017";
		dct:created "2017-09-12"^^xsd:date;
		dct:modified "2018-02-02"^^xsd:date;
		dct:issued "2017-08-03"^^xsd:date;
		dct:temporal [ a dct:PeriodOfTime; 
			schema:startDate "2006-06-01T00:00:00Z"^^xsd:dateTime; 
			schema:endDate "2006-06-12T00:00:00Z"^^xsd:dateTime; 
		];
		dct:spatial [ a dct:Location;
	        locn:geometry "POINT(15.989 40.324)"^^gsp:wktLiteral;
	    ];
		dcat:theme <epos:Conventionalhydrocarbonextraction>;
		dcat:keyword "anthropogenic hazards","TCS AH","IS-EPOS platform", "episode", "conventional hydrocarbon extraction", "wastewater injection", "anthropogenic seismicity", "catalogue", "seismic waveform", "station information", "injection industrial data", "velocity model";
		dct:publisher <PIC:999472675>;
		dcat:contactPoint <http://orcid.org/0000-0003-2915-1446/contactPoint>;
		dcat:contactPoint <http://orcid.org/0000-0003-3844-5059/contactPoint>;
		dcat:distribution <anthropogenic_hazards/distribution/episode-elements/VDF>;
. 
	<anthropogenic_hazards/dataset/episode/VD> a dcat:Dataset;
		dct:title "VAL D'AGRI: water reservoir";
		dct:identifier "anthropogenic_hazards/dataset/episode/VD";
		adms:identifier [ a adms:Identifier;
			adms:schemaAgency "DDSS-ID";
			skos:notation "WP14-DDSS-020";
		]; 
		adms:identifier [ a adms:Identifier;
      adms:schemaAgency "DOI";
      skos:notation "10.25171/InstGeoph_PAS_ISEPOS-2017-016";
    ];
    dct:description "Low magnitude earthquakes recorded by an experiment-specific temporary network deployed around the Pertusillo Lake impoundment. During the one-year survey the network recorded an intense microseismicity that appears correlated in time and space to severe seasonal oscillations of the artificial lake. Main objective is to provide seismic data to be analyzed for a better understanding of the mechanisms of protracted RIS and of physical properties of the carbonate rocks where seismicity occurs.  Episode integrated in the framework of: EPOS IP project, European Plate Observing System Implementation Phase. This project has received funding from the European Union’s Horizon 2020 research and innovation programme under grant agreement No 676564.  How to cite: IS EPOS (2017), Episode: VAL D'AGRI, https://tcs.ah-epos.eu/#episode:VD, doi:10.25171/InstGeoph_PAS_ISEPOS-2017-016";
		dct:created "2017-09-12"^^xsd:date;
		dct:modified "2018-02-02"^^xsd:date;
		dct:issued "2017-09-12"^^xsd:date;
		dct:temporal [ a dct:PeriodOfTime; 
			schema:startDate "2005-05-05T00:00:00Z"^^xsd:dateTime; 
			schema:endDate "2006-06-12T00:00:00Z"^^xsd:dateTime; 
		];
		dct:spatial [ a dct:Location;
	        locn:geometry "POINT(15.9180 40.2270)"^^gsp:wktLiteral;
	    ];
		dcat:theme <epos:Reservoirimpoundment>;
		dcat:keyword "anthropogenic hazards","TCS AH","IS-EPOS platform", "episode", "reservoir impoundment", "anthropogenic seismicity", "catalogue", "seismic waveform", "station information", "reservoir industrial data", "water level", "velocity model";
		dct:publisher <PIC:999472675>;
		dcat:contactPoint <http://orcid.org/0000-0003-2915-1446/contactPoint>;
		dcat:contactPoint <http://orcid.org/0000-0003-3844-5059/contactPoint>;
		dcat:distribution <anthropogenic_hazards/distribution/episode-elements/VD>;
. 
#	<anthropogenic_hazards/dataset/episode/EMILIA_ROMAGNA> a dcat:Dataset;
#		dct:title "EMILIA ROMAGNA: cavone oil field";
#		dct:identifier "anthropogenic_hazards/dataset/episode/EMILIA_ROMAGNA";
#		adms:identifier [ a adms:Identifier;
#			adms:schemaAgency "DDSS-ID";
#			skos:notation "WP14-DDSS-021";
#		]; 
#		adms:identifier [ a adms:Identifier;
#     adms:schemaAgency "DOI";
#     skos:notation "XXX";
#   ];
#   dct:description "Episode consists of the various data describing the seismicity caused by conventional hydrocarbon extraction and fluid injection in Emilia Romagna, Italy.	Episode integrated in the framework of: EPOS IP project, European Plate Observing System Implementation Phase. This project has received funding from the European Union’s Horizon 2020 research and innovation programme under grant agreement No 676564.";
#		dct:created "2019-03-08"^^xsd:date;
#		dct:modified "2019-03-08"^^xsd:date;
#		dct:issued "2019-03-08"^^xsd:date;
#		dct:temporal [ a dct:PeriodOfTime; 
#			schema:startDate "2005-05-01T12:00:00Z"^^xsd:dateTime; 
#			schema:endDate "2006-12-01T12:00:00Z"^^xsd:dateTime; 
#		];
#		dct:spatial [ a dct:Location;
#	        locn:geometry "POINT(11.48375 44.875)"^^gsp:wktLiteral;
#	    ];
#		dcat:theme <epos:Conventionalhydrocarbonextraction>;
#		dcat:keyword "anthropogenic hazards","TCS AH","IS-EPOS platform", "episode", "conventional hydrocarbon extraction", "anthropogenic seismicity", "catalogue", "hydrocarbon production data";
#		dct:publisher <PIC:999472675>;
#		dcat:contactPoint <http://orcid.org/0000-0001-9196-8452/contactPoint>;
#		dcat:distribution <anthropogenic_hazards/distribution/episode-elements/EMILIA_ROMAGNA>;
#. 
	<anthropogenic_hazards/dataset/episode/PREESE_HALL> a dcat:Dataset;
		dct:title "PREESE HALL: Shale Gas";
		dct:identifier "anthropogenic_hazards/dataset/episode/PREESE_HALL";
		adms:identifier [ a adms:Identifier;
			adms:schemaAgency "DDSS-ID";
			skos:notation "WP14-DDSS-022";
		]; 
		adms:identifier [ a adms:Identifier;
      adms:schemaAgency "DOI";
      skos:notation "10.25171/InstGeoph_PAS_ISEPOS-2017-010";
    ];
    dct:description "An exploration well for shale gas was drilled into the Bowland Shale formation to a depth of 2.7 km. Hydrofracture stimulations were carried out at five depths. Felt earthquakes occurred during the stage 2 treatment.  Episode integrated in the framework of: SHEER project, SHale gas Exploration and Exploitation induced Risks project has received funding from the European Union's Horizon 2020 research and innovation programme under grant agreement No 640896; EPOS IP project, European Plate Observing System Implementation Phase. This project has received funding from the European Union’s Horizon 2020 research and innovation programme under grant agreement No 676564.  How to cite: IS EPOS (2017), Episode: PREESE HALL, https://tcs.ah-epos.eu/#episode:PREESE_HALL, doi:10.25171/InstGeoph_PAS_ISEPOS-2017-010";
		dct:created "2016-05-15"^^xsd:date;
		dct:modified "2018-05-01"^^xsd:date;
		dct:issued "2016-05-15"^^xsd:date;
		dct:temporal [ a dct:PeriodOfTime; 
			schema:startDate "2011-03-26T00:00:00Z"^^xsd:dateTime; 
			schema:endDate "2011-11-23T00:00:00Z"^^xsd:dateTime; 
		];
		dct:spatial [ a dct:Location;
	        locn:geometry "POINT(-2.9442207 53.8219037)"^^gsp:wktLiteral;
	    ];
		dcat:theme <epos:Unconventionalhydrocarbonextraction>;
		dcat:keyword "anthropogenic hazards","TCS AH","IS-EPOS platform", "episode", "unconventional hydrocarbon extraction", "anthropogenic seismicity", "catalogue", "seismic waveform", "station information", "injection industrial data", "hydrocarbon production data", "velocity model";
		dct:publisher <PIC:999862324>;
		dcat:contactPoint <http://orcid.org/0000-0002-0769-5277/contactPoint>;
		dcat:distribution <anthropogenic_hazards/distribution/episode-elements/PREESE_HALL>;
. 
	<anthropogenic_hazards/dataset/episode/THORESBY_COLLIERY> a dcat:Dataset;
		dct:title "THORESBY COLLIERY: underground coal mining";
		dct:identifier "anthropogenic_hazards/dataset/episode/THORESBY_COLLIERY";
		adms:identifier [ a adms:Identifier;
			adms:schemaAgency "DDSS-ID";
			skos:notation "WP14-DDSS-023";
		]; 
		adms:identifier [ a adms:Identifier;
      adms:schemaAgency "DOI";
      skos:notation "10.25171/InstGeoph_PAS_ISEPOS-2018-011";
    ];
    dct:description "Situated in the North of the Nottinghamshire Coalfield, Thoresby Colliery closed in 2015 and was the last deep coal mine in England's East Midlands. Production at the mine lasted over 90 years with the extraction of Middle Coal Measure seams at depths between 650m to 820m below ground level. Sherwood Sandstone (containing fissures at the surface presumed to be associated with mining) overlie the Middle Coal Measures and form the surface rock in the Thoresby Colliery area. Workings of the colliery extend beneath Thoresby Park near Edwinstowe where over 100 felt tremors were reported by the public between June 1989 and August 1990 and have since been associated with induced seismicity from the longwall mining of coal in the area (Bishop et al., 1993 and Styles et al., 1997 – references in episode repository). This episode contains microseismic monitoring data caused by the underground mining of coal at Thoresby Colliery between late 1996 and early 1997. Episode integrated in the framework of: EPOS IP project, European Plate Observing System Implementation Phase. This project has received funding from the European Union’s Horizon 2020 research and innovation programme under grant agreement No 676564. How to cite: IS EPOS (2018), Episode: THORESBY COLLIERY, https://tcs.ah-epos.eu/#episode:THORESBY_COLLIERY, doi:10.25171/InstGeoph_PAS_ISEPOS-2018-011";
		dct:created "2019-05-06"^^xsd:date;
		dct:modified "2019-05-06"^^xsd:date;
		dct:issued "2019-05-06"^^xsd:date;
		dct:temporal [ a dct:PeriodOfTime; 
			schema:startDate "1996-08-31T12:00:00Z"^^xsd:dateTime; 
			schema:endDate "1997-03-11T12:00:00Z"^^xsd:dateTime; 
		];
		dct:spatial [ a dct:Location;
	        locn:geometry "POINT(-1.0511 52.20244)"^^gsp:wktLiteral;
	    ];
		dcat:theme <epos:Coalmining>;
		dcat:keyword "anthropogenic hazards","TCS AH","IS-EPOS platform", "episode", "underground mining", "anthropogenic seismicity", "catalogue", "seismic waveform", "station information", "mine industrial data", "velocity model";
		dct:publisher <PIC:999862324>;
		dcat:contactPoint <http://orcid.org/0000-0002-0769-5277/contactPoint>;
		dcat:distribution <anthropogenic_hazards/distribution/episode-elements/THORESBY_COLLIERY>;
. 
	<anthropogenic_hazards/dataset/episode/ASFORDBY> a dcat:Dataset;
		dct:title "ASFORDBY: underground coal mining";
		dct:identifier "anthropogenic_hazards/dataset/episode/ASFORDBY";
		adms:identifier [ a adms:Identifier;
			adms:schemaAgency "DDSS-ID";
			skos:notation "WP14-DDSS-024";
		]; 
		adms:identifier [ a adms:Identifier;
      adms:schemaAgency "DOI";
      skos:notation "10.25171/InstGeoph_PAS_ISEPOS-2018-008";
    ];
    dct:description "Asfordby mine (also referred to as the Asfordby Colliery or Asfordby Super-pit) is situated North East of the town of Melton Mowbray in the East Midlands County of Leicestershire, England. Coal Measures at Asfordby mine are part of the southerly extending South-East Nottinghamshire Carboniferous basin with the deep main seam occurring at depths of over 500m. Asfordby mine was the first and last modern deep mine to exploit the coalfield in the area. Coal production at the mine began in 1991 but was short lived with closure of the mine in 1997 following a damaging collapse at the mine and production issues linked to the geological complications of dolerite sills within the coal measures and from the overlying Sherwood sandstone aquifer. This episode contains geotechnical, industrial and microseismic monitoring data from an investigation conducted in 1995 during the longwall excavation of Panel 101 in the Deep Main seam at Asfordby Mine. The associated IMCL Ltd investigation report carried out to determine whether microseismic monitoring can detect and map fracturing and overburden failure from the longwall extraction of coal is also provided. Episode integrated in the framework of: EPOS IP project, European Plate Observing System Implementation Phase. This project has received funding from the European Union’s Horizon 2020 research and innovation programme under grant agreement No 676564. How to cite: IS EPOS (2018), Episode: ASFORDBY, https://tcs.ah-epos.eu/#episode:ASFORDBY, doi:10.25171/InstGeoph_PAS_ISEPOS-2018-008";
		dct:created "2019-05-17"^^xsd:date;
		dct:modified "2019-05-17"^^xsd:date;
		dct:issued "2019-05-17"^^xsd:date;
		dct:temporal [ a dct:PeriodOfTime; 
			schema:startDate "1995-04-10T12:00:00Z"^^xsd:dateTime; 
			schema:endDate "1996-01-21T12:00:00Z"^^xsd:dateTime; 
		];
		dct:spatial [ a dct:Location;
	        locn:geometry "POINT(-0.9279 52.77511)"^^gsp:wktLiteral;
	    ];
		dcat:theme <epos:Coalmining>;
		dcat:keyword "anthropogenic hazards","TCS AH","IS-EPOS platform", "episode", "underground mining", "anthropogenic seismicity", "catalogue", "seismic waveform", "station information", "mine industrial data", "geology", "fault", "velocity model";
		dct:publisher <PIC:999862324>;
		dcat:contactPoint <http://orcid.org/0000-0002-0769-5277/contactPoint>;
		dcat:distribution <anthropogenic_hazards/distribution/episode-elements/ASFORDBY>;
. 
	<anthropogenic_hazards/dataset/episode/NORTHWICH> a dcat:Dataset;
		dct:title "NORTHWICH: underground salt extraction cavities";
		dct:identifier "anthropogenic_hazards/dataset/episode/NORTHWICH";
		adms:identifier [ a adms:Identifier;
			adms:schemaAgency "DDSS-ID";
			skos:notation "WP14-DDSS-025";
		]; 
		adms:identifier [ a adms:Identifier;
      adms:schemaAgency "DOI";
      skos:notation "10.25171/InstGeoph_PAS_ISEPOS-2018-009";
    ];
    dct:description "Situated in Cheshire in the NW of England, Northwich overlies Triassic Halite beds that have been industrially and extensively mined for salt since the 17th century. As a result of poor early mining practices, combined with natural and anthropogenic salt dissolution, the area has suffered from mine void collapse and large scale catastrophic surface land subsidence. This episode contains long term microgravity data obtained for the detection and monitoring of voids, and time-lapse topography data for subsidence and ground deformation records. Both datasets are from a section of the Trent and Mersey Canal that has been severely affected by subsidence and the episode is supplemented with mine plans of the area along with details of a seismic network situated to the south of the monitored canal section. A 2012 paper detailing 10 years of monitoring + canal topography data is also available. Episode integrated in the framework of: EPOS IP project, European Plate Observing System Implementation Phase. This project has received funding from the European Union’s Horizon 2020 research and innovation programme under grant agreement No 676564. How to cite: IS EPOS (2018), Episode: NORTHWICH, https://tcs.ah-epos.eu/#episode:NORTHWICH, doi:10.25171/InstGeoph_PAS_ISEPOS-2018-009";
		dct:created "2019-05-06"^^xsd:date;
		dct:modified "2019-05-06"^^xsd:date;
		dct:issued "2019-05-06"^^xsd:date;
		dct:temporal [ a dct:PeriodOfTime; 
			schema:startDate "2001-07-01T12:00:00Z"^^xsd:dateTime; 
			schema:endDate "2006-03-01T12:00:00Z"^^xsd:dateTime; 
		];
		dct:spatial [ a dct:Location;
	        locn:geometry "POINT(-2.50935 53.26354)"^^gsp:wktLiteral;
	    ];
		dcat:theme <epos:Saltsolutionsmining>;
		dcat:keyword "anthropogenic hazards","TCS AH","IS-EPOS platform", "episode", "underground mining", "anthropogenic seismicity", "seismic waveform", "station information", "mine industrial data", "gravity data", "deformation", "velocity model";
		dct:publisher <PIC:999862324>;
		dcat:contactPoint <http://orcid.org/0000-0002-0769-5277/contactPoint>;
		dcat:distribution <anthropogenic_hazards/distribution/episode-elements/NORTHWICH>;
. 
	<anthropogenic_hazards/dataset/episode/OK> a dcat:Dataset;
		dct:title "OKLAHOMA: conventional and unconventional hydrocarbon extraction and wastewater injection";
		dct:identifier "anthropogenic_hazards/dataset/episode/OK";
		adms:identifier [ a adms:Identifier;
			adms:schemaAgency "DDSS-ID";
			skos:notation "WP14-DDSS-027";
		]; 
		adms:identifier [ a adms:Identifier;
      adms:schemaAgency "DOI";
      skos:notation "10.25171/InstGeoph_PAS_ISEPOS-2018-002";
    ];
    dct:description "In recent years the seismicity rate and magnitude of seismicity in Oklahoma has increased. It has been found that this is due to the injection of fluids for both conventional and unconvential hydrocarbon exploitation as well as waste water injection. Episode integrated in the framework of: SHEER project, SHale gas Exploration and Exploitation induced Risks project has received funding from the European Union's Horizon 2020 research and innovation programme under grant agreement No 640896; EPOS IP project, European Plate Observing System Implementation Phase. This project has received funding from the European Union’s Horizon 2020 research and innovation programme under grant agreement No 676564. How to cite: IS EPOS (2018), Episode: OKLAHOMA, https://tcs.ah-epos.eu/#episode:OK, doi:10.25171/InstGeoph_PAS_ISEPOS-2018-002";
		dct:created "2018-04-17"^^xsd:date;
		dct:modified "2018-05-01"^^xsd:date;
		dct:issued "2018-04-17"^^xsd:date;
		dct:temporal [ a dct:PeriodOfTime; 
			schema:startDate "2010-01-01T00:00:00Z"^^xsd:dateTime; 
			schema:endDate "2016-12-31T00:00:00Z"^^xsd:dateTime; 
		];
		dct:spatial [ a dct:Location;
	        locn:geometry "POINT(-97.34 36.03)"^^gsp:wktLiteral;
	    ];
		dcat:theme <epos:Unconventionalhydrocarbonextraction>;
		dcat:theme <epos:Conventionalhydrocarbonextraction>;
		dcat:keyword "anthropogenic hazards","TCS AH","IS-EPOS platform", "episode", "conventional hydrocarbon extraction", "unconventional hydrocarbon extraction", "wastewater injection", "anthropogenic seismicity", "catalogue", "seismic waveform", "station information", "injection industrial data", "hydrocarbon production data", "fault";
		dct:publisher <PIC:999862324>;
		dcat:contactPoint <http://orcid.org/0000-0002-0769-5277/contactPoint>;
		dcat:distribution <anthropogenic_hazards/distribution/episode-elements/OK>;
. 
	<anthropogenic_hazards/dataset/episode/PREESALL_MINE> a dcat:Dataset;
		dct:title "PREESALL MINE: underground salt extraction cavities";
		dct:identifier "anthropogenic_hazards/dataset/episode/PREESALL_MINE";
		adms:identifier [ a adms:Identifier;
			adms:schemaAgency "DDSS-ID";
			skos:notation "WP14-DDSS-028";
		]; 
		adms:identifier [ a adms:Identifier;
      adms:schemaAgency "DOI";
      skos:notation "10.25171/InstGeoph_PAS_ISEPOS-2018-010";
    ];
    dct:description "Located in the NW of England in the county of Lancashire, the Preesall Salt field (also known as the Preesall Brine field) is one of the UK’s major onshore halite formations. The field contains thick beds of Triassic aged halite (Pressall Halite) which lie along the Fylde Coast (to the north of Blackpool and East of the river Wyre) and was once the site of the largest salt producer in Britain. Since the 1870’s the heavy exploitation of salt by dry mining and by brine extraction has left the Preesall area with dramatic subsidence damage including unstable cavities and several deep flashes following a number of major collapse events. This episode contains seismic data and time-lapse micro-gravity data collected from around a brine well over an unstable cavity situated South-west of the previous Preesall Salt Mine. Episode integrated in the framework of: EPOS IP project, European Plate Observing System Implementation Phase. This project has received funding from the European Union’s Horizon 2020 research and innovation programme under grant agreement No 676564. How to cite: IS EPOS (2018), Episode: PREESALL MINE, https://tcs.ah-epos.eu/#episode:PREESALL_MINE, doi:10.25171/InstGeoph_PAS_ISEPOS-2018-011";
		dct:created "2019-05-06"^^xsd:date;
		dct:modified "2019-05-06"^^xsd:date;
		dct:issued "2019-05-06"^^xsd:date;
		dct:temporal [ a dct:PeriodOfTime; 
			schema:startDate "2000-04-01T12:00:00Z"^^xsd:dateTime; 
			schema:endDate "2001-03-01T12:00:00Z"^^xsd:dateTime; 
		];
		dct:spatial [ a dct:Location;
	        locn:geometry "POINT(-2.97555 53.9028)"^^gsp:wktLiteral;
	    ];
		dcat:theme <epos:Saltsolutionsmining>;
		dcat:keyword "anthropogenic hazards","TCS AH","IS-EPOS platform", "episode", "underground mining", "anthropogenic seismicity", "catalogue", "seismic waveform", "station information", "mine industrial data", "gravity data";
		dct:publisher <PIC:999862324>;
		dcat:contactPoint <http://orcid.org/0000-0002-0769-5277/contactPoint>;
		dcat:distribution <anthropogenic_hazards/distribution/episode-elements/PREESALL_MINE>;
. 
	<anthropogenic_hazards/dataset/episode/GRONINGEN_FIELD> a dcat:Dataset;
		dct:title "GRONINGEN FIELD: conventional hydrocarbon production";
		dct:identifier "anthropogenic_hazards/dataset/episode/GRONINGEN_FIELD";
		adms:identifier [ a adms:Identifier;
			adms:schemaAgency "DDSS-ID";
			skos:notation "WP14-DDSS-029";
		]; 
		adms:identifier [ a adms:Identifier;
      adms:schemaAgency "DOI";
      skos:notation "10.25171/InstGeoph_PAS_ISEPOS-2017-008";
    ];
    dct:description "The Groningen gas field is a giant natural gas field located near Slochteren in Groningen province in the northeastern part of the Netherlands. Discovered in 1959, it is the largest natural gas field in Europe and the tenth-largest in the world. Episode integrated in the framework of: SHEER project, SHale gas Exploration and Exploitation induced Risks project has received funding from the European Union's Horizon 2020 research and innovation programme under grant agreement No 640896. How to cite: IS EPOS (2017), Episode: GRONINGEN FIELD, https://tcs.ah-epos.eu/#episode:GRONINGEN_FIELD, doi:10.25171/InstGeoph_PAS_ISEPOS-2017-008";
		dct:accrualPeriodicity "http://purl.org/cld/freq/quarterly"^^xsd:anyURI;
		dct:created "2016-05-15"^^xsd:date;
		dct:modified "2019-08-06"^^xsd:date;
		dct:issued "2016-05-15"^^xsd:date;
		dct:temporal [ a dct:PeriodOfTime; 
			schema:startDate "2001-06-01T00:00:00Z"^^xsd:dateTime;
			schema:endDate "2017-05-30T00:00:00Z"^^xsd:dateTime;
		];
		dct:spatial [ a dct:Location;
	        locn:geometry "POINT(6.707173 53.284546)"^^gsp:wktLiteral;
	    ];
		dcat:theme <epos:Conventionalhydrocarbonextraction>;
		dcat:keyword "anthropogenic hazards","TCS AH","IS-EPOS platform", "episode", "conventional hydrocarbon extraction", "anthropogenic seismicity", "catalogue", "seismic waveform", "ground motion parameters", "station information", "hydrocarbon production data";
		dct:publisher <PIC:999518944>;
		dcat:contactPoint <http://orcid.org/0000-0001-7153-5115/contactPoint>;
		dcat:distribution <anthropogenic_hazards/distribution/episode-elements/GRONINGEN_FIELD>;
. 
	<anthropogenic_hazards/dataset/episode/LAI_CHAU> a dcat:Dataset;
		dct:title "LAI CHAU: water reservoir";
		dct:identifier "anthropogenic_hazards/dataset/episode/LAI_CHAU";
		adms:identifier [ a adms:Identifier;
			adms:schemaAgency "DDSS-ID";
			skos:notation "WP14-DDSS-033";
		]; 
		adms:identifier [ a adms:Identifier;
      adms:schemaAgency "DOI";
      skos:notation "10.25171/InstGeoph_PAS_ISEPOS-2018-012";
    ];
    dct:description "Seismic activity linked to Lai Chau hydropower plant and the reservoir containing backed up water of Da river (Black river) in northwestern Vietnam. Construction started on 5 January 2011 and it is expected to be operational by 2017 with the first turbine put into operation in 2016. The area of the reservoir is considered as tectonically active with known earthquakes in the past. During the period from September 2014 to May 2015, network of seismological stations in broad Lai Chau region recorded nearly 40 earthquakes M 1.1 to 4.0. Three of them occurred directly in Lai Chau hydro reservoir area (October 19 and 31, 2014 M3.5 and November 26, 2014 M2.0). The reservoir filling started in June 2015. The water level varies between 205 and 280 m. a.s.l. During the period from October 2014 to October 2015, network of seismological stations in wide Lai Chau area recorded nearly 60 earthquakes with M1.0 to 4.0. Several of them were located a radius of 6-20 km from Lai Chau dam. How to cite: IS EPOS (2018), Episode: LAI CHAU, https://tcs.ah-epos.eu/#episode:LAI_CHAU, doi:10.25171/InstGeoph_PAS_ISEPOS-2018-012";
		dct:created "2019-02-21"^^xsd:date;
		dct:modified "2019-02-21"^^xsd:date;
		dct:issued "2019-02-21"^^xsd:date;
		dct:temporal [ a dct:PeriodOfTime; 
			schema:startDate "2014-10-06T21:06:06Z"^^xsd:dateTime;
		];
		dct:spatial [ a dct:Location;
	        locn:geometry "POINT(102.9875 22.139444)"^^gsp:wktLiteral;
	    ];
		dcat:theme <epos:Reservoirimpoundment>;
		dcat:keyword "anthropogenic hazards","TCS AH","IS-EPOS platform", "episode", "reservoir impoundment", "anthropogenic seismicity", "catalogue", "seismic waveform", "station information", "reservoir industrial data", "water level";
		dct:publisher <PIC:996625337>;
		dcat:contactPoint <http://orcid.org/0000-0002-4801-4888/contactPoint>;
		dcat:distribution <anthropogenic_hazards/distribution/episode-elements/LAI_CHAU>;
. 
	<anthropogenic_hazards/dataset/episode/LUBOCINO> a dcat:Dataset;
		dct:title "LUBOCINO: Shale Gas";
		dct:identifier "anthropogenic_hazards/dataset/episode/LUBOCINO";
		adms:identifier [ a adms:Identifier;
			adms:schemaAgency "DDSS-ID";
			skos:notation "WP14-DDSS-036";
		]; 
		adms:identifier [ a adms:Identifier;
      adms:schemaAgency "DOI";
      skos:notation "10.25171/InstGeoph_PAS_ISEPOS-2017-009";
    ];
    dct:description "Hydrofracturing is being conducted in Pomerania, Poland by PGNiG (Polish Oil and Gas Company). It is accompanied by a seismic monitoring, monitoring of air and water quality and ground deformation. With the participation of representatives of government and private industry, best practices to monitor and minimize the environmental impact of shale gas in Europe will be developed. Episode integrated in the framework of: SHEER project, SHale gas Exploration and Exploitation induced Risks project has received funding from the European Union's Horizon 2020 research and innovation programme under grant agreement No 640896. How to cite: IS EPOS (2017), Episode: LUBOCINO, https://tcs.ah-epos.eu/#episode:LUBOCINO, doi:10.25171/InstGeoph_PAS_ISEPOS-2017-009";
		dct:created "2016-07-10"^^xsd:date;
		dct:modified "2018-05-01"^^xsd:date;
		dct:issued "2016-07-10"^^xsd:date;
		dct:temporal [ a dct:PeriodOfTime; 
			schema:startDate "2011-06-20T00:00:00Z"^^xsd:dateTime;
			schema:endDate "2014-04-02T00:00:00Z"^^xsd:dateTime; 
		];
		dct:spatial [ a dct:Location;
	        locn:geometry "POINT(18.148734 54.72094)"^^gsp:wktLiteral;
	    ];
		dcat:theme <epos:Unconventionalhydrocarbonextraction>;
		dcat:keyword "anthropogenic hazards","TCS AH","IS-EPOS platform", "episode", "unconventional hydrocarbon extraction", "anthropogenic seismicity", "station information", "water quality data";
		dct:publisher <PIC:996625337>;
		dcat:contactPoint <http://orcid.org/0000-0002-4801-4888/contactPoint>;
		dcat:distribution <anthropogenic_hazards/distribution/episode-elements/LUBOCINO>;
. 
	<anthropogenic_hazards/dataset/episode/WYSIN> a dcat:Dataset;
		dct:title "WYSIN: Shale Gas";
		dct:identifier "anthropogenic_hazards/dataset/episode/WYSIN";
		adms:identifier [ a adms:Identifier;
			adms:schemaAgency "DDSS-ID";
			skos:notation "WP14-DDSS-037";
		]; 
		adms:identifier [ a adms:Identifier;
      adms:schemaAgency "DOI";
      skos:notation "10.25171/InstGeoph_PAS_ISEPOS-2017-012";
    ];
    dct:description "Monitoring the environmental impacts of shale gas exploration/exploitation at the site of one of the concessions of the Polish Oil and Gas SA company before, during and after termination of fracking operations. Detailed objectives are: • to establish background levels of seismicity, water condition and air pollution, • to sample the actual impact of fracking on the seismicity, water and air conditions in the direct vicinity and during fracking operations, • to recognize protracted effects of shale gas operations on the environment, • to provide observational data to be analyzed. Episode integrated in the framework of: SHEER project, SHale gas Exploration and Exploitation induced Risks project has received funding from the European Union's Horizon 2020 research and innovation programme under grant agreement No 640896. How to cite: IS EPOS (2017), Episode: WYSIN, https://tcs.ah-epos.eu/#episode:WYSIN, doi:10.25171/InstGeoph_PAS_ISEPOS-2017-012";
		dct:accrualPeriodicity "http://purl.org/cld/freq/quarterly"^^xsd:anyURI;
		dct:created "2016-05-15"^^xsd:date;
		dct:modified "2019-08-06"^^xsd:date;
		dct:issued "2016-05-15"^^xsd:date;
		dct:temporal [ a dct:PeriodOfTime; 
			schema:startDate "2015-06-09T00:00:00Z"^^xsd:dateTime;
			schema:endDate "2018-02-28T00:00:00Z"^^xsd:dateTime;
		];
		dct:spatial [ a dct:Location;
	        locn:geometry "POINT(18.3039 54.09417)"^^gsp:wktLiteral;
	    ];
		dcat:theme <epos:Unconventionalhydrocarbonextraction>;
		dcat:keyword "anthropogenic hazards","TCS AH","IS-EPOS platform", "episode", "unconventional hydrocarbon extraction", "anthropogenic seismicity", "seismic waveform", "station information", "air quality data", "radon concentration", "water quality data", "injection industrial data", "geology", "velocity model", "hydrocarbon production data";
		dct:publisher <PIC:996625337>;
		dcat:contactPoint <http://orcid.org/0000-0002-4801-4888/contactPoint>;
		dcat:distribution <anthropogenic_hazards/distribution/episode-elements/WYSIN>;
. 
	<anthropogenic_hazards/dataset/episode/CARBFIX> a dcat:Dataset;
		dct:title "CARBFIX: geothermal energy producion and CCS";
		dct:identifier "anthropogenic_hazards/dataset/episode/CARBFIX";
		adms:identifier [ a adms:Identifier;
			adms:schemaAgency "DDSS-ID";
			skos:notation "WP14-DDSS-038";
		]; 
		adms:identifier [ a adms:Identifier;
      adms:schemaAgency "DOI";
      skos:notation "10.25171/InstGeoph_PAS_ISEPOS-2018-006";
    ];
    dct:description "CarbFix is a CCS consortium operated by RE, UI, Columbia University (USA) and CNRS (France). It is one of the most successful and best-known examples of CO2 sequestration processes in the world. RE operates over 100 wells at Hellisheidi, about 10 of which are used for re-injection of geothermal water, one is used for re-injection of captured gases, the others are production and monitoring wells. Roughly one-third of the CO2 and H2S presently emitted from the Hellishidi power plant is being injected as a dissolved water phase into fractured basaltic rocks. CCS operations are followed by the seismic activity. Episode integrated in the framework of: S4CE, Science for Clean Energy. This project has received funding from the European Union’s Horizon 2020 research and innovation programme under grant agreement No 764810";
		dct:created "2018-05-08"^^xsd:date;
		dct:modified "2018-05-08"^^xsd:date;
		dct:issued "2018-05-08"^^xsd:date;
		dct:temporal [ a dct:PeriodOfTime; 
			schema:startDate "2017-11-29T00:00:00Z"^^xsd:dateTime;
			schema:endDate "2018-02-28T00:00:00Z"^^xsd:dateTime;
		];
		dct:spatial [ a dct:Location;
	        locn:geometry "POINT(-21.31484 64.05818)"^^gsp:wktLiteral;
	    ];
		dcat:theme <epos:Geothermalenergyproduction>;
		dcat:keyword "anthropogenic hazards","TCS AH","IS-EPOS platform", "episode", "geothermal energy production", "CO2 sequestration", "anthropogenic seismicity", "catalogue", "station information", "water level", "ground water", "injection industrial data", "geology";
		dct:publisher <PIC:974007459>;
		dcat:contactPoint <https://orcid.org/0000-0003-2989-1663/contactPoint>;
		dcat:distribution <anthropogenic_hazards/distribution/episode-elements/CARBFIX>;
. 
	<anthropogenic_hazards/dataset/episode/SG> a dcat:Dataset;
		dct:title "ST. GALLEN: geothermal project";
		dct:identifier "anthropogenic_hazards/dataset/episode/SG";
		adms:identifier [ a adms:Identifier;
			adms:schemaAgency "DDSS-ID";
			skos:notation "WP14-DDSS-039";
		]; 
		adms:identifier [ a adms:Identifier;
      adms:schemaAgency "DOI";
      skos:notation "10.25171/InstGeoph_PAS_ISEPOS-2018-007";
    ];
    dct:description "The geothermal project undertaken by the city of St. Gallen (Switzerland) and operated by the St. Galler Stadtwerke was based on a large-scale 3D seismic survey in 2010. The survey led to drilling of the geothermal well, “St. Gallen GT-1”, to a measured depth of 4450 m across Paleozoic / Mesozoic rock formations as well as extensive scientific and technical analysis, and well completion aimed at geothermal use. The area has additionally been instrumented with a micro-seismic array operated since 2012 by the Swiss Seismic Survey (SED). After complications occurred during well stimulation and testing in July 2013 (a gas kick and seismic events up to ML 3.5 as a consequence of killing the well) the project was temporarily stopped. In October 2013 the project was resumed with a modified drill stem test producing gas and water and collection of a comprehensive data set on the developed jointed aquifer within the regionally prominent St. Gallen Fault Zone. The geothermal project has been halted in May 2014. This episode is a data set for correlating seismic activity to fluid injection and gas-water production that lead to increased seismic activity in the past. Episode integrated in the framework of: S4CE, Science for Clean Energy. This project has received funding from the European Union’s Horizon 2020 research and innovation programme under grant agreement No 764810.";
		dct:created "2018-05-08"^^xsd:date;
		dct:modified "2018-05-08"^^xsd:date;
		dct:issued "2018-05-08"^^xsd:date;
		dct:temporal [ a dct:PeriodOfTime; 
			schema:startDate "2010-01-01T00:00:00Z"^^xsd:dateTime;
			schema:endDate "2014-05-31T00:00:00Z"^^xsd:dateTime;
		];
		dct:spatial [ a dct:Location;
	        locn:geometry "POINT(9.32 47.42)"^^gsp:wktLiteral;
	    ];
		dcat:theme <epos:Geothermalenergyproduction>;
		dcat:keyword "anthropogenic hazards","TCS AH","IS-EPOS platform", "episode", "geothermal energy production", "anthropogenic seismicity", "catalogue", "seismic waveform", "injection industrial data";
		dct:publisher <https://www.sgsw.ch>;
		dcat:contactPoint <mailto:thomas.bloch@sgsw.ch/contactPoint>;
		dcat:contactPoint <mailto:Egill.Arni.Gudnason@isor.is/contactPoint>;
		dcat:distribution <anthropogenic_hazards/distribution/episode-elements/SG>;
. 
#	<anthropogenic_hazards/dataset/episode/COTTON_VALLEY> a dcat:Dataset;
#		dct:title "COTTON VALLEY: hydraulic fracturing";
#		dct:identifier "anthropogenic_hazards/dataset/episode/COTTON_VALLEY";
#		adms:identifier [ a adms:Identifier;
#			adms:schemaAgency "DDSS-ID";
#			skos:notation "WP14-DDSS-042";
#		]; 
#		adms:identifier [ a adms:Identifier;
#     adms:schemaAgency "DOI";
#     skos:notation "XXX";
#   ];
#   dct:description "Fracture imaging study in the Carthage Gas Unit, Panola County, Texas, USA is shown that microseismic events induced by hydraulic fracturing at a depth of 9,500 ft were detected at distances exceeding 1,300 ft from the origin. An industry consortium of major operators, service companies, government agencies and national laboratories was formed to perform a more detailed study using 96, 3-component geophone sondes distributed among two monitor wells. A unique microseismic recording system specifically designed and manufactured for these operating depths is presented. Applications of the technology include optimization of hydraulic fracture designs and accurate mapping of fracture geometry. How to cite: IS EPOS (2019), Episode: COTTON VALLEY, https://tcs.ah-epos.eu/#episode:COTTON_VALLEY";
#		dct:created "2019-04-30"^^xsd:date;
#		dct:modified "2019-04-30"^^xsd:date;
#		dct:issued "2019-04-30"^^xsd:date;
#		dct:temporal [ a dct:PeriodOfTime; 
#			schema:startDate "1997-05-12T08:30:36Z"^^xsd:dateTime;
#			schema:endDate "1997-05-16T12:36:00Z"^^xsd:dateTime;
#		];
#		dct:spatial [ a dct:Location;
#	        locn:geometry "POINT(-94.42 32.17)"^^gsp:wktLiteral;
#	    ];
#		dcat:theme <epos:Unconventionalhydrocarbonextraction>;
#		dcat:keyword "anthropogenic hazards","TCS AH","IS-EPOS platform", "episode", "unconventional hydrocarbon extraction", "anthropogenic seismicity", "catalogue", "seismic waveform", "station information", "injection industrial data", "velocity model", "hydrocarbon production data";
#		dct:publisher <TODO>;
#		dcat:contactPoint <TODO>;
#		dcat:distribution <anthropogenic_hazards/distribution/episode-elements/COTTON_VALLEY>;
#. 
	<anthropogenic_hazards/dataset/episode/VOUGLANS> a dcat:Dataset;
		dct:title "VOUGLANS: water reservoir";
		dct:identifier "anthropogenic_hazards/dataset/episode/VOUGLANS";
		adms:identifier [ a adms:Identifier;
			adms:schemaAgency "DDSS-ID";
			skos:notation "WP14-DDSS-043";
		]; 
		adms:identifier [ a adms:Identifier;
      adms:schemaAgency "DOI";
      skos:notation "10.25171/InstGeoph_PAS_ISEPOS-2018-004";
    ];
    dct:description "The Vouglans dam is an hydropower reservoir located on the Ain river, Jura, France. The dam construction was completed in 1968 and so for the Vouglans Lake impoundment. This is the third largest artificial water reservoir in France by its capacity (605 Mm3). When no earthquake was recorded in the 1962-1968 period, seismicity close (25km radius) from the reservoir starts in 1969 and it lasted up to 2000’. The largest shock M4.6 occurred in 1971. Episode integrated in the framework of: EPOS IP project, European Plate Observing System Implementation Phase. This project has received funding from the European Union’s Horizon 2020 research and innovation programme under grant agreement No 676564. How to cite: IS EPOS (2018), Episode: VOUGLANS, https://tcs.ah-epos.eu/#episode:VOUGLANS, doi:10.25171/InstGeoph_PAS_ISEPOS-2018-004";
		dct:created "2019-05-06"^^xsd:date;
		dct:modified "2019-05-06"^^xsd:date;
		dct:issued "2019-05-06"^^xsd:date;
		dct:temporal [ a dct:PeriodOfTime; 
			schema:startDate "1977-09-21T23:59:59Z"^^xsd:dateTime;
			schema:endDate "2009-12-30T23:59:59Z"^^xsd:dateTime;
		];
		dct:spatial [ a dct:Location;
	        locn:geometry "POINT(5.6654 46.3976)"^^gsp:wktLiteral;
	    ];
		dcat:theme <epos:Reservoirimpoundment>;
		dcat:keyword "anthropogenic hazards","TCS AH","IS-EPOS platform", "episode", "reservoir impoundment", "anthropogenic seismicity", "catalogue", "reservoir industrial data";
		dct:publisher <https://isterre.fr>;
		dcat:contactPoint <http://orcid.org/0000-0002-9580-7864/contactPoint>;
		dcat:distribution <anthropogenic_hazards/distribution/episode-elements/VOUGLANS>;
. 
	<anthropogenic_hazards/dataset/episode/GAZLI> a dcat:Dataset;
		dct:title "GAZLI: hydrocarbon field";
		dct:identifier "anthropogenic_hazards/dataset/episode/GAZLI";
		adms:identifier [ a adms:Identifier;
			adms:schemaAgency "DDSS-ID";
			skos:notation "WP14-DDSS-044";
		]; 
		adms:identifier [ a adms:Identifier;
      adms:schemaAgency "DOI";
      skos:notation "10.25171/InstGeoph_PAS_ISEPOS-2019-002";
    ];
    dct:description "From 1976 to 1984, three magnitude 7 earthquakes struck the interplate area of Gazli (Uzbekistan), an area previously assigned to a 'low seismic risk' zone. The closeness of an important gas field suggests that these events may be induced or triggered by geo-resource production related to fluid manipulations. Since these early 1976-84 M7 events, the seismic sequence develops as a long lasting seismic swarm, up to now. Episode integrated in the framework of: EPOS IP project, European Plate Observing System Implementation Phase. This project has received funding from the European Union’s Horizon 2020 research and innovation programme under grant agreement No 676564. How to cite: IS-EPOS (2019), Episode: GAZLI, https://tcs.ah-epos.eu/#episode:GAZLI, doi:10.25171/InstGeoph_PAS_ISEPOS-2019-002";
		dct:created "2019-03-27"^^xsd:date;
		dct:modified "2019-03-27"^^xsd:date;
		dct:issued "2019-03-27"^^xsd:date;
		dct:temporal [ a dct:PeriodOfTime; 
			schema:startDate "1978-12-31T23:59:59Z"^^xsd:dateTime;
			schema:endDate "2018-12-31T00:00:00Z"^^xsd:dateTime;
		];
		dct:spatial [ a dct:Location;
	        locn:geometry "POINT(63.4 40.2)"^^gsp:wktLiteral;
	    ];
		dcat:theme <epos:Conventionalhydrocarbonextraction>;
		dcat:keyword "anthropogenic hazards","TCS AH","IS-EPOS platform", "episode", "conventional hydrocarbon extraction", "anthropogenic seismicity", "catalogue", "reservoir industrial data", "injection industrial data", "hydrocarbon production data";
		dct:publisher <https://isterre.fr>;
		dcat:contactPoint <http://orcid.org/0000-0002-9580-7864/contactPoint>;
		dcat:distribution <anthropogenic_hazards/distribution/episode-elements/GAZLI>;
. 
	<anthropogenic_hazards/dataset/episode/BOGDANKA> a dcat:Dataset;
		dct:title "BOGDANKA: underground coal mining";
		dct:identifier "anthropogenic_hazards/dataset/episode/BOGDANKA";
		adms:identifier [ a adms:Identifier;
			adms:schemaAgency "DDSS-ID";
			skos:notation "WP14-DDSS-045";
		]; 
		adms:identifier [ a adms:Identifier;
      adms:schemaAgency "DOI";
      skos:notation "10.25171/InstGeoph_PAS_ISEPOS-2019-001";
    ];
    dct:description "The BOIS contains data related to seismic activity induced by mining. In the region which is located in eastern Poland, coal is excavated by Lubelski Węgiel 'Bogdnaka' mine. The mine uses longwall system and coal seams are located from 0.5 – 1.2 km below the surface. The seismicity is monitored with 12 broad-band (5s) seismometers (GeoSIG VE-53/BB). The episode started since November 2018 and remains open. How to cite: IS-EPOS (2019), Episode: BOGDANKA, https://tcs.ah-epos.eu/#episode:BOGDANKA, doi:10.25171/InstGeoph_PAS_ISEPOS-2019-001";
		dct:created "2019-03-29"^^xsd:date;
		dct:modified "2019-03-29"^^xsd:date;
		dct:issued "2019-03-29"^^xsd:date;
		dct:temporal [ a dct:PeriodOfTime; 
			schema:startDate "2018-07-03T00:00:00Z"^^xsd:dateTime;
		];
		dct:spatial [ a dct:Location;
	        locn:geometry "POINT(23.01795 51.33645)"^^gsp:wktLiteral;
	    ];
		dcat:theme <epos:Coalmining>;
		dcat:keyword "anthropogenic hazards","TCS AH","IS-EPOS platform", "episode", "underground mining", "anthropogenic seismicity", "catalogue", "seismic waveform", "station information", "mine industrial data", "velocity model";
		dct:publisher <PIC:996625337>;
		dcat:contactPoint <http://orcid.org/0000-0002-4801-4888/contactPoint>;
		dcat:distribution <anthropogenic_hazards/distribution/episode-elements/BOGDANKA>;
. 


<anthropogenic_hazards/webservice/is-epos_platform> a epos:WebService;
	schema:identifier "anthropogenic_hazards/webservice/is-epos_platform";
	schema:description "Virtual access to IS-EPOS Platform (multiservice)";
	schema:name "Virtual access to IS-EPOS Platform";
	hydra:entrypoint "https://tcs.ah-epos.eu/"^^xsd:anyURI; 
	schema:provider <PIC:996625337>;
	schema:datePublished "2015-10-20Z"^^xsd:date;
	schema:dateModified "2018-07-30Z"^^xsd:date;
  dct:conformsTo <anthropogenic_hazards/webservice/is-epos_platform/documentation>;
	hydra:supportedOperation <anthropogenic_hazards/webservice/is-epos_platform/episodes>;
	hydra:supportedOperation <anthropogenic_hazards/webservice/is-epos_platform/apps>;
	hydra:supportedOperation <anthropogenic_hazards/webservice/is-epos_platform/episode-elements/CZORSZTYN>;
	hydra:supportedOperation <anthropogenic_hazards/webservice/is-epos_platform/episode-elements/GS>;
	hydra:supportedOperation <anthropogenic_hazards/webservice/is-epos_platform/episode-elements/LGCD>;
	hydra:supportedOperation <anthropogenic_hazards/webservice/is-epos_platform/episode-elements/SONG_TRANH>;
	hydra:supportedOperation <anthropogenic_hazards/webservice/is-epos_platform/episode-elements/USCB>;
	hydra:supportedOperation <anthropogenic_hazards/webservice/is-epos_platform/episode-elements/BOBREK>;
	hydra:supportedOperation <anthropogenic_hazards/webservice/is-epos_platform/episode-elements/PYHASALMI_MINE>;
	hydra:supportedOperation <anthropogenic_hazards/webservice/is-epos_platform/episode-elements/LGF>;
	hydra:supportedOperation <anthropogenic_hazards/webservice/is-epos_platform/episode-elements/MONTEYNARD>;
	hydra:supportedOperation <anthropogenic_hazards/webservice/is-epos_platform/episode-elements/SSFS1993>;
	hydra:supportedOperation <anthropogenic_hazards/webservice/is-epos_platform/episode-elements/SSFS2000>;
	hydra:supportedOperation <anthropogenic_hazards/webservice/is-epos_platform/episode-elements/SSFS2003>;
	hydra:supportedOperation <anthropogenic_hazards/webservice/is-epos_platform/episode-elements/SSFS2004>;
	hydra:supportedOperation <anthropogenic_hazards/webservice/is-epos_platform/episode-elements/SSFS2005>;
	hydra:supportedOperation <anthropogenic_hazards/webservice/is-epos_platform/episode-elements/GISOS-CERVILLE>;
	hydra:supportedOperation <anthropogenic_hazards/webservice/is-epos_platform/episode-elements/STARFISH>;
	hydra:supportedOperation <anthropogenic_hazards/webservice/is-epos_platform/episode-elements/THE_GEYSERS_Prati_9_and_Prati_29_cluster>;
	hydra:supportedOperation <anthropogenic_hazards/webservice/is-epos_platform/episode-elements/THE_GEYSERS>;
	hydra:supportedOperation <anthropogenic_hazards/webservice/is-epos_platform/episode-elements/VDF>;
	hydra:supportedOperation <anthropogenic_hazards/webservice/is-epos_platform/episode-elements/VD>;
#	hydra:supportedOperation <anthropogenic_hazards/webservice/is-epos_platform/episode-elements/EMILIA_ROMAGNA>;
	hydra:supportedOperation <anthropogenic_hazards/webservice/is-epos_platform/episode-elements/PREESE_HALL>;
	hydra:supportedOperation <anthropogenic_hazards/webservice/is-epos_platform/episode-elements/THORESBY_COLLIERY>;
	hydra:supportedOperation <anthropogenic_hazards/webservice/is-epos_platform/episode-elements/ASFORDBY>;
	hydra:supportedOperation <anthropogenic_hazards/webservice/is-epos_platform/episode-elements/NORTHWICH>;
	hydra:supportedOperation <anthropogenic_hazards/webservice/is-epos_platform/episode-elements/OK>;
	hydra:supportedOperation <anthropogenic_hazards/webservice/is-epos_platform/episode-elements/PREESALL_MINE>;
	hydra:supportedOperation <anthropogenic_hazards/webservice/is-epos_platform/episode-elements/GRONINGEN_FIELD>;
	hydra:supportedOperation <anthropogenic_hazards/webservice/is-epos_platform/episode-elements/LAI_CHAU>;
	hydra:supportedOperation <anthropogenic_hazards/webservice/is-epos_platform/episode-elements/LUBOCINO>;
	hydra:supportedOperation <anthropogenic_hazards/webservice/is-epos_platform/episode-elements/WYSIN>;
	hydra:supportedOperation <anthropogenic_hazards/webservice/is-epos_platform/episode-elements/CARBFIX>;
	hydra:supportedOperation <anthropogenic_hazards/webservice/is-epos_platform/episode-elements/SG>;
#	hydra:supportedOperation <anthropogenic_hazards/webservice/is-epos_platform/episode-elements/COTTON_VALLEY>;
	hydra:supportedOperation <anthropogenic_hazards/webservice/is-epos_platform/episode-elements/VOUGLANS>;
	hydra:supportedOperation <anthropogenic_hazards/webservice/is-epos_platform/episode-elements/GAZLI>;
	hydra:supportedOperation <anthropogenic_hazards/webservice/is-epos_platform/episode-elements/BOGDANKA>;
	dcat:theme <epos:Reservoirimpoundment>;
	dcat:theme <epos:Geothermalenergyproduction>;
	dcat:theme <epos:Hardrockmining>;
	dcat:theme <epos:Coalmining>;
	dcat:theme <epos:Saltsolutionsmining>;
	dcat:theme <epos:Conventionalhydrocarbonextraction>;
	dcat:theme <epos:Unconventionalhydrocarbonextraction>;
	dcat:theme <epos:CollectivePropertiesOfSeismicityAnalysis>;
  dcat:theme <epos:Converters>;
  dcat:theme <epos:CorrelationAnalysis>;
  dcat:theme <epos:Dataprocessingapplications>;
  dcat:theme <epos:DownloadTools>;
  dcat:theme <epos:EarthquakeInteractionsAnalysis>;
  dcat:theme <epos:EventDetectionAlgorithms>;
  dcat:theme <epos:FilteringTools>;
  dcat:theme <epos:ProbabilisticSeismicHazardAnalysis>;
  dcat:theme <epos:SeismogramAnalysisTools>;
  dcat:theme <epos:SourceParameterEstimation>;
  dcat:theme <epos:StressFieldModeling>;
  dcat:theme <epos:Visualizations>;
  schema:keywords "anthropogenic hazards","tcs ah","is-epos platform","web platform","multiservice","research environment","workspace","applications","episode","document repository";
	dcat:contactPoint <http://orcid.org/0000-0002-4801-4888/contactPoint>;
	dcat:contactPoint <mailto:m.sterzel@cyfronet.pl/contactPoint>;
. 

<anthropogenic_hazards/webservice/is-epos_platform/documentation> a hydra:APIDocumentation ;
      hydra:title "IS-EPOS Platform User Guide" ;
      hydra:description "IS-EPOS Platform User Guide" ;
      hydra:entrypoint "https://docs.cyfronet.pl/display/ISDOC" ;
.

	<anthropogenic_hazards/webservice/is-epos_platform/episodes> a hydra:Operation;
		hydra:method "GET"^^xsd:string;
		hydra:returns "application/json";
		hydra:property[ a hydra:IriTemplate;
			hydra:template "https://tcs.ah-epos.eu/api/epos/episodes{?impactingFactor}"^^xsd:string;
				hydra:mapping[ a hydra:IriTemplateMapping;
					hydra:variable "impactingFactor"^^xsd:string;
					rdfs:range "xsd:string";
					rdfs:label "Impacting Factor of the episode";
					http:paramValue "CO2 sequestration";
					http:paramValue "conventional hydrocarbon extraction";
					http:paramValue "geothermal energy production";
					http:paramValue "reservoir impoundment";
					http:paramValue "unconventional hydrocarbon extraction";
					http:paramValue "underground gas storage";
					http:paramValue "underground mining";
					http:paramValue "wastewater injection";
					hydra:required "false"^^xsd:boolean;
				];
		] ;
. 
	<anthropogenic_hazards/webservice/is-epos_platform/apps> a hydra:Operation;
		hydra:method "GET"^^xsd:string;
		hydra:returns "application/json";
		hydra:property[ a hydra:IriTemplate;
			hydra:template "https://tcs.ah-epos.eu/api/epos/apps{?category, keyword}"^^xsd:string;
				hydra:mapping[ a hydra:IriTemplateMapping;
					hydra:variable "category"^^xsd:string;
					rdfs:range "xsd:string";
					rdfs:label "Category to filter applications";
					http:paramValue "Collective Properties of Seismicity";
					http:paramValue "Converters";
					http:paramValue "Correlation Analysis";
					http:paramValue "Data Processing Applications";
					http:paramValue "Download Tools";
					http:paramValue "Earthquake Interactions";
					http:paramValue "Event Detection Algorithms";
					http:paramValue "Filtering Tools";
					http:paramValue "Probabilistic Seismic Hazard Analysis";
					http:paramValue "Seismogram Analysis Tools";
					http:paramValue "Source Parameter Estimation";
					http:paramValue "Stress Field Modeling";
					http:paramValue "Visualizations";
					hydra:required "false"^^xsd:boolean;
				];
				hydra:mapping[ a hydra:IriTemplateMapping;
					hydra:variable "keyword"^^xsd:string;
					rdfs:range "xsd:string";
					rdfs:label "Keywords to filter applications. Sample values: 'Statistical analysis', 'Statistical properties of seismicity', 'Parameter probabilistic distribution', 'Source parameters', 'Source location', 'Earthquake spectra, 'Stress modelling', 'Geo-resource production impact', 'Production - seismicity interaction', 'Time-dependent hazard'";
					hydra:required "false"^^xsd:boolean;
				];
		] ;
. 
	<anthropogenic_hazards/webservice/is-epos_platform/episode-elements/CZORSZTYN> a hydra:Operation;
		hydra:method "GET"^^xsd:string;
		hydra:returns "application/json";
		hydra:property[ a hydra:IriTemplate;
			hydra:template "https://tcs.ah-epos.eu/api/epos/episodes/{episode}"^^xsd:string;
				hydra:mapping[ a hydra:IriTemplateMapping;
					hydra:variable "episode"^^xsd:string;
					rdfs:range "xsd:string";
					rdfs:label "Episode dataset contains: seismic data: Catalog, Seismic Network, Event related waveforms; industrial data: Shoreline, Water Level, Water Volume; geodata: Velocity Model, Bathymetric map. From 2013-08-25 till now. Additional configuration and filtration possible on the IS-EPOS Platform - please select the 'Download' button.";
					schema:defaultValue "CZORSZTYN";
					http:paramValue "CZORSZTYN" ;
					hydra:required "true"^^xsd:boolean;
				];
		] ;
. 
	<anthropogenic_hazards/webservice/is-epos_platform/episode-elements/GS> a hydra:Operation;
		hydra:method "GET"^^xsd:string;
		hydra:returns "application/json";
		hydra:property[ a hydra:IriTemplate;
			hydra:template "https://tcs.ah-epos.eu/api/epos/episodes/{episode}"^^xsd:string;
				hydra:mapping[ a hydra:IriTemplateMapping;
					hydra:variable "episode"^^xsd:string;
					rdfs:range "xsd:string";
					rdfs:label "Episode dataset contains: seismic data: Catalog, Seismic Network, Event related waveforms; industrial data: Injection Rate, Wellhead Pressure, Well Paths; geodata: Velocity Model. From 2007-08-09 till 2007-08-19. Additional configuration and filtration possible on the IS-EPOS Platform - please select the 'Download' button.";
					schema:defaultValue "GS";
					http:paramValue "GS" ;
					hydra:required "true"^^xsd:boolean;
				];
		] ;
. 
	<anthropogenic_hazards/webservice/is-epos_platform/episode-elements/LGCD> a hydra:Operation;
		hydra:method "GET"^^xsd:string;
		hydra:returns "application/json";
		hydra:property[ a hydra:IriTemplate;
			hydra:template "https://tcs.ah-epos.eu/api/epos/episodes/{episode}"^^xsd:string;
				hydra:mapping[ a hydra:IriTemplateMapping;
					hydra:variable "episode"^^xsd:string;
					rdfs:range "xsd:string";
					rdfs:label "Episode dataset contains: seismic data: Catalog, Event related accelerograms, Event related waveforms, Continuous waveforms, Ground Motion Catalog, Ground Motion Network, Seismic Network; industrial data: Mine Area, Shoreline; geodata: Velocity Model. From 2013-12-10 till now. Additional configuration and filtration possible on the IS-EPOS Platform - please select the 'Download' button.";
					schema:defaultValue "LGCD";
					http:paramValue "LGCD" ;
					hydra:required "true"^^xsd:boolean;
				];
		] ;
. 
	<anthropogenic_hazards/webservice/is-epos_platform/episode-elements/SONG_TRANH> a hydra:Operation;
		hydra:method "GET"^^xsd:string;
		hydra:returns "application/json";
		hydra:property[ a hydra:IriTemplate;
			hydra:template "https://tcs.ah-epos.eu/api/epos/episodes/{episode}"^^xsd:string;
				hydra:mapping[ a hydra:IriTemplateMapping;
					hydra:variable "episode"^^xsd:string;
					rdfs:range "xsd:string";
					rdfs:label "Episode dataset contains: seismic data: Catalog, Event related waveforms, Seismic Network; industrial data: Shoreline, Water Level; geodata: Velocity Model, Faults map. From 2011-01-01 till now. Additional configuration and filtration possible on the IS-EPOS Platform - please select the 'Download' button.";
					schema:defaultValue "SONG_TRANH";
					http:paramValue "SONG_TRANH" ;
					hydra:required "true"^^xsd:boolean;
				];
		] ;
. 
	<anthropogenic_hazards/webservice/is-epos_platform/episode-elements/USCB> a hydra:Operation;
		hydra:method "GET"^^xsd:string;
		hydra:returns "application/json";
		hydra:property[ a hydra:IriTemplate;
			hydra:template "https://tcs.ah-epos.eu/api/epos/episodes/{episode}"^^xsd:string;
				hydra:mapping[ a hydra:IriTemplateMapping;
					hydra:variable "episode"^^xsd:string;
					rdfs:range "xsd:string";
					rdfs:label "Episode dataset contains: seismic data: Catalog, Event related accelerograms, Event related waveforms, Ground Motion Catalog, Ground Motion Network, Seismic Network; industrial data: Mine Area, Geoarea; geodata: Faults, Shear Wave Velocity, Velocity Model. From 2014-01-02 till now. Additional configuration and filtration possible on the IS-EPOS Platform - please select the 'Download' button.";
					schema:defaultValue "USCB";
					http:paramValue "USCB" ;
					hydra:required "true"^^xsd:boolean;
				];
		] ;
. 
	<anthropogenic_hazards/webservice/is-epos_platform/episode-elements/BOBREK> a hydra:Operation;
		hydra:method "GET"^^xsd:string;
		hydra:returns "application/json";
		hydra:property[ a hydra:IriTemplate;
			hydra:template "https://tcs.ah-epos.eu/api/epos/episodes/{episode}"^^xsd:string;
				hydra:mapping[ a hydra:IriTemplateMapping;
					hydra:variable "episode"^^xsd:string;
					rdfs:range "xsd:string";
					rdfs:label "Episode dataset contains: seismic data: Catalog, Event related waveforms, Seismic Network; industrial data: Mine Area, Mining Front Advance; geodata: 3D models of mine seams, Velocity Model. From 2009-04-12 till 2010-07-07. Additional configuration and filtration possible on the IS-EPOS Platform - please select the 'Download' button.";
					schema:defaultValue "BOBREK";
					http:paramValue "BOBREK" ;
					hydra:required "true"^^xsd:boolean;
				];
		] ;
. 
	<anthropogenic_hazards/webservice/is-epos_platform/episode-elements/PYHASALMI_MINE> a hydra:Operation;
		hydra:method "GET"^^xsd:string;
		hydra:returns "application/json";
		hydra:property[ a hydra:IriTemplate;
			hydra:template "https://tcs.ah-epos.eu/api/epos/episodes/{episode}"^^xsd:string;
				hydra:mapping[ a hydra:IriTemplateMapping;
					hydra:variable "episode"^^xsd:string;
					rdfs:range "xsd:string";
					rdfs:label "Episode dataset contains: seismic data: Catalog, Event related waveforms, Seismic Network; industrial data: Blast Information, Collar Drillhole Position, Mine Area, Mining Polygon Advance, Well Paths; geodata: Bedrock Maps, Drillhole Lithology, Geophysical Maps, Velocity Model. From 2010-10-01 till 2011-03-31. Additional configuration and filtration possible on the IS-EPOS Platform - please select the 'Download' button.";
					schema:defaultValue "PYHASALMI_MINE";
					http:paramValue "PYHASALMI_MINE" ;
					hydra:required "true"^^xsd:boolean;
				];
		] ;
. 
	<anthropogenic_hazards/webservice/is-epos_platform/episode-elements/LGF> a hydra:Operation;
		hydra:method "GET"^^xsd:string;
		hydra:returns "application/json";
		hydra:property[ a hydra:IriTemplate;
			hydra:template "https://tcs.ah-epos.eu/api/epos/episodes/{episode}"^^xsd:string;
				hydra:mapping[ a hydra:IriTemplateMapping;
					hydra:variable "episode"^^xsd:string;
					rdfs:range "xsd:string";
					rdfs:label "Episode dataset contains: seismic data: Catalog, Seismic Network; industrial data: Gas Reservoir Pressure, Injection Volume, Gas Field Area, Natural Gas Production; geodata: Geological Section, Velocity Model. From 1977-12-31 till 2016-12-31. Additional configuration and filtration possible on the IS-EPOS Platform - please select the 'Download' button.";
					schema:defaultValue "LGF";
					http:paramValue "LGF" ;
					hydra:required "true"^^xsd:boolean;
				];
		] ;
. 
	<anthropogenic_hazards/webservice/is-epos_platform/episode-elements/MONTEYNARD> a hydra:Operation;
		hydra:method "GET"^^xsd:string;
		hydra:returns "application/json";
		hydra:property[ a hydra:IriTemplate;
			hydra:template "https://tcs.ah-epos.eu/api/epos/episodes/{episode}"^^xsd:string;
				hydra:mapping[ a hydra:IriTemplateMapping;
					hydra:variable "episode"^^xsd:string;
					rdfs:range "xsd:string";
					rdfs:label "Episode dataset contains: seismic data: Catalog; industrial data: Water Height, Water Level, Shoreline. From 1962-04-12 till 2009-12-29. Additional configuration and filtration possible on the IS-EPOS Platform - please select the 'Download' button.";
					schema:defaultValue "MONTEYNARD";
					http:paramValue "MONTEYNARD" ;
					hydra:required "true"^^xsd:boolean;
				];
		] ;
. 
	<anthropogenic_hazards/webservice/is-epos_platform/episode-elements/SSFS1993> a hydra:Operation;
		hydra:method "GET"^^xsd:string;
		hydra:returns "application/json";
		hydra:property[ a hydra:IriTemplate;
			hydra:template "https://tcs.ah-epos.eu/api/epos/episodes/{episode}"^^xsd:string;
				hydra:mapping[ a hydra:IriTemplateMapping;
					hydra:variable "episode"^^xsd:string;
					rdfs:range "xsd:string";
					rdfs:label "Episode dataset contains: seismic data: Catalog, Event related waveforms, Seismic Network; industrial data: Injection Rate, Wellhead Presssure; geodata: Velocity Model. From 1993-09-01 till 1993-10-25. Additional configuration and filtration possible on the IS-EPOS Platform - please select the 'Download' button.";
					schema:defaultValue "SSFS1993";
					http:paramValue "SSFS1993" ;
					hydra:required "true"^^xsd:boolean;
				];
		] ;
. 
	<anthropogenic_hazards/webservice/is-epos_platform/episode-elements/SSFS2000> a hydra:Operation;
		hydra:method "GET"^^xsd:string;
		hydra:returns "application/json";
		hydra:property[ a hydra:IriTemplate;
			hydra:template "https://tcs.ah-epos.eu/api/epos/episodes/{episode}"^^xsd:string;
				hydra:mapping[ a hydra:IriTemplateMapping;
					hydra:variable "episode"^^xsd:string;
					rdfs:range "xsd:string";
					rdfs:label "Episode dataset contains: seismic data: Catalog, Seismic Stations; industrial data: Injection Rate, Wellhead Presssure. From 2000-06-28 till 2000-07-16. Additional configuration and filtration possible on the IS-EPOS Platform - please select the 'Download' button.";
					schema:defaultValue "SSFS2000";
					http:paramValue "SSFS2000" ;
					hydra:required "true"^^xsd:boolean;
				];
		] ;
. 
	<anthropogenic_hazards/webservice/is-epos_platform/episode-elements/SSFS2003> a hydra:Operation;
		hydra:method "GET"^^xsd:string;
		hydra:returns "application/json";
		hydra:property[ a hydra:IriTemplate;
			hydra:template "https://tcs.ah-epos.eu/api/epos/episodes/{episode}"^^xsd:string;
				hydra:mapping[ a hydra:IriTemplateMapping;
					hydra:variable "episode"^^xsd:string;
					rdfs:range "xsd:string";
					rdfs:label "Episode dataset contains: seismic data: Catalog, Seismic Stations; industrial data: Injection Rate, Wellhead Presssure, Flowback Rate. From 2003-01-22 till 2003-03-19. Additional configuration and filtration possible on the IS-EPOS Platform - please select the 'Download' button.";
					schema:defaultValue "SSFS2003";
					http:paramValue "SSFS2003" ;
					hydra:required "true"^^xsd:boolean;
				];
		] ;
. 
	<anthropogenic_hazards/webservice/is-epos_platform/episode-elements/SSFS2004> a hydra:Operation;
		hydra:method "GET"^^xsd:string;
		hydra:returns "application/json";
		hydra:property[ a hydra:IriTemplate;
			hydra:template "https://tcs.ah-epos.eu/api/epos/episodes/{episode}"^^xsd:string;
				hydra:mapping[ a hydra:IriTemplateMapping;
					hydra:variable "episode"^^xsd:string;
					rdfs:range "xsd:string";
					rdfs:label "Episode dataset contains: seismic data: Catalog, Seismic Stations; industrial data: Injection Rate, Injection Volume, Wellhead Presssure, Flowback Rate, Flowback Volume; geodata: Velocity Model. From 2004-09-06 till 2004-10-01. Additional configuration and filtration possible on the IS-EPOS Platform - please select the 'Download' button.";
					schema:defaultValue "SSFS2004";
					http:paramValue "SSFS2004" ;
					hydra:required "true"^^xsd:boolean;
				];
		] ;
. 
	<anthropogenic_hazards/webservice/is-epos_platform/episode-elements/SSFS2005> a hydra:Operation;
		hydra:method "GET"^^xsd:string;
		hydra:returns "application/json";
		hydra:property[ a hydra:IriTemplate;
			hydra:template "https://tcs.ah-epos.eu/api/epos/episodes/{episode}"^^xsd:string;
				hydra:mapping[ a hydra:IriTemplateMapping;
					hydra:variable "episode"^^xsd:string;
					rdfs:range "xsd:string";
					rdfs:label "Episode dataset contains: seismic data: Catalog, Seismic Stations; industrial data: Injection Rate, Injection Volume, Wellhead Presssure; geodata: Velocity Model. From 2005-02-03 till 2005-04-02. Additional configuration and filtration possible on the IS-EPOS Platform - please select the 'Download' button.";
					schema:defaultValue "SSFS2005";
					http:paramValue "SSFS2005" ;
					hydra:required "true"^^xsd:boolean;
				];
		] ;
. 
	<anthropogenic_hazards/webservice/is-epos_platform/episode-elements/GISOS-CERVILLE> a hydra:Operation;
		hydra:method "GET"^^xsd:string;
		hydra:returns "application/json";
		hydra:property[ a hydra:IriTemplate;
			hydra:template "https://tcs.ah-epos.eu/api/epos/episodes/{episode}"^^xsd:string;
				hydra:mapping[ a hydra:IriTemplateMapping;
					hydra:variable "episode"^^xsd:string;
					rdfs:range "xsd:string";
					rdfs:label "Episode dataset contains: seismic data: Catalog, Event related waveforms, Seismic Network; industrial data: Cavity Roof Level, Cavity Roof Polygon, Ground Water Level, Well Positions; geodata: Deformation Measurements, Velocity Model. From 2008-03-06 till 2009-02-12. Additional configuration and filtration possible on the IS-EPOS Platform - please select the 'Download' button.";
					schema:defaultValue "GISOS-CERVILLE";
					http:paramValue "GISOS-CERVILLE" ;
					hydra:required "true"^^xsd:boolean;
				];
		] ;
. 
	<anthropogenic_hazards/webservice/is-epos_platform/episode-elements/STARFISH> a hydra:Operation;
		hydra:method "GET"^^xsd:string;
		hydra:returns "application/json";
		hydra:property[ a hydra:IriTemplate;
			hydra:template "https://tcs.ah-epos.eu/api/epos/episodes/{episode}"^^xsd:string;
				hydra:mapping[ a hydra:IriTemplateMapping;
					hydra:variable "episode"^^xsd:string;
					rdfs:range "xsd:string";
					rdfs:label "Episode dataset contains: seismic data: Catalog, Event related waveforms, Seismic Network; industrial data: Insitu Temperature, Insitu Temperature Stations; geodata: Strain Gauge Measurement. From 2014-04-09 till 2015-02-25. Additional configuration and filtration possible on the IS-EPOS Platform - please select the 'Download' button.";
					schema:defaultValue "STARFISH";
					http:paramValue "STARFISH" ;
					hydra:required "true"^^xsd:boolean;
				];
		] ;
. 
	<anthropogenic_hazards/webservice/is-epos_platform/episode-elements/THE_GEYSERS_Prati_9_and_Prati_29_cluster> a hydra:Operation;
		hydra:method "GET"^^xsd:string;
		hydra:returns "application/json";
		hydra:property[ a hydra:IriTemplate;
			hydra:template "https://tcs.ah-epos.eu/api/epos/episodes/{episode}"^^xsd:string;
				hydra:mapping[ a hydra:IriTemplateMapping;
					hydra:variable "episode"^^xsd:string;
					rdfs:range "xsd:string";
					rdfs:label "Episode dataset contains: seismic data: Catalog; industrial data: Injection Rate, Well Paths. From 2007-12-10 till 2014-08-23. Additional configuration and filtration possible on the IS-EPOS Platform - please select the 'Download' button.";
					schema:defaultValue "THE_GEYSERS_Prati_9_and_Prati_29_cluster";
					http:paramValue "THE_GEYSERS_Prati_9_and_Prati_29_cluster" ;
					hydra:required "true"^^xsd:boolean;
				];
		] ;
. 
	<anthropogenic_hazards/webservice/is-epos_platform/episode-elements/THE_GEYSERS> a hydra:Operation;
		hydra:method "GET"^^xsd:string;
		hydra:returns "application/json";
		hydra:property[ a hydra:IriTemplate;
			hydra:template "https://tcs.ah-epos.eu/api/epos/episodes/{episode}"^^xsd:string;
				hydra:mapping[ a hydra:IriTemplateMapping;
					hydra:variable "episode"^^xsd:string;
					rdfs:range "xsd:string";
					rdfs:label "Episode dataset contains: seismic data: Catalog, Event related accelerograms, Event related waveforms, Ground Motion Network, Seismic Network; industrial data: Injection Volume, Powerplant Positions, Steam Production, Well Positions, Wells Records; geodata: Faults. From 1970-04-01 till 2011-10-31. Additional configuration and filtration possible on the IS-EPOS Platform - please select the 'Download' button.";
					schema:defaultValue "THE_GEYSERS";
					http:paramValue "THE_GEYSERS" ;
					hydra:required "true"^^xsd:boolean;
				];
		] ;
. 
	<anthropogenic_hazards/webservice/is-epos_platform/episode-elements/VDF> a hydra:Operation;
		hydra:method "GET"^^xsd:string;
		hydra:returns "application/json";
		hydra:property[ a hydra:IriTemplate;
			hydra:template "https://tcs.ah-epos.eu/api/epos/episodes/{episode}"^^xsd:string;
				hydra:mapping[ a hydra:IriTemplateMapping;
					hydra:variable "episode"^^xsd:string;
					rdfs:range "xsd:string";
					rdfs:label "Episode dataset contains: seismic data: Catalog, Event related waveforms, Seismic Network; industrial data: Injection Volume, Wellhead Pressure; geodata: Velocity Model. From 2006-06-01 till 2006-06-12. Additional configuration and filtration possible on the IS-EPOS Platform - please select the 'Download' button.";
					schema:defaultValue "VDF";
					http:paramValue "VDF" ;
					hydra:required "true"^^xsd:boolean;
				];
		] ;
. 
	<anthropogenic_hazards/webservice/is-epos_platform/episode-elements/VD> a hydra:Operation;
		hydra:method "GET"^^xsd:string;
		hydra:returns "application/json";
		hydra:property[ a hydra:IriTemplate;
			hydra:template "https://tcs.ah-epos.eu/api/epos/episodes/{episode}"^^xsd:string;
				hydra:mapping[ a hydra:IriTemplateMapping;
					hydra:variable "episode"^^xsd:string;
					rdfs:range "xsd:string";
					rdfs:label "Episode dataset contains: seismic data: Catalog, Event related waveforms, Seismic Network; industrial data: Water Level; geodata: Velocity Model. From 2005-05-05 till 2006-06-12. Additional configuration and filtration possible on the IS-EPOS Platform - please select the 'Download' button.";
					schema:defaultValue "VD";
					http:paramValue "VD" ;
					hydra:required "true"^^xsd:boolean;
				];
		] ;
. 
#	<anthropogenic_hazards/webservice/is-epos_platform/episode-elements/EMILIA_ROMAGNA> a hydra:Operation;
#		hydra:method "GET"^^xsd:string;
#		hydra:returns "application/json";
#		hydra:property[ a hydra:IriTemplate;
#			hydra:template "https://tcs.ah-epos.eu/api/epos/episodes/{episode}"^^xsd:string;
#				hydra:mapping[ a hydra:IriTemplateMapping;
#					hydra:variable "episode"^^xsd:string;
#					rdfs:range "xsd:string";
#					rdfs:label "Episode dataset contains: seismic data: Catalog; industrial data: Natural Gas Production, Oil Production, Water Production. From 2005-05-01 till 2006-12-01. Additional configuration and filtration possible on the IS-EPOS Platform - please select the 'Download' button.";
#					schema:defaultValue "EMILIA ROMAGNA";
#					http:paramValue "EMILIA ROMAGNA" ;
#					hydra:required "true"^^xsd:boolean;
#				];
#				];
#		] ;
#. 
	<anthropogenic_hazards/webservice/is-epos_platform/episode-elements/PREESE_HALL> a hydra:Operation;
		hydra:method "GET"^^xsd:string;
		hydra:returns "application/json";
		hydra:property[ a hydra:IriTemplate;
			hydra:template "https://tcs.ah-epos.eu/api/epos/episodes/{episode}"^^xsd:string;
				hydra:mapping[ a hydra:IriTemplateMapping;
					hydra:variable "episode"^^xsd:string;
					rdfs:range "xsd:string";
					rdfs:label "Episode dataset contains: seismic data: Catalog, Continuous waveforms, Seismic Network; industrial data: Bottomhole Pressure, Flowback Bottomhole Pressure, Flowback Rate, Flowback Volume, Injection Rate, Injection Volume, Proppant Concentration, Well Path, Wellhead Pressure; geodata: Velocity Model. From 2011-03-26 till 2011-11-23. Additional configuration and filtration possible on the IS-EPOS Platform - please select the 'Download' button.";
					schema:defaultValue "PREESE_HALL";
					http:paramValue "PREESE_HALL" ;
					hydra:required "true"^^xsd:boolean;
				];
		] ;
. 
	<anthropogenic_hazards/webservice/is-epos_platform/episode-elements/THORESBY_COLLIERY> a hydra:Operation;
		hydra:method "GET"^^xsd:string;
		hydra:returns "application/json";
		hydra:property[ a hydra:IriTemplate;
			hydra:template "https://tcs.ah-epos.eu/api/epos/episodes/{episode}"^^xsd:string;
				hydra:mapping[ a hydra:IriTemplateMapping;
					hydra:variable "episode"^^xsd:string;
					rdfs:range "xsd:string";
					rdfs:label "Episode dataset contains: seismic data: Catalog, Event related waveforms, Seismic Network; industrial data: Mine Area; geodata: Velocity Model. From 1996-08-31 till 1997-03-11. Additional configuration and filtration possible on the IS-EPOS Platform - please select the 'Download' button.";
					schema:defaultValue "THORESBY_COLLIERY";
					http:paramValue "THORESBY_COLLIERY" ;
					hydra:required "true"^^xsd:boolean;
				];
		] ;
. 
	<anthropogenic_hazards/webservice/is-epos_platform/episode-elements/ASFORDBY> a hydra:Operation;
		hydra:method "GET"^^xsd:string;
		hydra:returns "application/json";
		hydra:property[ a hydra:IriTemplate;
			hydra:template "https://tcs.ah-epos.eu/api/epos/episodes/{episode}"^^xsd:string;
				hydra:mapping[ a hydra:IriTemplateMapping;
					hydra:variable "episode"^^xsd:string;
					rdfs:range "xsd:string";
					rdfs:label "Episode dataset contains: seismic data: Catalog, Event related waveforms, Seismic Network; industrial data: Mine Area, Mining Front Advance, Well Position; geodata: Faults, Velocity Model. From 1995-04-10 till 1996-01-21. Additional configuration and filtration possible on the IS-EPOS Platform - please select the 'Download' button.";
					schema:defaultValue "ASFORDBY";
					http:paramValue "ASFORDBY" ;
					hydra:required "true"^^xsd:boolean;
				];
		] ;
. 
	<anthropogenic_hazards/webservice/is-epos_platform/episode-elements/NORTHWICH> a hydra:Operation;
		hydra:method "GET"^^xsd:string;
		hydra:returns "application/json";
		hydra:property[ a hydra:IriTemplate;
			hydra:template "https://tcs.ah-epos.eu/api/epos/episodes/{episode}"^^xsd:string;
				hydra:mapping[ a hydra:IriTemplateMapping;
					hydra:variable "episode"^^xsd:string;
					rdfs:range "xsd:string";
					rdfs:label "Episode dataset contains: seismic data: Event related waveforms, Seismic Network; industrial data: Mine Area; geodata: Gravity Monitoring, Deformation Measurements, Velocity Model. From 2001-07-01 till 2006-03-01. Additional configuration and filtration possible on the IS-EPOS Platform - please select the 'Download' button.";
					schema:defaultValue "NORTHWICH";
					http:paramValue "NORTHWICH" ;
					hydra:required "true"^^xsd:boolean;
				];
		] ;
. 
	<anthropogenic_hazards/webservice/is-epos_platform/episode-elements/OK> a hydra:Operation;
		hydra:method "GET"^^xsd:string;
		hydra:returns "application/json";
		hydra:property[ a hydra:IriTemplate;
			hydra:template "https://tcs.ah-epos.eu/api/epos/episodes/{episode}"^^xsd:string;
				hydra:mapping[ a hydra:IriTemplateMapping;
					hydra:variable "episode"^^xsd:string;
					rdfs:range "xsd:string";
					rdfs:label "Episode dataset contains: seismic data: Catalog, Event related waveforms, Seismic Network; industrial data: Injection Rate, Injection Volume, Well Positions; geodata: Faults. From 2010-01-01 till 2016-12-31. Additional configuration and filtration possible on the IS-EPOS Platform - please select the 'Download' button.";
					schema:defaultValue "OK";
					http:paramValue "OK" ;
					hydra:required "true"^^xsd:boolean;
				];
		] ;
. 
	<anthropogenic_hazards/webservice/is-epos_platform/episode-elements/PREESALL_MINE> a hydra:Operation;
		hydra:method "GET"^^xsd:string;
		hydra:returns "application/json";
		hydra:property[ a hydra:IriTemplate;
			hydra:template "https://tcs.ah-epos.eu/api/epos/episodes/{episode}"^^xsd:string;
				hydra:mapping[ a hydra:IriTemplateMapping;
					hydra:variable "episode"^^xsd:string;
					rdfs:range "xsd:string";
					rdfs:label "Episode dataset contains: seismic data: Catalog, Event related waveforms, Seismic Network; industrial data: Brine Well Positions; geodata: Gravity Monitoring, Gravity Stations, Geology map. From 2000-04-01 till 2001-03-01. Additional configuration and filtration possible on the IS-EPOS Platform - please select the 'Download' button.";
					schema:defaultValue "PREESALL_MINE";
					http:paramValue "PREESALL_MINE" ;
					hydra:required "true"^^xsd:boolean;
				];
		] ;
. 
	<anthropogenic_hazards/webservice/is-epos_platform/episode-elements/GRONINGEN_FIELD> a hydra:Operation;
		hydra:method "GET"^^xsd:string;
		hydra:returns "application/json";
		hydra:property[ a hydra:IriTemplate;
			hydra:template "https://tcs.ah-epos.eu/api/epos/episodes/{episode}"^^xsd:string;
				hydra:mapping[ a hydra:IriTemplateMapping;
					hydra:variable "episode"^^xsd:string;
					rdfs:range "xsd:string";
					rdfs:label "Episode dataset contains: seismic data: Catalog, Ground Motion Catalog, Seismic Network; satellite data; industrial data: Natural Gas Production, Production Cluster Position. From 2001-06-01 till 2017-05-30. Additional configuration and filtration possible on the IS-EPOS Platform - please select the 'Download' button.";
					schema:defaultValue "GRONINGEN_FIELD";
					http:paramValue "GRONINGEN_FIELD" ;
					hydra:required "true"^^xsd:boolean;
				];
		] ;
. 
	<anthropogenic_hazards/webservice/is-epos_platform/episode-elements/LAI_CHAU> a hydra:Operation;
		hydra:method "GET"^^xsd:string;
		hydra:returns "application/json";
		hydra:property[ a hydra:IriTemplate;
			hydra:template "https://tcs.ah-epos.eu/api/epos/episodes/{episode}"^^xsd:string;
				hydra:mapping[ a hydra:IriTemplateMapping;
					hydra:variable "episode"^^xsd:string;
					rdfs:range "xsd:string";
					rdfs:label "Episode dataset contains: seismic data: Catalog, Event related waveforms, Seismic Network; industrial data: Shoreline, Water Level. From 2014-10-06 till now. Additional configuration and filtration possible on the IS-EPOS Platform - please select the 'Download' button.";
					schema:defaultValue "LAI_CHAU";
					http:paramValue "LAI_CHAU" ;
					hydra:required "true"^^xsd:boolean;
				];
		] ;
. 
	<anthropogenic_hazards/webservice/is-epos_platform/episode-elements/LUBOCINO> a hydra:Operation;
		hydra:method "GET"^^xsd:string;
		hydra:returns "application/json";
		hydra:property[ a hydra:IriTemplate;
			hydra:template "https://tcs.ah-epos.eu/api/epos/episodes/{episode}"^^xsd:string;
				hydra:mapping[ a hydra:IriTemplateMapping;
					hydra:variable "episode"^^xsd:string;
					rdfs:range "xsd:string";
					rdfs:label "Episode dataset contains: water quality data: Chemical Water Properties, Groundwater Level, Physicochemical Water Properties, Well Position, Water Lab Analyses, Water Stations; sattelite data. From 2011-06-20 till 2014-04-02. Additional configuration and filtration possible on the IS-EPOS Platform - please select the 'Download' button.";
					schema:defaultValue "LUBOCINO";
					http:paramValue "LUBOCINO" ;
					hydra:required "true"^^xsd:boolean;
				];
		] ;
. 
	<anthropogenic_hazards/webservice/is-epos_platform/episode-elements/WYSIN> a hydra:Operation;
		hydra:method "GET"^^xsd:string;
		hydra:returns "application/json";
		hydra:property[ a hydra:IriTemplate;
			hydra:template "https://tcs.ah-epos.eu/api/epos/episodes/{episode}"^^xsd:string;
				hydra:mapping[ a hydra:IriTemplateMapping;
					hydra:variable "episode"^^xsd:string;
					rdfs:range "xsd:string";
					rdfs:label "Episode dataset contains: seismic data: Continuous waveforms, Seismic Network; air quality data: Air Stations, Atmospheric Pressure, Chemical Air Properties, Radon 222 Concentration; water quality data: Physicochemical Water Properties, Water Lab Analyses, Water Stations, Well Paths, Well Positions; sattelite data; geodata: Drillhole Lithology, Velocity Model. From 2015-06-09 till 2018-02-28. Additional configuration and filtration possible on the IS-EPOS Platform - please select the 'Download' button.";
					schema:defaultValue "WYSIN";
					http:paramValue "WYSIN" ;
					hydra:required "true"^^xsd:boolean;
				];
		] ;
. 
	<anthropogenic_hazards/webservice/is-epos_platform/episode-elements/CARBFIX> a hydra:Operation;
		hydra:method "GET"^^xsd:string;
		hydra:returns "application/json";
		hydra:property[ a hydra:IriTemplate;
			hydra:template "https://tcs.ah-epos.eu/api/epos/episodes/{episode}"^^xsd:string;
				hydra:mapping[ a hydra:IriTemplateMapping;
					hydra:variable "episode"^^xsd:string;
					rdfs:range "xsd:string";
					rdfs:label "Episode dataset contains: seismic data: Catalog, Seismic Network; industrial data: Ground Water Level, Well Path, Well Position; geodata: Drillhole Lithology. From 2017-11-29 till 2018-02-28. Additional configuration and filtration possible on the IS-EPOS Platform - please select the 'Download' button.";
					schema:defaultValue "CARBFIX";
					http:paramValue "CARBFIX" ;
					hydra:required "true"^^xsd:boolean;
				];
		] ;
. 
	<anthropogenic_hazards/webservice/is-epos_platform/episode-elements/SG> a hydra:Operation;
		hydra:method "GET"^^xsd:string;
		hydra:returns "application/json";
		hydra:property[ a hydra:IriTemplate;
			hydra:template "https://tcs.ah-epos.eu/api/epos/episodes/{episode}"^^xsd:string;
				hydra:mapping[ a hydra:IriTemplateMapping;
					hydra:variable "episode"^^xsd:string;
					rdfs:range "xsd:string";
					rdfs:label "Episode dataset contains: seismic data: Catalog, Continuous waveforms; industrial data: Well Path, Well Position. From 2010-01-01 till 2014-05-31. Additional configuration and filtration possible on the IS-EPOS Platform - please select the 'Download' button.";
					schema:defaultValue "SG";
					http:paramValue "SG" ;
					hydra:required "true"^^xsd:boolean;
				];
		] ;
. 
#	<anthropogenic_hazards/webservice/is-epos_platform/episode-elements/COTTON_VALLEY> a hydra:Operation;
#		hydra:method "GET"^^xsd:string;
#		hydra:returns "application/json";
#		hydra:property[ a hydra:IriTemplate;
#			hydra:template "https://tcs.ah-epos.eu/api/epos/episodes/{episode}"^^xsd:string;
#				hydra:mapping[ a hydra:IriTemplateMapping;
#					hydra:variable "episode"^^xsd:string;
#					rdfs:range "xsd:string";
#					rdfs:label "Episode dataset contains: seismic data: Catalog, Event related waveforms, Seismic Network; industrial data: Fracking Process Parameters, Well Path, Well Position; geodata: Velocity Model. From 1997-05-12 till 1997-05-16. Additional configuration and filtration possible on the IS-EPOS Platform - please select the 'Download' button.";
#					schema:defaultValue "COTTON_VALLEY";
#					http:paramValue "COTTON_VALLEY" ;
#					hydra:required "true"^^xsd:boolean;
#				];
#		] ;
#. 
	<anthropogenic_hazards/webservice/is-epos_platform/episode-elements/VOUGLANS> a hydra:Operation;
		hydra:method "GET"^^xsd:string;
		hydra:returns "application/json";
		hydra:property[ a hydra:IriTemplate;
			hydra:template "https://tcs.ah-epos.eu/api/epos/episodes/{episode}"^^xsd:string;
				hydra:mapping[ a hydra:IriTemplateMapping;
					hydra:variable "episode"^^xsd:string;
					rdfs:range "xsd:string";
					rdfs:label "Episode dataset contains: seismic data: Catalog; industrial data: Shoreline, Water Height. From 1977-09-21 till 2009-12-30. Additional configuration and filtration possible on the IS-EPOS Platform - please select the 'Download' button.";
					schema:defaultValue "VOUGLANS";
					http:paramValue "VOUGLANS" ;
					hydra:required "true"^^xsd:boolean;
				];
		] ;
. 
	<anthropogenic_hazards/webservice/is-epos_platform/episode-elements/GAZLI> a hydra:Operation;
		hydra:method "GET"^^xsd:string;
		hydra:returns "application/json";
		hydra:property[ a hydra:IriTemplate;
			hydra:template "https://tcs.ah-epos.eu/api/epos/episodes/{episode}"^^xsd:string;
				hydra:mapping[ a hydra:IriTemplateMapping;
					hydra:variable "episode"^^xsd:string;
					rdfs:range "xsd:string";
					rdfs:label "Episode dataset contains: seismic data: Catalog; industrial data: Horizon Pressure, Hydrocarbon Field Area, Injected Gas Volume, Natural Gas Production; geodata: Locall cross sections. From 1978-12-31 till 2018-12-31. Additional configuration and filtration possible on the IS-EPOS Platform - please select the 'Download' button.";
					schema:defaultValue "GAZLI";
					http:paramValue "GAZLI" ;
					hydra:required "true"^^xsd:boolean;
				];
		] ;
. 
	<anthropogenic_hazards/webservice/is-epos_platform/episode-elements/BOGDANKA> a hydra:Operation;
		hydra:method "GET"^^xsd:string;
		hydra:returns "application/json";
		hydra:property[ a hydra:IriTemplate;
			hydra:template "https://tcs.ah-epos.eu/api/epos/episodes/{episode}"^^xsd:string;
				hydra:mapping[ a hydra:IriTemplateMapping;
					hydra:variable "episode"^^xsd:string;
					rdfs:range "xsd:string";
					rdfs:label "Episode dataset contains: seismic data: Catalog, Event related waveforms, Seismic Network; industrial data: Mine Area; geodata: Velocity Model. From 2018-07-03 till now. Additional configuration and filtration possible on the IS-EPOS Platform - please select the 'Download' button.";
					schema:defaultValue "BOGDANKA";
					http:paramValue "BOGDANKA" ;
					hydra:required "true"^^xsd:boolean;
				];
		] ;
. 


	<anthropogenic_hazards/distribution/episodes> a dcat:Distribution;
		dct:identifier "anthropogenic_hazards/distribution/episodes";
		dct:title "List of episodes";
		dct:description "The IS-EPOS Platform integrates research infrastructure of EPOS TCS AH (https://tcs.ah-epos.eu/). It provides access to Episodes, which are collections of time-correlated geophysical, technological and other relevant geodata, relating comprehensively anthropogenic seismicity to its industrial cause." ; 
		dct:type "http://publications.europa.eu/resource/authority/distribution-type/WEB_SERVICE"^^xsd:anyURI;
		dct:conformsTo <anthropogenic_hazards/webservice/is-epos_platform> ;
		dcat:accessURL <anthropogenic_hazards/webservice/is-epos_platform/episodes>;
		dct:format "http://publications.europa.eu/resource/authority/file-type/JSON"^^xsd:anyURI;
		dct:license "https://creativecommons.org/licenses/by/4.0/"^^xsd:anyURI;
.
	<anthropogenic_hazards/distribution/apps> a dcat:Distribution;
		dct:identifier "anthropogenic_hazards/distribution/apps";
		dct:title "List of applications";
		dct:description "The IS-EPOS Platform integrates research infrastructure of EPOS TCS AH (https://tcs.ah-epos.eu/). It provides access to applications, which are software tools to process and analyze the data. They can be used to relate seismicity and technological factors for hazard assessment and other scientific purposes."; 
		dct:type "http://publications.europa.eu/resource/authority/distribution-type/WEB_SERVICE"^^xsd:anyURI;
		dct:conformsTo <anthropogenic_hazards/webservice/is-epos_platform> ;
		dcat:accessURL <anthropogenic_hazards/webservice/is-epos_platform/apps>;
		dct:format "http://publications.europa.eu/resource/authority/file-type/JSON"^^xsd:anyURI;
		dct:license "https://creativecommons.org/licenses/by/4.0/"^^xsd:anyURI;
.
	<anthropogenic_hazards/distribution/episode-elements/CZORSZTYN> a dcat:Distribution;
		dct:identifier "anthropogenic_hazards/distribution/episode-elements/CZORSZTYN";
		dct:title "Episode CZORSZTYN: shallow water reservoir - dataset";
		dct:description "Enables to list data items contained in the episode (dataset) as ‘Catalog', 'Seismic Network', 'Event related waveforms', 'Velocity model' and some 'Industrial data', features filtering. Episode comprehensively describes a geophysical process induced or triggered by human technological activity, which could pose a hazard for populations, infrastructure and environment. Seismic activity is linked to the impoundment of Czorsztyn artificial lake. The lake was created by backing up water by an earth dam of the hydropower plant Niedzica on Dunajec river in south of Poland. Its filling ended in 1997. The reservoir of 234.5 milion cubic meters capacity is shallow, on average between 20 to 50 m of water column. Seismic activity began in 2011. "; 
		dct:type "http://publications.europa.eu/resource/authority/distribution-type/WEB_SERVICE"^^xsd:anyURI;
		dct:conformsTo <anthropogenic_hazards/webservice/is-epos_platform> ;
		dcat:accessURL <anthropogenic_hazards/webservice/is-epos_platform/episode-elements/CZORSZTYN>;
		dct:format "http://publications.europa.eu/resource/authority/file-type/JSON"^^xsd:anyURI;
		dct:license "https://creativecommons.org/licenses/by/4.0/"^^xsd:anyURI;
. 
	<anthropogenic_hazards/distribution/episode-elements/GS> a dcat:Distribution;
		dct:identifier "anthropogenic_hazards/distribution/episode-elements/GS";
		dct:title "Episode GROSS SCHOENEBECK: geothermal energy production experiment - dataset";
		dct:description "Enables to list data items contained in the episode (dataset) as ‘Catalog', 'Seismic Network', 'Event related waveforms', 'Velocity model' and some 'Industrial data', features filtering. Episode comprehensively describes a geophysical process induced or triggered by human technological activity, which could pose a hazard for populations, infrastructure and environment. A deep injection well and a doublet of production wells were established in this area reaching the reservoir rocks like red bed sandstone and andesitic volcanic rock at the 4200m depth. Injection performed from 9th to 14th August 2007 was used for repeated stimulation treatments to investigate scenarios of enhancing productivity of thermal fluid recovery from the underground. A total amount of 13.000 m^3 of water was injected. The maximum injection well-head pressure reached 58.6 MPa."; 
		dct:type "http://publications.europa.eu/resource/authority/distribution-type/WEB_SERVICE"^^xsd:anyURI;
		dct:conformsTo <anthropogenic_hazards/webservice/is-epos_platform> ;
		dcat:accessURL <anthropogenic_hazards/webservice/is-epos_platform/episode-elements/GS>;
		dct:format "http://publications.europa.eu/resource/authority/file-type/JSON"^^xsd:anyURI;
		dct:license "https://creativecommons.org/licenses/by/4.0/"^^xsd:anyURI;
.
	<anthropogenic_hazards/distribution/episode-elements/LGCD> a dcat:Distribution;
		dct:identifier "anthropogenic_hazards/distribution/episode-elements/LGCD";
		dct:title "Episode LGCD: regional seismicity and ground motion associating underground hard rock mining - dataset";
		dct:description "Enables to list data items contained in the episode (dataset) as ‘Catalog','Ground Motion Catalog ', 'Seismic Network','Ground Motion Network', 'Event related waveforms', 'Velocity model' and some 'Industrial data', features filtering. Episode comprehensively describes a geophysical process; induced or triggered by human technological activity, which could pose a hazard for populations, infrastructure and environment. The LGCD episode describes the seismicity induced by underground copper ore exploitation in mines located in the Legnica-Glogow Copper District (LGCD), southwestern Poland. The room and pillar exploitation system is used in the mines at the level from 0.6 to 1.3 km below surface. Episode LGCD contains only seismic events recorded inside the seismic network."; 
		dct:type "http://publications.europa.eu/resource/authority/distribution-type/WEB_SERVICE"^^xsd:anyURI;
		dct:conformsTo <anthropogenic_hazards/webservice/is-epos_platform> ;
		dcat:accessURL <anthropogenic_hazards/webservice/is-epos_platform/episode-elements/LGCD>;
		dct:format "http://publications.europa.eu/resource/authority/file-type/JSON"^^xsd:anyURI;
		dct:license "https://creativecommons.org/licenses/by/4.0/"^^xsd:anyURI;
.
	<anthropogenic_hazards/distribution/episode-elements/SONG_TRANH> a dcat:Distribution;
		dct:identifier "anthropogenic_hazards/distribution/episode-elements/SONG_TRANH";
		dct:title "Episode SONG TRANH: deep water reservoir - dataset";
		dct:description "Enables to list data items contained in the episode (dataset) as ‘Catalog', 'Seismic Network', 'Event related waveforms', 'Velocity model' and some 'Industrial data', features filtering. Episode comprehensively describes a geophysical process induced or triggered by human technological activity, which could pose a hazard for populations, infrastructure and environment. Seismic activity decribed in this episode is linked to Song Tranh 2 hydropower plant and the reservoir containing backed up water of Tranh river in central Vietnam. The reservoir volume is 740 million cubic meters and the water level varies between 140 and 175 m. Seismic activity in the reservoir region, previously known as aseismic, began in 2011, soon after filling of the reservoir."; 
		dct:type "http://publications.europa.eu/resource/authority/distribution-type/WEB_SERVICE"^^xsd:anyURI;
		dct:conformsTo <anthropogenic_hazards/webservice/is-epos_platform> ;
		dcat:accessURL <anthropogenic_hazards/webservice/is-epos_platform/episode-elements/SONG_TRANH>;
		dct:format "http://publications.europa.eu/resource/authority/file-type/JSON"^^xsd:anyURI;
		dct:license "https://creativecommons.org/licenses/by/4.0/"^^xsd:anyURI;
.
	<anthropogenic_hazards/distribution/episode-elements/USCB> a dcat:Distribution;
		dct:identifier "anthropogenic_hazards/distribution/episode-elements/USCB";
		dct:title "Episode USCB: regional seismicity and ground motion associating underground coal mining - dataset";
		dct:description "Enables to list data items contained in the episode (dataset) as ‘Catalog', 'Ground Motion Catalog', 'Seismic Network', 'Ground Motion Network','Event related waveforms', 'Velocity model', 'Faults' and some 'Industrial data', features filtering. Episode comprehensively describes a geophysical process induced or triggered by human technological activity, which could pose a hazard for populations, infrastructure and environment. Seismic activity is linked to underground coal mining in Upper Silesia Coal Basin (USCB) in Poland. Multilevel mine operations have been conducted for more than 200 years. Presently (2016), there are more than 20 seismically active mines."; 
		dct:type "http://publications.europa.eu/resource/authority/distribution-type/WEB_SERVICE"^^xsd:anyURI;
		dct:conformsTo <anthropogenic_hazards/webservice/is-epos_platform> ;
		dcat:accessURL <anthropogenic_hazards/webservice/is-epos_platform/episode-elements/USCB>;
		dct:format "http://publications.europa.eu/resource/authority/file-type/JSON"^^xsd:anyURI;
		dct:license "https://creativecommons.org/licenses/by/4.0/"^^xsd:anyURI;
.
	<anthropogenic_hazards/distribution/episode-elements/BOBREK> a dcat:Distribution;
		dct:identifier "anthropogenic_hazards/distribution/episode-elements/BOBREK";
		dct:title "Episode BOBREK MINE: local seismicity linked to longwall mining - dataset";
		dct:description "Enables to list data items contained in the episode (dataset) as ‘Catalog', 'Seismic Network', 'Event related waveforms', 'Velocity model' and some 'Industrial data', features filtering. Episode comprehensively describes a geophysical process induced or triggered by human technological activity, which could pose a hazard for populations, infrastructure and environment. Bobrek Mine local seismicity is linked to longwall mining. The mine forms the Laboratory for Monitoring Mining Induced Seismicity (LMMIS) of passive seismic records of seismicity induced and triggered by underground coal mining. The episode is related to seismic activity linked to longwall mining of panel 3 in coal seam 503 in Bobrek colliery in Upper Silesia Coal Basin in Poland. The coal seam no. 503 was 3.0 to 3.5 m thick in the area of longwall panel no. 3 and at the depth of 700 m below surface. The coal extraction was carried on during the period 1/04/2009-8/07/2010."; 
		dct:type "http://publications.europa.eu/resource/authority/distribution-type/WEB_SERVICE"^^xsd:anyURI;
		dct:conformsTo <anthropogenic_hazards/webservice/is-epos_platform> ;
		dcat:accessURL <anthropogenic_hazards/webservice/is-epos_platform/episode-elements/BOBREK>;
		dct:format "http://publications.europa.eu/resource/authority/file-type/JSON"^^xsd:anyURI;
		dct:license "https://creativecommons.org/licenses/by/4.0/"^^xsd:anyURI;
.
	<anthropogenic_hazards/distribution/episode-elements/PYHASALMI_MINE> a dcat:Distribution;
		dct:identifier "anthropogenic_hazards/distribution/episode-elements/PYHASALMI_MINE";
		dct:title "Episode PYHASALMI MINE: in situ underground laboratory - dataset";
		dct:description "Enables to list data items contained in the episode (dataset) as ‘Catalog', 'Seismic Network', 'Event related waveforms', 'Velocity model' and some 'Industrial data', features filtering. Episode comprehensively describes a geophysical process induced or triggered by human technological activity, which could pose a hazard for populations, infrastructure and environment. Pyhasalmi mine, Central Finland, is an underground mine which produces copper, zinc and pyrite. A seismic network was installed underground in 2002 to monitor and locate frequently occurring microseismic scale events. Main target in Pyhasalmi episode is to: 1. Compare microseismic networks detected events with observations with national permanent seismic stations observations. 2. Correlate mining related microseismic events with the production data of the Pyhasalmi mine. 3. Analyze regions, where events concentrate and compare the locations with known geology. Pyhasalmi Episode consists of various data in order to track relation between seismicity and Pyhasalmi mine production. Data consists of seismic waverform and catalog, borehole information and basemaps."; 
		dct:type "http://publications.europa.eu/resource/authority/distribution-type/WEB_SERVICE"^^xsd:anyURI;
		dct:conformsTo <anthropogenic_hazards/webservice/is-epos_platform> ;
		dcat:accessURL <anthropogenic_hazards/webservice/is-epos_platform/episode-elements/PYHASALMI_MINE>;
		dct:format "http://publications.europa.eu/resource/authority/file-type/JSON"^^xsd:anyURI;
		dct:license "https://creativecommons.org/licenses/by/4.0/"^^xsd:anyURI;
.
	<anthropogenic_hazards/distribution/episode-elements/LGF> a dcat:Distribution;
		dct:identifier "anthropogenic_hazards/distribution/episode-elements/LGF";
		dct:title "Episode LACQ GAS FIELD: conventional hydrocarbon extraction - dataset";
		dct:description "Enables to list data items contained in the episode (dataset) as ‘Catalog', 'Seismic Network', 'Velocity model' and some 'Industrial data', features filtering. Episode comprehensively describes a geophysical process induced or triggered by human technological activity, which could pose a hazard for populations, infrastructure and environment. The LACQ GAS FIELD episode is related to a seismic swarm that developed contemporary to and in the vicinity of a deep conventional gas extraction field (Aquitaine, France). Onset of Lacq gas field production took place in 1958, whereas the first local M3 event occurred in 1969. Since that time, hundreds of shallow, small to moderate magnitude earthquakes (Mmax=4) have occurred near the Lacq deep gas field. These earthquakes are clearly separated from tectonic seismicity occurring in the Pyrenees, 25 km to the southwest. The induced seismicity began when the reservoir pressure had declined by 30 MPa. Repeated leveling over the field shows localized subsidence reaching a maximum of 60 mm in 1989. Episode data includes (i) regional seismicity catalogue for the 1962-2009 period, local catalogue for the 1975-1995 period; (ii) yearly production volumes, 1958-2016; (iii) yearly reservoir pressure drop, 1958-2016; (iv) yearly injected volume, 1958-2016."; 
		dct:type "http://publications.europa.eu/resource/authority/distribution-type/WEB_SERVICE"^^xsd:anyURI;
		dct:conformsTo <anthropogenic_hazards/webservice/is-epos_platform> ;
		dcat:accessURL <anthropogenic_hazards/webservice/is-epos_platform/episode-elements/LGF>;
		dct:format "http://publications.europa.eu/resource/authority/file-type/JSON"^^xsd:anyURI;
		dct:license "https://creativecommons.org/licenses/by/4.0/"^^xsd:anyURI;
.
	<anthropogenic_hazards/distribution/episode-elements/MONTEYNARD> a dcat:Distribution;
		dct:identifier "anthropogenic_hazards/distribution/episode-elements/MONTEYNARD";
		dct:title "Episode MONTEYNARD: water reservoir - dataset";
		dct:description "Enables to list data items contained in the episode (dataset) as ‘Catalog' and some 'Industrial data', features filtering. Episode comprehensively describes a geophysical process induced or triggered by human technological activity, which could pose a hazard for populations, infrastructure and environment. The episode describes the seismicity sequence around Monteynard dam, caused by reservoir impoundment in France. The seismic sequence, April 1962, M=5.5, April 1963, M=4.9, November 1979, M=4.5 is located is the near field of the reservoir, i.e. within 1-3 reservoir lake lengths. Monteynard reservoir situated in moderate activity seismic zone of western Alps. Initially within first few years, six earthquakes (ML higher than 3.5) occurred in quick succession in close vicinity of the reservoir (less than 15 km) thereby supporting the hypothesis of reservoir induced earthquakes at Monteynard. The first significant earthquake (M5.2) occurred near the reservoir when the reservoir was only one third full (40 m deep). The two other earthquakes (ML bigger than 4.5) in 1963 and 1979 occurred when the reservoir level peaked to its maximum value (115 m). The episode data correspond to (i) seismicity catalogues (1962,2009) around the reservoir up to a 10L distance to reservoir (L being the reservoir lake length). The users can select catalogue for seismicity either in 1L or 3L or 10L distance to lake reservoir; (ii) Yearly values for reservoir lake level are provided on the 1961-1992 period as mean, maximum and minimum values; monthly values being only available on the 1961-1964 period."; 
		dct:type "http://publications.europa.eu/resource/authority/distribution-type/WEB_SERVICE"^^xsd:anyURI;
		dct:conformsTo <anthropogenic_hazards/webservice/is-epos_platform> ;
		dcat:accessURL <anthropogenic_hazards/webservice/is-epos_platform/episode-elements/MONTEYNARD>;
		dct:format "http://publications.europa.eu/resource/authority/file-type/JSON"^^xsd:anyURI;
		dct:license "https://creativecommons.org/licenses/by/4.0/"^^xsd:anyURI;
.
	<anthropogenic_hazards/distribution/episode-elements/SSFS1993> a dcat:Distribution;
		dct:identifier "anthropogenic_hazards/distribution/episode-elements/SSFS1993";
		dct:title "Episode SOULTZ-SOUS-FORETS 1993 STIMULATION - dataset";
		dct:description "Enables to list data items contained in the episode (dataset) as ‘Catalog', 'Seismic Stations', 'Event related waveforms', 'Velocity model' and some 'Industrial data', features filtering. Episode comprehensively describes a geophysical process induced or triggered by human technological activity, which could pose a hazard for populations, infrastructure and environment. In 1993, during the development of the european enhanced geothermal system of Soultz-sous-Forêts (Alsace), 44000 m3 of water were injected to create the reservoir by stimulating the natural fracture system of the granitic rock mass. Some 16000 microseismic events were recorded by a network consisting of a hydrophone and 3 four-component accelerometers, cemented in the granite at the bottom of observation wells."; 
		dct:type "http://publications.europa.eu/resource/authority/distribution-type/WEB_SERVICE"^^xsd:anyURI;
		dct:conformsTo <anthropogenic_hazards/webservice/is-epos_platform> ;
		dcat:accessURL <anthropogenic_hazards/webservice/is-epos_platform/episode-elements/SSFS1993>;
		dct:format "http://publications.europa.eu/resource/authority/file-type/JSON"^^xsd:anyURI;
		dct:license "https://creativecommons.org/licenses/by/4.0/"^^xsd:anyURI;
. 
	<anthropogenic_hazards/distribution/episode-elements/SSFS2000> a dcat:Distribution;
		dct:identifier "anthropogenic_hazards/distribution/episode-elements/SSFS2000";
		dct:title "Episode SOULTZ-SOUS-FORETS 2000 STIMULATION - dataset";
		dct:description "Enables to list data items contained in the episode (dataset) as 'Catalog', 'Seismic Stations' and some 'Industrial data', features filtering. Episode comprehensively describes a geophysical process induced or triggered by human technological activity, which could pose a hazard for populations, infrastructure and environment. During June/July 2000 a hydraulic stimulation program was conducted in the well GPK2. The stimulation was performed over the open hole section of GPK2 from 4431 m (measured depth) to the bottom of the well at around 5084 m. A total of 27 800 m3 of water were injected. At the start of the stimulation 700m3 of brine were injected in an effort to encourage downward growth of the stimulated region. The stimulation covered a period of six days. After a break of seven days a post-stimulation injection test was performed. Microseismic emissions were monitored and recorded throughout the experiment and continued for 11 more days after the injection test."; 
		dct:type "http://publications.europa.eu/resource/authority/distribution-type/WEB_SERVICE"^^xsd:anyURI;
		dct:conformsTo <anthropogenic_hazards/webservice/is-epos_platform> ;
		dcat:accessURL <anthropogenic_hazards/webservice/is-epos_platform/episode-elements/SSFS2000>;
		dct:format "http://publications.europa.eu/resource/authority/file-type/JSON"^^xsd:anyURI;
		dct:license "https://creativecommons.org/licenses/by/4.0/"^^xsd:anyURI;
. 
	<anthropogenic_hazards/distribution/episode-elements/SSFS2003> a dcat:Distribution;
		dct:identifier "anthropogenic_hazards/distribution/episode-elements/SSFS2003";
		dct:title "Episode SOULTZ-SOUS-FORETS 2003 STIMULATION - dataset";
		dct:description "Enables to list data items contained in the episode (dataset) as  'Catalog', 'Seismic Stations' and some 'Industrial data', features filtering. Episode comprehensively describes a geophysical process induced or triggered by human technological activity, which could pose a hazard for populations, infrastructure and environment. The stimulation was performed in 2003 mainly by massive injection into the well GPK3. The stimulation strategy can be divided in five parts: - Injection into GPK3 - Injection into both GPK2 and GPK3 (“dual” or “focused” stimulation, Baria et al., 2004) - Shut in GPK2 - Shut in both GPK2 and GPK3 and production from GPK2 - Circulation test GPK2-GPK3 following stimulation."; 
		dct:type "http://publications.europa.eu/resource/authority/distribution-type/WEB_SERVICE"^^xsd:anyURI;
		dct:conformsTo <anthropogenic_hazards/webservice/is-epos_platform> ;
		dcat:accessURL <anthropogenic_hazards/webservice/is-epos_platform/episode-elements/SSFS2003>;
		dct:format "http://publications.europa.eu/resource/authority/file-type/JSON"^^xsd:anyURI;
		dct:license "https://creativecommons.org/licenses/by/4.0/"^^xsd:anyURI;
.
	<anthropogenic_hazards/distribution/episode-elements/SSFS2004> a dcat:Distribution;
		dct:identifier "anthropogenic_hazards/distribution/episode-elements/SSFS2004";
		dct:title "Episode SOULTZ-SOUS-FORETS 2004 STIMULATION - dataset";
		dct:description "Enables to list data items contained in the episode (dataset) as 'Catalog', 'Seismic Stations' and some 'Industrial data', features filtering. Episode comprehensively describes a geophysical process induced or triggered by human technological activity, which could pose a hazard for populations, infrastructure and environment. The 2004 stimulation was aimed at improving the hydraulic performances of the well GPK4. This borehole was stimulated twice. The present test corresponds to the first stimulation of GPK4. The data from a pre-stimulation low flow injection test performed to evaluate the initial injectivity of GPK4 are included."; 
		dct:type "http://publications.europa.eu/resource/authority/distribution-type/WEB_SERVICE"^^xsd:anyURI;
		dct:conformsTo <anthropogenic_hazards/webservice/is-epos_platform> ;
		dcat:accessURL <anthropogenic_hazards/webservice/is-epos_platform/episode-elements/SSFS2004>;
		dct:format "http://publications.europa.eu/resource/authority/file-type/JSON"^^xsd:anyURI;
		dct:license "https://creativecommons.org/licenses/by/4.0/"^^xsd:anyURI;
. 
	<anthropogenic_hazards/distribution/episode-elements/SSFS2005> a dcat:Distribution;
		dct:identifier "anthropogenic_hazards/distribution/episode-elements/SSFS2005";
		dct:title "Episode SOULTZ-SOUS-FORETS 2005 STIMULATION - dataset";
		dct:description "Enables to list data items contained in the episode (dataset) as  'Catalog', 'Seismic Stations' and some 'Industrial data', features filtering. Episode comprehensively describes a geophysical process induced or triggered by human technological activity, which could pose a hazard for populations, infrastructure and environment. The 2005 stimulation is the second stimulation of GPK4, after the previous one, performed in September 2004. The stimulation was followed a few days later by a program of chemical stimulation (injection of diluted HCl). This program involved the chemical stimulation itself and two identical step-rate injection tests: the first was performed before the chemical stimulation and the second after, in order to observe the efficiency of the chemical stimulation. The program was in the following order: - Second hydraulic stimulation of GPK4 - First step-rate test - Chemical stimulation of GPK4 with HCl - Second step-rate test."; 
		dct:type "http://publications.europa.eu/resource/authority/distribution-type/WEB_SERVICE"^^xsd:anyURI;
		dct:conformsTo <anthropogenic_hazards/webservice/is-epos_platform> ;
		dcat:accessURL <anthropogenic_hazards/webservice/is-epos_platform/episode-elements/SSFS2005>;
		dct:format "http://publications.europa.eu/resource/authority/file-type/JSON"^^xsd:anyURI;
		dct:license "https://creativecommons.org/licenses/by/4.0/"^^xsd:anyURI;
.
	<anthropogenic_hazards/distribution/episode-elements/GISOS-CERVILLE> a dcat:Distribution;
		dct:identifier "anthropogenic_hazards/distribution/episode-elements/GISOS-CERVILLE";
		dct:title "Episode GISOS-CERVILLE: underground solution mining - dataset";
		dct:description "Enables to list data items contained in the episode (dataset) as ‘Catalog', 'Seismic Network', 'Event related waveforms', 'Velocity model' and some 'Industrial data', features filtering. Episode comprehensively describes a geophysical process induced or triggered by human technological activity, which could pose a hazard for populations, infrastructure and environment. Ground failures, caving processes and collapses of large natural or man-made underground cavities can produce significant socio-economic damages and represent a serious risk envisaged by the stakeholders and municipalities. In order to improve our understanding of the mechanisms governing such a geohazard and to test the potential of geophysical methods to prevent them, the development and collapse of a salt solution mining cavity (channel and drilling exploitation technique) was monitored. This experiment was conducted by the research “Groupement d’Intérêt Scientifique sur l’impact et la Sécurité des Ouvrages Souterrains” (GISOS), at the SOLVAY exploitation site of Cerville-Buissoncourt (Lorraine basin, France). During the experiment, ten thousands seismic events were recorded by a local high frequency microseismic network, installed by INERIS, which provides a unique opportunity to study in detail the microseismic response of a caving and collapsing underground cavity. In addition, several geotechnical measurements such as GPS, extensometer have been perfomed to measure local insitu deformation and to visualize the evolving cavity structure from sonar campaign."; 
		dct:type "http://publications.europa.eu/resource/authority/distribution-type/WEB_SERVICE"^^xsd:anyURI;
		dct:conformsTo <anthropogenic_hazards/webservice/is-epos_platform> ;
		dcat:accessURL <anthropogenic_hazards/webservice/is-epos_platform/episode-elements/GISOS-CERVILLE>;
		dct:format "http://publications.europa.eu/resource/authority/file-type/JSON"^^xsd:anyURI;
		dct:license "https://creativecommons.org/licenses/by/4.0/"^^xsd:anyURI;
.
	<anthropogenic_hazards/distribution/episode-elements/STARFISH> a dcat:Distribution;
		dct:identifier "anthropogenic_hazards/distribution/episode-elements/STARFISH";
		dct:title "Episode STARFISH: underground gas storage - dataset";
		dct:description "Enables to list data items contained in the episode (dataset) as ‘Catalog', 'Seismic Network', 'Event related waveforms' and some 'Industrial data', features filtering. Episode comprehensively describes a geophysical process induced or triggered by human technological activity, which could pose a hazard for populations, infrastructure and environment. An experiment was undertaken in an underground salt mine to assess the influence of thermal loading of high-frequency gas storage operations cycles on the stability of salt cavities. A footwall salt block was exposed to repetitive rapid cooling cycles while its thermo-mechanical and acoustic response was recorded by multi-parameter geotechnical monitoring approach performed by different project partners (SMRI, BGR, Ecole de mines Paris). The cooling system allowed cooling with maximum temperature drops of 25 °C. Data of this episode was recorded by a multi parameter monitoring system set up by INERIS, comprising 16 high-resolution acoustic sensors, thermal sensors as well as strain cells, at different depths. Results of data analysis indicate that the nature of the first cooling cycle seems to be a crucial factor for the following mechanical behavior of salt rocks to successive cooling cycles."; 
		dct:type "http://publications.europa.eu/resource/authority/distribution-type/WEB_SERVICE"^^xsd:anyURI;
		dct:conformsTo <anthropogenic_hazards/webservice/is-epos_platform> ;
		dcat:accessURL <anthropogenic_hazards/webservice/is-epos_platform/episode-elements/STARFISH>;
		dct:format "http://publications.europa.eu/resource/authority/file-type/JSON"^^xsd:anyURI;
		dct:license "https://creativecommons.org/licenses/by/4.0/"^^xsd:anyURI;
.
	<anthropogenic_hazards/distribution/episode-elements/THE_GEYSERS_Prati_9_and_Prati_29_cluster> a dcat:Distribution;
		dct:identifier "anthropogenic_hazards/distribution/episode-elements/THE_GEYSERS_Prati_9_and_Prati_29_cluster";
		dct:title "Episode THE GEYSERS Prati 9 and Prati 29 cluster: Treated wastewater injection for geothermal power production - dataset";
		dct:description "Enables to list data items contained in the episode (dataset) as ‘Catalog' and some 'Industrial data', features filtering. Episode comprehensively describes a geophysical process induced or triggered by human technological activity, which could pose a hazard for populations, infrastructure and environment. The Geysers is the world's largest geothermal (hydrothermal) field located 116km north of San Francisco, California. The injection of treated wastewater leads to occurrence of significant seismic activity with thousands of earthquakes above the magnitude of completeness of 1.4 occurring every year. This episode contains high quality seismic catalogs and other associated data from a cluster of seismicity related to fluid injection in the vicinity of Prati 9 and Prati 29 injection wells located in the north-western part of the field. The first catalog contains source parameters (including high quality static stress drop) estimated using mesh spectral ratio technique. The second catalog contains refined focal mechanism derived using HASH software. The catalog data are accompanied by technological data (injection rates) as well as supplementary information (well traces)."; 
		dct:type "http://publications.europa.eu/resource/authority/distribution-type/WEB_SERVICE"^^xsd:anyURI;
		dct:conformsTo <anthropogenic_hazards/webservice/is-epos_platform> ;
		dcat:accessURL <anthropogenic_hazards/webservice/is-epos_platform/episode-elements/THE_GEYSERS_Prati_9_and_Prati_29_cluster>;
		dct:format "http://publications.europa.eu/resource/authority/file-type/JSON"^^xsd:anyURI;
		dct:license "https://creativecommons.org/licenses/by/4.0/"^^xsd:anyURI;
.
	<anthropogenic_hazards/distribution/episode-elements/THE_GEYSERS> a dcat:Distribution;
		dct:identifier "anthropogenic_hazards/distribution/episode-elements/THE_GEYSERS";
		dct:title "Episode THE GEYSERS: geothermal energy production - dataset";
		dct:description "Enables to list data items contained in the episode (dataset) as ‘Catalog', 'Seismic Network', 'Ground Motion Network', 'Event related waveforms', 'Faults' and some 'Industrial data', features filtering. Episode comprehensively describes a geophysical process induced or triggered by human technological activity, which could pose a hazard for populations, infrastructure and environment. The Geysers geothermal field is one of the largest geothermal fields worldwide in terms of steam production. The Geysers is a vapor-dominated reservoir, located 116km north of San Francisco, California. It has been in operation for more than 50 years resulting in the occurrence of several hundred thousand induced seismic events. Over the years, field exploitation resulted in a long-term reduction of reservoir pressure and a decrease in steam production. Episode consists of various data describing the seismicity connected with fluid injection at this geothermal site. The seismicity data are accompanied by technological data (injection volumes, steam production) as well as supplementary information (well positions and location of power plants)."; 
		dct:type "http://publications.europa.eu/resource/authority/distribution-type/WEB_SERVICE"^^xsd:anyURI;
		dct:conformsTo <anthropogenic_hazards/webservice/is-epos_platform> ;
		dcat:accessURL <anthropogenic_hazards/webservice/is-epos_platform/episode-elements/THE_GEYSERS>;
		dct:format "http://publications.europa.eu/resource/authority/file-type/JSON"^^xsd:anyURI;
		dct:license "https://creativecommons.org/licenses/by/4.0/"^^xsd:anyURI;
.
	<anthropogenic_hazards/distribution/episode-elements/VDF> a dcat:Distribution;
		dct:identifier "anthropogenic_hazards/distribution/episode-elements/VDF";
		dct:title "Episode VAL D'AGRI FIELD: conventional hydrocarbon extraction - dataset";
		dct:description "Enables to list data items contained in the episode (dataset) as ‘Catalog', 'Seismic Network', 'Event related waveforms', 'Velocity model' and some 'Industrial data', features filtering. Episode comprehensively describes a geophysical process induced or triggered by human technological activity, which could pose a hazard for populations, infrastructure and environment. This episode describes seismic monitoring of the initial stage of wastewater injection into a disposal well of the Val d'Agri oil field. The monitoring unraveled a low magnitude swarm induced by disposal operations that initiated just a few hours after the beginning of injection. Main objective is to provide seismic data to be analyzed with advanced techniques for a better understanding of the mechanisms of injection-linked seismicity and of physical properties of the reservoir."; 
		dct:type "http://publications.europa.eu/resource/authority/distribution-type/WEB_SERVICE"^^xsd:anyURI;
		dct:conformsTo <anthropogenic_hazards/webservice/is-epos_platform> ;
		dcat:accessURL <anthropogenic_hazards/webservice/is-epos_platform/episode-elements/VDF>;
		dct:format "http://publications.europa.eu/resource/authority/file-type/JSON"^^xsd:anyURI;
		dct:license "https://creativecommons.org/licenses/by/4.0/"^^xsd:anyURI;
.
	<anthropogenic_hazards/distribution/episode-elements/VD> a dcat:Distribution;
		dct:identifier "anthropogenic_hazards/distribution/episode-elements/VD";
		dct:title "Episode VAL D'AGRI: water reservoir - dataset";
		dct:description "Enables to list data items contained in the episode (dataset) as ‘Catalog', 'Seismic Network', 'Event related waveforms', 'Velocity model' and some 'Industrial data', features filtering. Episode comprehensively describes a geophysical process induced or triggered by human technological activity, which could pose a hazard for populations, infrastructure and environment. This episode describes low magnitude earthquakes recorded by an experiment-specific temporary network deployed around the Pertusillo Lake impoundment. During the one-year survey the network recorded an intense microseismicity that appears correlated in time and space to severe seasonal oscillations of the artificial lake. Main objective is to provide seismic data to be analyzed for a better understanding of the mechanisms of protracted RIS and of physical properties of the carbonate rocks where seismicity occurs."; 
		dct:type "http://publications.europa.eu/resource/authority/distribution-type/WEB_SERVICE"^^xsd:anyURI;
		dct:conformsTo <anthropogenic_hazards/webservice/is-epos_platform> ;
		dcat:accessURL <anthropogenic_hazards/webservice/is-epos_platform/episode-elements/VD>;
		dct:format "http://publications.europa.eu/resource/authority/file-type/JSON"^^xsd:anyURI;
		dct:license "https://creativecommons.org/licenses/by/4.0/"^^xsd:anyURI;
. 
# will be available July/August 2019
#	<anthropogenic_hazards/distribution/episode-elements/EMILIA_ROMAGNA> a dcat:Distribution;
#		dct:identifier "anthropogenic_hazards/distribution/episode-elements/EMILIA_ROMAGNA";
#		dct:title "Episode EMILIA ROMAGNA: cavone oil field - dataset";
#		dct:description "Enables to list data items contained in the episode (dataset) as 'Catalog' and some 'Industrial data', features filtering. Episode comprehensively describes a geophysical process induced or triggered by human technological activity, which could pose a hazard for populations, infrastructure and environment. Episode consists of various data describing the seismicity caused by conventional hydrocarbon extraction and fluid injection in Emilia Romagna, Italy."; 
#		dct:type "http://publications.europa.eu/resource/authority/distribution-type/WEB_SERVICE"^^xsd:anyURI;
#		dct:conformsTo <anthropogenic_hazards/webservice/is-epos_platform> ;
#		dcat:accessURL <anthropogenic_hazards/webservice/is-epos_platform/episode-elements/EMILIA_ROMAGNA>;
#		dct:format "http://publications.europa.eu/resource/authority/file-type/JSON"^^xsd:anyURI;
#		dct:license "https://creativecommons.org/licenses/by/4.0/"^^xsd:anyURI;
#.
	<anthropogenic_hazards/distribution/episode-elements/PREESE_HALL> a dcat:Distribution;
		dct:identifier "anthropogenic_hazards/distribution/episode-elements/PREESE_HALL";
		dct:title "Episode PREESE HALL: Shale Gas - dataset";
		dct:description "Enables to list data items contained in the episode (dataset) as ‘Catalog', 'Seismic Network', 'Velocity model' and some 'Industrial data', features filtering. Episode comprehensively describes a geophysical process induced or triggered by human technological activity, which could pose a hazard for populations, infrastructure and environment. An exploration well for shale gas was drilled into the Bowland Shale formation to a depth of 2.7 km. Hydrofracture stimulations were carried out at five depths. Felt earthquakes occurred during the stage 2 treatment."; 
		dct:type "http://publications.europa.eu/resource/authority/distribution-type/WEB_SERVICE"^^xsd:anyURI;
		dct:conformsTo <anthropogenic_hazards/webservice/is-epos_platform> ;
		dcat:accessURL <anthropogenic_hazards/webservice/is-epos_platform/episode-elements/PREESE_HALL>;
		dct:format "http://publications.europa.eu/resource/authority/file-type/JSON"^^xsd:anyURI;
		dct:license "https://creativecommons.org/licenses/by/4.0/"^^xsd:anyURI;
. 
	<anthropogenic_hazards/distribution/episode-elements/THORESBY_COLLIERY> a dcat:Distribution;
		dct:identifier "anthropogenic_hazards/distribution/episode-elements/THORESBY_COLLIERY";
		dct:title "Episode THORESBY COLLIERY: underground coal mining - dataset";
		dct:description "Enables to list data items contained in the episode (dataset) as ‘Catalog', 'Seismic Network', 'Event related waveforms', 'Velocity model' and some 'Industrial data', features filtering. Episode comprehensively describes a geophysical process induced or triggered by human technological activity, which could pose a hazard for populations, infrastructure and environment. Situated in the North of the Nottinghamshire Coalfield, Thoresby Colliery closed in 2015 and was the last deep coal mine in England's East Midlands. Production at the mine lasted over 90 years with the extraction of Middle Coal Measure seams at depths between 650m to 820m below ground level. Sherwood Sandstone (containing fissures at the surface presumed to be associated with mining) overlie the Middle Coal Measures and form the surface rock in the Thoresby Colliery area. Workings of the colliery extend beneath Thoresby Park near Edwinstowe where over 100 felt tremors were reported by the public between June 1989 and August 1990 and have since been associated with induced seismicity from the longwall mining of coal in the area (Bishop et al., 1993 and Styles et al., 1997 – references in episode repository). This episode contains microseismic monitoring data caused by the underground mining of coal at Thoresby Colliery between late 1996 and early 1997."; 
		dct:type "http://publications.europa.eu/resource/authority/distribution-type/WEB_SERVICE"^^xsd:anyURI;
		dct:conformsTo <anthropogenic_hazards/webservice/is-epos_platform> ;
		dcat:accessURL <anthropogenic_hazards/webservice/is-epos_platform/episode-elements/THORESBY_COLLIERY>;
		dct:format "http://publications.europa.eu/resource/authority/file-type/JSON"^^xsd:anyURI;
		dct:license "https://creativecommons.org/licenses/by/4.0/"^^xsd:anyURI;
. 
	<anthropogenic_hazards/distribution/episode-elements/ASFORDBY> a dcat:Distribution;
		dct:identifier "anthropogenic_hazards/distribution/episode-elements/ASFORDBY";
		dct:title "Episode ASFORDBY: underground coal mining - dataset";
		dct:description "Enables to list data items contained in the episode (dataset) as ‘Catalog', 'Seismic Network', 'Event related waveforms', 'Velocity model', ''Faults' and some 'Industrial data', features filtering. Episode comprehensively describes a geophysical process induced or triggered by human technological activity, which could pose a hazard for populations, infrastructure and environment. Asfordby mine (also referred to as the Asfordby Colliery or Asfordby Super-pit) is situated North East of the town of Melton Mowbray in the East Midlands County of Leicestershire, England. Coal Measures at Asfordby mine are part of the southerly extending South-East Nottinghamshire Carboniferous basin with the deep main seam occurring at depths of over 500m. Asfordby mine was the first and last modern deep mine to exploit the coalfield in the area. Coal production at the mine began in 1991 but was short lived with closure of the mine in 1997 following a damaging collapse at the mine and production issues linked to the geological complications of dolerite sills within the coal measures and from the overlying Sherwood sandstone aquifer."; 
		dct:type "http://publications.europa.eu/resource/authority/distribution-type/WEB_SERVICE"^^xsd:anyURI;
		dct:conformsTo <anthropogenic_hazards/webservice/is-epos_platform> ;
		dcat:accessURL <anthropogenic_hazards/webservice/is-epos_platform/episode-elements/ASFORDBY>;
		dct:format "http://publications.europa.eu/resource/authority/file-type/JSON"^^xsd:anyURI;
		dct:license "https://creativecommons.org/licenses/by/4.0/"^^xsd:anyURI;
. 
	<anthropogenic_hazards/distribution/episode-elements/NORTHWICH> a dcat:Distribution;
		dct:identifier "anthropogenic_hazards/distribution/episode-elements/NORTHWICH";
		dct:title "Episode NORTHWICH: underground salt extraction cavities - dataset";
		dct:description "Enables to list data items contained in the episode (dataset) as 'Seismic Network', 'Event related waveforms', 'Velocity model', 'Deformation Measurements' and some 'Industrial data', features filtering. Episode comprehensively describes a geophysical process induced or triggered by human technological activity, which could pose a hazard for populations, infrastructure and environment. Situated in Cheshire in the NW of England, Northwich overlies Triassic Halite beds that have been industrially and extensively mined for salt since the 17th century. As a result of poor early mining practices, combined with natural and anthropogenic salt dissolution, the area has suffered from mine void collapse and large scale catastrophic surface land subsidence. This episode contains long term microgravity data obtained for the detection and monitoring of voids, and time-lapse topography data for subsidence and ground deformation records. Both datasets are from a section of the Trent and Mersey Canal that has been severely affected by subsidence and the episode is supplemented with mine plans of the area along with details of a seismic network situated to the south of the monitored canal section. A 2012 paper detailing 10 years of monitoring + canal topography data is also available."; 
		dct:type "http://publications.europa.eu/resource/authority/distribution-type/WEB_SERVICE"^^xsd:anyURI;
		dct:conformsTo <anthropogenic_hazards/webservice/is-epos_platform> ;
		dcat:accessURL <anthropogenic_hazards/webservice/is-epos_platform/episode-elements/NORTHWICH>;
		dct:format "http://publications.europa.eu/resource/authority/file-type/JSON"^^xsd:anyURI;
		dct:license "https://creativecommons.org/licenses/by/4.0/"^^xsd:anyURI;
.
	<anthropogenic_hazards/distribution/episode-elements/OK> a dcat:Distribution;
		dct:identifier "anthropogenic_hazards/distribution/episode-elements/OK";
		dct:title "Episode OKLAHOMA: conventional and unconventional hydrocarbon extraction and wastewater injection - dataset";
		dct:description "Enables to list data items contained in the episode (dataset) as ‘Catalog', 'Seismic Network', 'Event related waveforms', 'Faults' and some 'Industrial data', features filtering. Episode comprehensively describes a geophysical process induced or triggered by human technological activity, which could pose a hazard for populations, infrastructure and environment. In recent years the seismicity rate and magnitude of seismicity in Oklahoma has increased. It has been found that this is due to the injection of fluids for both conventional and unconvential hydrocarbon exploitation as well as waste water injection."; 
		dct:type "http://publications.europa.eu/resource/authority/distribution-type/WEB_SERVICE"^^xsd:anyURI;
		dct:conformsTo <anthropogenic_hazards/webservice/is-epos_platform> ;
		dcat:accessURL <anthropogenic_hazards/webservice/is-epos_platform/episode-elements/OK>;
		dct:format "http://publications.europa.eu/resource/authority/file-type/JSON"^^xsd:anyURI;
		dct:license "https://creativecommons.org/licenses/by/4.0/"^^xsd:anyURI;
. 
	<anthropogenic_hazards/distribution/episode-elements/PREESALL_MINE> a dcat:Distribution;
		dct:identifier "anthropogenic_hazards/distribution/episode-elements/PREESALL_MINE";
		dct:title "Episode PREESALL MINE: underground salt extraction cavities - dataset";
		dct:description "Enables to list data items contained in the episode (dataset) as ‘Catalog', 'Seismic Network', 'Event related waveforms', 'Gravity Monitoring' and some 'Industrial data', features filtering. Episode comprehensively describes a geophysical process induced or triggered by human technological activity, which could pose a hazard for populations, infrastructure and environment. Located in the NW of England in the county of Lancashire, the Preesall Salt field (also known as the Preesall Brine field) is one of the UK’s major onshore halite formations. The field contains thick beds of Triassic aged halite (Pressall Halite) which lie along the Fylde Coast (to the north of Blackpool and East of the river Wyre) and was once the site of the largest salt producer in Britain. Since the 1870’s the heavy exploitation of salt by dry mining and by brine extraction has left the Preesall area with dramatic subsidence damage including unstable cavities and several deep flashes, subsidence induced lakes following a number of major collapse events. This episode contains seismic data and time-lapse micro-gravity data collected from around a brine well over an unstable cavity situated South-west of the previous Preesall Salt Mine. Data collected as part of a PhD Thesis by Mike Branston at Keele University - (Branston, 2003)."; 
		dct:type "http://publications.europa.eu/resource/authority/distribution-type/WEB_SERVICE"^^xsd:anyURI;
		dct:conformsTo <anthropogenic_hazards/webservice/is-epos_platform> ;
		dcat:accessURL <anthropogenic_hazards/webservice/is-epos_platform/episode-elements/PREESALL_MINE>;
		dct:format "http://publications.europa.eu/resource/authority/file-type/JSON"^^xsd:anyURI;
		dct:license "https://creativecommons.org/licenses/by/4.0/"^^xsd:anyURI;
.
	<anthropogenic_hazards/distribution/episode-elements/GRONINGEN_FIELD> a dcat:Distribution;
		dct:identifier "anthropogenic_hazards/distribution/episode-elements/GRONINGEN_FIELD";
		dct:title "Episode GRONINGEN FIELD: conventional hydrocarbon production - dataset";
		dct:description "Enables to list data items contained in the episode (dataset) as ‘Catalog', 'Ground Motion Catalog','Seismic Network', 'Event related waveforms', 'Satellite Data' and some 'Industrial data', features filtering. Episode comprehensively describes a geophysical process induced or triggered by human technological activity, which could pose a hazard for populations, infrastructure and environment. The Groningen gas field is a giant natural gas field located near Slochteren in Groningen province in the northeastern part of the Netherlands. Discovered in 1959, it is the largest natural gas field in Europe and the tenth-largest in the world."; 
		dct:type "http://publications.europa.eu/resource/authority/distribution-type/WEB_SERVICE"^^xsd:anyURI;
		dct:conformsTo <anthropogenic_hazards/webservice/is-epos_platform> ;
		dcat:accessURL <anthropogenic_hazards/webservice/is-epos_platform/episode-elements/GRONINGEN_FIELD>;
		dct:format "http://publications.europa.eu/resource/authority/file-type/JSON"^^xsd:anyURI;
		dct:license "https://creativecommons.org/licenses/by/4.0/"^^xsd:anyURI;
. 
	<anthropogenic_hazards/distribution/episode-elements/LAI_CHAU> a dcat:Distribution;
		dct:identifier "anthropogenic_hazards/distribution/episode-elements/LAI_CHAU";
		dct:title "Episode LAI CHAU: water reservoir - dataset";
		dct:description "Enables to list data items contained in the episode (dataset) as ‘Catalog', 'Seismic Network', 'Event related waveforms' and some 'Industrial data', features filtering. Episode comprehensively describes a geophysical process induced or triggered by human technological activity, which could pose a hazard for populations, infrastructure and environment. Seismic activity in Lai Chau episode is linked to the hydropower plant and the reservoir containing backed up water of Da river (Black river) in northwestern Vietnam. Construction started on 5 January 2011 and it is expected to be operational by 2017 with the first turbine put into operation in 2016. The area of the reservoir is considered as tectonically active with known earthquakes in the past. During the period from September 2014 to May 2015, the network of seismological stations in broad Lai Chau region recorded nearly 40 earthquakes M 1.1 to 4.0. Three of them occurred directly in Lai Chau hydro reservoir area (October 19 and 31, 2014 M3.5 and November 26, 2014 M2.0). The reservoir filling started in June 2015. The water level varies between 205 and 280 m. a.s.l. During the period from October 2014 to October 2015, the network of seismological stations in wide Lai Chau area recorded nearly 60 earthquakes with M1.0 to 4.0. Several of them were located a radius of 6-20 km from Lai Chau dam."; 
		dct:type "http://publications.europa.eu/resource/authority/distribution-type/WEB_SERVICE"^^xsd:anyURI;
		dct:conformsTo <anthropogenic_hazards/webservice/is-epos_platform> ;
		dcat:accessURL <anthropogenic_hazards/webservice/is-epos_platform/episode-elements/LAI_CHAU>;
		dct:format "http://publications.europa.eu/resource/authority/file-type/JSON"^^xsd:anyURI;
		dct:license "https://creativecommons.org/licenses/by/4.0/"^^xsd:anyURI;
.
	<anthropogenic_hazards/distribution/episode-elements/LUBOCINO> a dcat:Distribution;
		dct:identifier "anthropogenic_hazards/distribution/episode-elements/LUBOCINO";
		dct:title "Episode LUBOCINO: Shale Gas - dataset";
		dct:description "Enables to list data items contained in the episode (dataset) as ‘Water Quality data' and 'Satellite data', features filtering. Episode comprehensively describes a geophysical process induced or triggered by human technological activity, which could pose a hazard for populations, infrastructure and the environment. Hydrofracturing described in Lubocino episode was conducted in Pomerania, Poland by PGNiG (Polish Oil and Gas Company). The data available in the episode includes seismic monitoring, monitoring of air and water quality and ground deformation information. With participation of the government representatives and the private industry, best practices to monitor and minimize the environmental impact of shale gas exploitation in Europe were developed."; 
		dct:type "http://publications.europa.eu/resource/authority/distribution-type/WEB_SERVICE"^^xsd:anyURI;
		dct:conformsTo <anthropogenic_hazards/webservice/is-epos_platform> ;
		dcat:accessURL <anthropogenic_hazards/webservice/is-epos_platform/episode-elements/LUBOCINO>;
		dct:format "http://publications.europa.eu/resource/authority/file-type/JSON"^^xsd:anyURI;
		dct:license "https://creativecommons.org/licenses/by/4.0/"^^xsd:anyURI;
.
	<anthropogenic_hazards/distribution/episode-elements/WYSIN> a dcat:Distribution;
		dct:identifier "anthropogenic_hazards/distribution/episode-elements/WYSIN";
		dct:title "Episode WYSIN: Shale Gas - dataset";
		dct:description "Enables to list data items contained in the episode (dataset) as 'Seismic Network', 'Waveforms', 'Air Quality Data', 'Water Quality Data', 'Satellite Data', 'Velocity model' and some 'Industrial data', features filtering. Episode comprehensively describes a geophysical process induced or triggered by human technological activity, which could pose a hazard for populations, infrastructure and environment. This episode describes monitoring the environmental impacts of shale gas exploration/exploitation at the site of one of the concessions of the Polish Oil and Gas SA company before, during and after termination of fracking operations. Detailed objectives are: • to establish background levels of seismicity, water condition and air pollution, • to sample the actual impact of fracking on the seismicity, water and air conditions in the direct vicinity and during fracking operations, • to recognize protracted effects of shale gas operations on the environment, • to provide observational data to be analyzed."; 
		dct:type "http://publications.europa.eu/resource/authority/distribution-type/WEB_SERVICE"^^xsd:anyURI;
		dct:conformsTo <anthropogenic_hazards/webservice/is-epos_platform> ;
		dcat:accessURL <anthropogenic_hazards/webservice/is-epos_platform/episode-elements/WYSIN>;
		dct:format "http://publications.europa.eu/resource/authority/file-type/JSON"^^xsd:anyURI;
		dct:license "https://creativecommons.org/licenses/by/4.0/"^^xsd:anyURI;
.
	<anthropogenic_hazards/distribution/episode-elements/CARBFIX> a dcat:Distribution;
		dct:identifier "anthropogenic_hazards/distribution/episode-elements/CARBFIX";
		dct:title "Episode CARBFIX: geothermal energy production and CCS - dataset";
		dct:description "Enables to list data items contained in the episode (dataset) as ‘Catalog', 'Seismic Network' and some 'Industrial data', features filtering. Episode comprehensively describes a geophysical process induced or triggered by human technological activity, which could pose a hazard for populations, infrastructure and environment. CarbFix is a CCS consortium operated by RE, UI, Columbia University (USA) and CNRS (France). It is one of the most successful and best-known examples of CO2 sequestration processes in the world. RE operates over 100 wells at Hellisheidi, about 10 of which are used for re-injection of geothermal water, one is used for re-injection of captured gases, the others are production and monitoring wells. Roughly one-third of the CO2 and H2S presently emitted from the Hellishidi power plant is being injected as a dissolved water phase into fractured basaltic rocks. CCS operations are followed by the seismic activity."; 
		dct:type "http://publications.europa.eu/resource/authority/distribution-type/WEB_SERVICE"^^xsd:anyURI;
		dct:conformsTo <anthropogenic_hazards/webservice/is-epos_platform> ;
		dcat:accessURL <anthropogenic_hazards/webservice/is-epos_platform/episode-elements/CARBFIX>;
		dct:format "http://publications.europa.eu/resource/authority/file-type/JSON"^^xsd:anyURI;
		dct:license "https://creativecommons.org/licenses/by/4.0/"^^xsd:anyURI;
.
	<anthropogenic_hazards/distribution/episode-elements/SG> a dcat:Distribution;
		dct:identifier "anthropogenic_hazards/distribution/episode-elements/SG";
		dct:title "Episode ST. GALLEN: geothermal project - dataset";
		dct:description "Enables to list data items contained in the episode (dataset) as ‘Catalog' and some 'Industrial data', features filtering. Episode comprehensively describes a geophysical process induced or triggered by human technological activity, which could pose a hazard for populations, infrastructure and environment. This episode decribes the geothermal project undertaken by the city of St. Gallen (Switzerland) and operated by the St. Galler Stadtwerke was based on a large-scale 3D seismic survey in 2010. The survey led to drilling of the geothermal well, “St. Gallen GT-1”, to a measured depth of 4450 m across Paleozoic / Mesozoic rock formations as well as extensive scientific and technical analysis, and well completion aimed at geothermal use. The area has additionally been instrumented with a micro-seismic array operated since 2012 by the Swiss Seismic Survey (SED). After complications occurred during well stimulation and testing in July 2013 (a gas kick and seismic events up to ML 3.5 as a consequence of killing the well) the project was temporarily stopped. In October 2013 the project was resumed with a modified drill stem test producing gas and water and collection of a comprehensive data set on the developed jointed aquifer within the regionally prominent St. Gallen Fault Zone. The geothermal project has been halted in May 2014. This episode is a data set for correlating seismic activity to fluid injection and gas-water production that lead to increased seismic activity in the past."; 
		dct:type "http://publications.europa.eu/resource/authority/distribution-type/WEB_SERVICE"^^xsd:anyURI;
		dct:conformsTo <anthropogenic_hazards/webservice/is-epos_platform> ;
		dcat:accessURL <anthropogenic_hazards/webservice/is-epos_platform/episode-elements/SG>;
		dct:format "http://publications.europa.eu/resource/authority/file-type/JSON"^^xsd:anyURI;
		dct:license "https://creativecommons.org/licenses/by/4.0/"^^xsd:anyURI;
. 
# will be available July/August 2019
#	<anthropogenic_hazards/distribution/episode-elements/COTTON_VALLEY> a dcat:Distribution;
#		dct:identifier "anthropogenic_hazards/distribution/episode-elements/COTTON_VALLEY";
#		dct:title "Episode COTTON VALLEY: hydraulic fracturing - dataset";
#		dct:description "Enables to list data items contained in the episode (dataset) as 'Catalog, 'Seismic Network', 'Event Related Waveforms', 'Velocity model' and some 'Industrial data', features filtering. Episode comprehensively describes a geophysical process induced or triggered by human technological activity, which could pose a hazard for populations, infrastructure and environment. Fracture imaging study in the Carthage Gas Unit, Panola County, Texas, USA is shown where microseismic events induced by hydraulic fracturing at a depth of 9,500 ft were detected at distances exceeding 1,300 ft from the origin. An industry consortium of major operators, service companies, government agencies and national laboratories was formed to perform a more detailed study using 96, 3-component geophone sondes distributed among two monitor wells. A unique microseismic recording system specifically designed and manufactured for these operating depths is presented. Applications of the technology include optimization of hydraulic fracture designs and accurate mapping of fracture geometry. The data recorded at the Cotton Valley hydrofracture were of high quality and provided definitive results in gaining an understanding of the fracture generations at this site. The instrumentation worked admirably with only minor problems resulting from loss of some of the downhole sensors damaged during installation. Additionally, several channels have been contaminated by electrical noise and in many instances, the P-wave amplitudes were often lost within the background noise. Data integrated as Cotton Valley episode have been converted from the original CDs. Some data were corrupted on those CDs as well as the original full filenames were lost during the transfer to PC format from Unix operating system."; 
#		dct:type "http://publications.europa.eu/resource/authority/distribution-type/WEB_SERVICE"^^xsd:anyURI;
#		dct:conformsTo <anthropogenic_hazards/webservice/is-epos_platform> ;
#		dcat:accessURL <anthropogenic_hazards/webservice/is-epos_platform/episode-elements/COTTON_VALLEY>;
#		dct:format "http://publications.europa.eu/resource/authority/file-type/JSON"^^xsd:anyURI;
#		dct:license "https://creativecommons.org/licenses/by/4.0/"^^xsd:anyURI;
#. 
	<anthropogenic_hazards/distribution/episode-elements/VOUGLANS> a dcat:Distribution;
		dct:identifier "anthropogenic_hazards/distribution/episode-elements/VOUGLANS";
		dct:title "Episode VOUGLANS: water reservoir - dataset";
		dct:description "Enables to list data items contained in the episode (dataset) as ‘Catalog' and some 'Industrial data', features filtering. Episode comprehensively describes a geophysical process induced or triggered by human technological activity, which could pose a hazard for populations, infrastructure and environment. The Vouglans dam is an hydropower reservoir located on the Ain river, Jura, France. The dam construction was completed in 1968 and so for the Vouglans Lake impoundment. This is the third largest artificial water reservoir in France by its capacity (605 Mm3). Although no earthquakes were recorded in the 1962-1968 period, seismicity close (25km radius) to the reservoir started in 1969 and it lasted up to 2000’. The largest shock (M4.6) occurred in 1971."; 
		dct:type "http://publications.europa.eu/resource/authority/distribution-type/WEB_SERVICE"^^xsd:anyURI;
		dct:conformsTo <anthropogenic_hazards/webservice/is-epos_platform> ;
		dcat:accessURL <anthropogenic_hazards/webservice/is-epos_platform/episode-elements/VOUGLANS>;
		dct:format "http://publications.europa.eu/resource/authority/file-type/JSON"^^xsd:anyURI;
		dct:license "https://creativecommons.org/licenses/by/4.0/"^^xsd:anyURI;
. 
	<anthropogenic_hazards/distribution/episode-elements/GAZLI> a dcat:Distribution;
		dct:identifier "anthropogenic_hazards/distribution/episode-elements/GAZLI";
		dct:title "Episode GAZLI: hydrocarbon field - dataset";
		dct:description "Enables to list data items contained in the episode (dataset) as ‘Catalog' and some 'Industrial data', features filtering. Episode comprehensively describes a geophysical process induced or triggered by human technological activity, which could pose a hazard for populations, infrastructure and environment. From 1976 to 1984, three magnitude 7 earthquakes struck the intraplate area of Gazli (Uzbekistan), an area previously assigned to a 'low seismic risk' zone. Their closeness to an important gas field suggests that these events may be induced or triggered by geo-resource production related to fluid manipulations. Since these early 1976-84 M7 events, the seismic sequence develops as a long lasting seismic swarm, up to now."; 
		dct:type "http://publications.europa.eu/resource/authority/distribution-type/WEB_SERVICE"^^xsd:anyURI;
		dct:conformsTo <anthropogenic_hazards/webservice/is-epos_platform> ;
		dcat:accessURL <anthropogenic_hazards/webservice/is-epos_platform/episode-elements/GAZLI>;
		dct:format "http://publications.europa.eu/resource/authority/file-type/JSON"^^xsd:anyURI;
		dct:license "https://creativecommons.org/licenses/by/4.0/"^^xsd:anyURI;
. 
	<anthropogenic_hazards/distribution/episode-elements/BOGDANKA> a dcat:Distribution;
		dct:identifier "anthropogenic_hazards/distribution/episode-elements/BOGDANKA";
		dct:title "Episode BOGDANKA: underground coal mining - dataset";
		dct:description "Enables to list data items contained in the episode (dataset) as ‘Catalog', 'Seismic Network', 'Event related waveforms', 'Velocity model' and some 'Industrial data', features filtering. Episode comprehensively describes a geophysical process induced or triggered by human technological activity, which could pose a hazard for populations, infrastructure and environment. The BOIS episode contains data related to seismic activity induced by mining. In the region which is located in eastern Poland, coal is excavated by Lubelski Węgiel “Bogdnaka” mine. The mine uses longwall system and coal seams are located from 0.5 – 1.2 km below the surface. The seismicity is monitored with 12 broad-band (5s) seismometers (GeoSIG VE-53/BB). The episode started in November 2018 and remains open."; 
		dct:type "http://publications.europa.eu/resource/authority/distribution-type/WEB_SERVICE"^^xsd:anyURI;
		dct:conformsTo <anthropogenic_hazards/webservice/is-epos_platform> ;
		dcat:accessURL <anthropogenic_hazards/webservice/is-epos_platform/episode-elements/BOGDANKA>;
		dct:format "http://publications.europa.eu/resource/authority/file-type/JSON"^^xsd:anyURI;
		dct:license "https://creativecommons.org/licenses/by/4.0/"^^xsd:anyURI;
. 


	<anthropogenic_hazards/software/CatalogToXls> a schema:SoftwareApplication;
		schema:identifier "anthropogenic_hazards/software/CatalogToXls" ;
		schema:identifier [ a schema:PropertyValue ;
			schema:propertyID  "DDSS-ID" ;
		  	schema:value "WP14-DDSS-A01" ;
		];
		schema:name "Catalog to XLS converter" ;
		schema:description "Exports a Catalog MATLAB file as a spreadsheet file (in XLSX format)" ;
  		schema:contactPoint  <https://orcid.org/0000-0002-9824-7962/contactPoint> ;
  		schema:mainEntityOfPage "https://tcs.ah-epos.eu/#app:CatalogToXls"^^xsd:anyURI ;
		schema:license "https://creativecommons.org/licenses/by/4.0/"^^xsd:anyURI ;
		schema:softwareVersion "1.0";
		schema:keywords "format conversion", "data download", "data export" ;
  		dcat:theme <epos:Converters>;
.

	<anthropogenic_hazards/software/GDFToXls> a schema:SoftwareApplication;
		schema:identifier "anthropogenic_hazards/software/GDFToXls" ;
		schema:identifier [ a schema:PropertyValue ;
			schema:propertyID  "DDSS-ID" ;
		  	schema:value "WP14-DDSS-A02" ;
		];
		schema:name "GDF to XLS converter" ;
		schema:description "Exports a GDF MATLAB file as a spreadsheet file (in XLSX format)" ;
  		schema:contactPoint  <https://orcid.org/0000-0002-9824-7962/contactPoint> ;
		schema:mainEntityOfPage "https://tcs.ah-epos.eu/#app:GDFToXls"^^xsd:anyURI ;
		schema:license "https://creativecommons.org/licenses/by/4.0/"^^xsd:anyURI ;
		schema:softwareVersion "1.0";
		schema:keywords "format conversion", "data download", "data export" ;
		dcat:theme <epos:Converters>;
.

	<anthropogenic_hazards/software/FrontHistogramsVis> a schema:SoftwareApplication;
		schema:identifier "anthropogenic_hazards/software/FrontHistogramsVis" ;
		schema:identifier [ a schema:PropertyValue ;
			schema:propertyID  "DDSS-ID" ;
		  	schema:value "WP14-DDSS-A03" ;
		];
		schema:name "Front Advance Histograms" ;
		schema:description "Application for drawing histograms and cumulative histograms of events count and seismic energy for selected bins, the width of which corresponds to a constant value of the mining front advance. Calculations are performed from the beginning of the excavation along the axis of the excavation" ;
  		schema:contactPoint  <https://orcid.org/0000-0002-9824-7962/contactPoint> ;
		schema:mainEntityOfPage "https://tcs.ah-epos.eu/#app:FrontHistogramsVis"^^xsd:anyURI ;
		schema:license "https://creativecommons.org/licenses/by/4.0/"^^xsd:anyURI ;
		schema:softwareVersion "1.0";
		schema:keywords "episode-oriented graphics", "production data visualization";
		dcat:theme <epos:Visualizations>;
.

	<anthropogenic_hazards/software/FrontAdvanceVis> a schema:SoftwareApplication;
		schema:identifier "anthropogenic_hazards/software/FrontAdvanceVis" ;
		schema:identifier [ a schema:PropertyValue ;
			schema:propertyID  "DDSS-ID" ;
		  	schema:value "WP14-DDSS-A04" ;
		];
		schema:name "Seismic Activity with Front Advance" ;
		schema:description "Application allowing for visualization of the activity changes in time relatively to the front location" ;
  		schema:contactPoint  <https://orcid.org/0000-0002-9824-7962/contactPoint> ;
		schema:mainEntityOfPage "https://tcs.ah-epos.eu/#app:FrontAdvanceVis"^^xsd:anyURI ;
		schema:license "https://creativecommons.org/licenses/by/4.0/"^^xsd:anyURI ;
		schema:softwareVersion "1.0";
		schema:keywords "episode-oriented graphics", "production data visualization", "production - seismicity interaction";
		dcat:theme <epos:Visualizations>;
.

	<anthropogenic_hazards/software/EPISODE_BASIC_GMAPS_Visualization> a schema:SoftwareApplication;
		schema:identifier "anthropogenic_hazards/software/EPISODE_BASIC_GMAPS_Visualization" ;
		schema:identifier [ a schema:PropertyValue ;
			schema:propertyID  "DDSS-ID" ;
		  	schema:value "WP14-DDSS-A05" ;
		];
		schema:name "Integrated Google Maps data visualization" ;
		schema:description "Application allowing visualization of miscellaneous data related to episode" ;
  		schema:contactPoint  <https://orcid.org/0000-0002-9824-7962/contactPoint> ;
		schema:mainEntityOfPage "https://tcs.ah-epos.eu/#app:EPISODE_BASIC_GMAPS_Visualization"^^xsd:anyURI ;
		schema:license "https://creativecommons.org/licenses/by/4.0/"^^xsd:anyURI ;
		schema:softwareVersion "1.0";
		schema:keywords "episode-oriented graphics", "episode visualization", "GIS data visualization", "production - seismicity interaction";
		dcat:theme <epos:Visualizations>;
.

	<anthropogenic_hazards/software/CatalogFilter> a schema:SoftwareApplication;
		schema:identifier "anthropogenic_hazards/software/CatalogFilter" ;
		schema:identifier [ a schema:PropertyValue ;
			schema:propertyID  "DDSS-ID" ;
		  	schema:value "WP14-DDSS-A06" ;
		];
		schema:name "Catalog Filter" ;
		schema:description "This application performs selection of catalog data by filtering fields specified by the user. This can be by selecting a particular range/list of values from diverse catalog attributes, or interactively by the mapped events epicenters" ;
  		schema:contactPoint  <https://orcid.org/0000-0002-9824-7962/contactPoint> ;
		schema:mainEntityOfPage "https://tcs.ah-epos.eu/#app:CatalogFilter"^^xsd:anyURI ;
		schema:license "https://creativecommons.org/licenses/by/4.0/"^^xsd:anyURI ;
		schema:softwareVersion "1.0";
		schema:keywords "data selection", "data filtering";
		dcat:theme <epos:FilteringTools>;
.

	<anthropogenic_hazards/software/CatalogToVector> a schema:SoftwareApplication;
		schema:identifier "anthropogenic_hazards/software/CatalogToVector" ;
		schema:identifier [ a schema:PropertyValue ;
			schema:propertyID  "DDSS-ID" ;
		  	schema:value "WP14-DDSS-A07" ;
		];
		schema:name "Catalog to Vectors converter" ;
		schema:description "Tool for converting a Catalog into a series of vectors that can be further used in other applications (e.g. Time Series Builder)." ;
  		schema:contactPoint  <https://orcid.org/0000-0002-9824-7962/contactPoint> ;
		schema:mainEntityOfPage "https://tcs.ah-epos.eu/#app:CatalogToVector"^^xsd:anyURI ;
		schema:license "https://creativecommons.org/licenses/by/4.0/"^^xsd:anyURI ;
		schema:softwareVersion "1.0";
		schema:keywords "data selection", "data extraction";
		dcat:theme <epos:Converters>;
.

	<anthropogenic_hazards/software/GDFToVector> a schema:SoftwareApplication;
		schema:identifier "anthropogenic_hazards/software/GDFToVector" ;
		schema:identifier [ a schema:PropertyValue ;
			schema:propertyID  "DDSS-ID" ;
		  	schema:value "WP14-DDSS-A08" ;
		];
		schema:name "GDF to Vectors converter" ;
		schema:description "Tool for converting a GDF file into a series of vectors that can be further used in other applications (e.g. Time Series Builder)." ;
  		schema:contactPoint  <https://orcid.org/0000-0002-9824-7962/contactPoint> ;
		schema:mainEntityOfPage "https://tcs.ah-epos.eu/#app:GDFToVector"^^xsd:anyURI ;
		schema:license "https://creativecommons.org/licenses/by/4.0/"^^xsd:anyURI ;
		schema:softwareVersion "1.0";
		schema:keywords "data selection", "data extraction";
		dcat:theme <epos:Converters>;
.

	<anthropogenic_hazards/software/CatalogMergeTool> a schema:SoftwareApplication;
		schema:identifier "anthropogenic_hazards/software/CatalogMergeTool" ;
		schema:identifier [ a schema:PropertyValue ;
			schema:propertyID  "DDSS-ID" ;
		  	schema:value "WP14-DDSS-A09" ;
		];
		schema:name "Ground Motion Parameters Catalog builder" ;
		schema:description "Joins a Seismic Catalog and a GM Catalog into a joined catalog" ;
  		schema:contactPoint  <https://orcid.org/0000-0002-9824-7962/contactPoint> ;
		schema:mainEntityOfPage "https://tcs.ah-epos.eu/#app:CatalogMergeTool"^^xsd:anyURI ;
		schema:license "https://creativecommons.org/licenses/by/4.0/"^^xsd:anyURI ;
		schema:softwareVersion "1.0";
		schema:keywords "data selection", "data merging";
		dcat:theme <epos:Converters>;
.

	<anthropogenic_hazards/software/SeedConverter> a schema:SoftwareApplication;
		schema:identifier "anthropogenic_hazards/software/SeedConverter" ;
		schema:identifier [ a schema:PropertyValue ;
			schema:propertyID  "DDSS-ID" ;
		  	schema:value "WP14-DDSS-A10" ;
		];
		schema:name "Seed converter" ;
		schema:description "Converts SEED volume (either fullSEED or miniSEED) to either SAC or ASCII" ;
  		schema:contactPoint  <https://orcid.org/0000-0002-9824-7962/contactPoint> ;
		schema:mainEntityOfPage "https://tcs.ah-epos.eu/#app:SeedConverter"^^xsd:anyURI ;
		schema:license "https://creativecommons.org/licenses/by/4.0/"^^xsd:anyURI ;
		schema:softwareVersion "1.0";
		schema:keywords "format conversion", "data merging", "data filtering", "data export";
		dcat:theme <epos:Converters>;
.

	<anthropogenic_hazards/software/SeismogramPicks> a schema:SoftwareApplication;
		schema:identifier "anthropogenic_hazards/software/SeismogramPicks" ;
		schema:identifier [ a schema:PropertyValue ;
			schema:propertyID  "DDSS-ID" ;
		  	schema:value "WP14-DDSS-A11" ;
		];
		schema:name "Seismogram Picking Tool" ;
		schema:description "Performs selection of phases and picks on seismograms" ;
  		schema:contactPoint  <https://orcid.org/0000-0002-9824-7962/contactPoint> ;
		schema:mainEntityOfPage "https://tcs.ah-epos.eu/#app:SeismogramPicks"^^xsd:anyURI ;
		schema:license "https://creativecommons.org/licenses/by/4.0/"^^xsd:anyURI ;
		schema:softwareVersion "1.0";
		schema:keywords "waveform viewing", "picking on waveform", "format conversion";
		dcat:theme <epos:SeismogramAnalysisTools>;
.

	<anthropogenic_hazards/software/SignalDownload> a schema:SoftwareApplication;
		schema:identifier "anthropogenic_hazards/software/SignalDownload" ;
		schema:identifier [ a schema:PropertyValue ;
			schema:propertyID  "DDSS-ID" ;
		  	schema:value "WP14-DDSS-A12" ;
		];
		schema:name "Signal Download Tool" ;
		schema:description "Application that downloads signals for a selected events" ;
  		schema:contactPoint  <https://orcid.org/0000-0002-9824-7962/contactPoint> ;
		schema:mainEntityOfPage "https://tcs.ah-epos.eu/#app:SignalDownload"^^xsd:anyURI ;
		schema:license "https://creativecommons.org/licenses/by/4.0/"^^xsd:anyURI ;
		schema:softwareVersion "1.0";
		schema:keywords "data selection", "data export", "waveform viewing";
		dcat:theme <epos:SeismogramAnalysisTools>;
.

	<anthropogenic_hazards/software/TimeSeriesBuilder> a schema:SoftwareApplication;
		schema:identifier "anthropogenic_hazards/software/TimeSeriesBuilder" ;
		schema:identifier [ a schema:PropertyValue ;
			schema:propertyID  "DDSS-ID" ;
		  	schema:value "WP14-DDSS-A14" ;
		];
		schema:name "Time Series Builder" ;
		schema:description "Allows to choose stationary time series based on given time vector" ;
  		schema:contactPoint  <https://orcid.org/0000-0002-9824-7962/contactPoint> ;
		schema:mainEntityOfPage "https://tcs.ah-epos.eu/#app:TimeSeriesBuilder"^^xsd:anyURI ;
		schema:license "https://creativecommons.org/licenses/by/4.0/"^^xsd:anyURI ;
		schema:softwareVersion "1.0";
		schema:keywords "data selection", "data filtering", "data reshaping", "data conversion";
		dcat:theme <epos:Converters>;
.

	<anthropogenic_hazards/software/SeiscompOrder> a schema:SoftwareApplication;
		schema:identifier "anthropogenic_hazards/software/SeiscompOrder" ;
		schema:identifier [ a schema:PropertyValue ;
			schema:propertyID  "DDSS-ID" ;
		  	schema:value "WP14-DDSS-A15" ;
		];
		schema:name "Waveform Download Tool" ;
		schema:description "Application that allows for requesting parts of continuous waveforms for specific dates and stations. The preparation of the waveform is executed by Arclink-fetch." ;
  		schema:contactPoint  <https://orcid.org/0000-0002-9824-7962/contactPoint> ;
		schema:mainEntityOfPage "https://tcs.ah-epos.eu/#app:SeiscompOrder"^^xsd:anyURI ;
		schema:license "https://creativecommons.org/licenses/by/4.0/"^^xsd:anyURI ;
		schema:softwareVersion "1.0";
		schema:keywords "data selection", "data filtering", "data export", "waveform viewing";
		dcat:theme <epos:SeismogramAnalysisTools>;
.

	<anthropogenic_hazards/software/MagnitudeConversionApp> a schema:SoftwareApplication;
		schema:identifier "anthropogenic_hazards/software/MagnitudeConversionApp" ;
		schema:identifier [ a schema:PropertyValue ;
			schema:propertyID  "DDSS-ID" ;
		  	schema:value "WP14-DDSS-A16" ;
		];
		schema:name "Magnitude conversion" ;
		schema:description "Establishes empirical scaling relationships between different magnitude scales" ;
  		schema:contactPoint  <https://orcid.org/0000-0002-9824-7962/contactPoint> ;
		schema:mainEntityOfPage "https://tcs.ah-epos.eu/#app:MagnitudeConversionApp"^^xsd:anyURI ;
		schema:license "https://creativecommons.org/licenses/by/4.0/"^^xsd:anyURI ;
		schema:softwareVersion "1.0";
		schema:keywords "data conversion";
		dcat:theme <epos:CollectivePropertiesOfSeismicityAnalysis>;
.

	<anthropogenic_hazards/software/StationarityTestingApp> a schema:SoftwareApplication;
		schema:identifier "anthropogenic_hazards/software/StationarityTestingApp" ;
		schema:identifier [ a schema:PropertyValue ;
			schema:propertyID  "DDSS-ID" ;
		  	schema:value "WP14-DDSS-A17" ;
		];
		schema:name "Anderson-Darling test for exponentiality of inter-event time" ;
		schema:description "Performs the Anderson-Darling test to study the null hypothesis that the inter-event times of a given series of events are drawn from an exponential distribution, alternatively that they are drawn from a Weibull distribution." ;
  		schema:contactPoint  <https://orcid.org/0000-0002-9824-7962/contactPoint> ;
		schema:mainEntityOfPage "https://tcs.ah-epos.eu/#app:StationarityTestingApp"^^xsd:anyURI ;
		schema:license "https://creativecommons.org/licenses/by/4.0/"^^xsd:anyURI ;
		schema:softwareVersion "1.0";
		schema:keywords "statistical analysis", "statistical properties of seismicity", "parameter probabilistic distribution";
		dcat:theme <epos:CollectivePropertiesOfSeismicityAnalysis>;
.

	<anthropogenic_hazards/software/CompletenessLevelApp> a schema:SoftwareApplication;
		schema:identifier "anthropogenic_hazards/software/CompletenessLevelApp" ;
		schema:identifier [ a schema:PropertyValue ;
			schema:propertyID  "DDSS-ID" ;
		  	schema:value "WP14-DDSS-A18" ;
		];
		schema:name "Completeness Magnitude Estimation" ;
		schema:description "To evaluate the magnitude of completeness Mc, defined as the lowest magnitude at which all seismic events in a selected space-time volume are recorded by a network. Mc is an essential prerequisite for most seismicity analyses." ;
  		schema:contactPoint  <https://orcid.org/0000-0002-9824-7962/contactPoint> ;
		schema:mainEntityOfPage "https://tcs.ah-epos.eu/#app:CompletenessLevelApp"^^xsd:anyURI ;
		schema:license "https://creativecommons.org/licenses/by/4.0/"^^xsd:anyURI ;
		schema:softwareVersion "1.0";
		schema:keywords "statistical analysis", "statistical properties of seismicity", "parameter probabilistic distribution";
		dcat:theme <epos:CollectivePropertiesOfSeismicityAnalysis>;
.

	<anthropogenic_hazards/software/GDFTDSH> a schema:SoftwareApplication;
		schema:identifier "anthropogenic_hazards/software/GDFTDSH" ;
		schema:identifier [ a schema:PropertyValue ;
			schema:propertyID  "DDSS-ID" ;
		  	schema:value "WP14-DDSS-A19" ;
		];
		schema:name "Estimation of Source Parameters in Time-varying Production Parameters Geometry" ;
		schema:description "To estimate time-dependent values of seismic hazard parameters: the activity rate, the Gutenberg-Richter b-value, the return period and the exceedance probability for a prescribed area. The parameter values for the time moment t are estimated optionally either from events that occurred in dt time units preceding t, where dt is kept constant, or from n last events before t, where n is kept constant. Four magnitude distribution estimation methods are supported: maximum likelihood using the unbounded Gutenberg-Richter relation based model, maximum likelihood using the upper-bounded Gutenberg-Richter relation based model, unbounded non-parametric kernel estimation, upper-bounded non-parametric kernel estimation. The upper limit of magnitude distribution is evaluated using the Kijko-Sellevol generic formula." ;
  		schema:contactPoint  <https://orcid.org/0000-0002-9824-7962/contactPoint> ;
		schema:mainEntityOfPage "https://tcs.ah-epos.eu/#app:GDFTDSH"^^xsd:anyURI ;
		schema:license "https://creativecommons.org/licenses/by/4.0/"^^xsd:anyURI ;
		schema:softwareVersion "1.0";
		schema:keywords "statistical analysis", "probabilistic seismic hazard analysis", "time-dependent hazard", "production-dependent hazard", "production - seismicity interaction";
		dcat:theme <epos:ProbabilisticSeismicHazardAnalysis>;
.

	<anthropogenic_hazards/software/TimeVaryingFullTDSH> a schema:SoftwareApplication;
		schema:identifier "anthropogenic_hazards/software/TimeVaryingFullTDSH" ;
		schema:identifier [ a schema:PropertyValue ;
			schema:propertyID  "DDSS-ID" ;
		  	schema:value "WP14-DDSS-A20" ;
		];
		schema:name "Time Dependent Hazard in Mining Front Surroundings" ;
		schema:description "To estimate time-dependent values of seismic hazard parameters: the activity rate, the Gutenberg-Richter b-value, the return period and the exceedance probability for a space window surrounding an advancing mining front. The parameter values for the time moment t are estimated optionally either from events that occurred in dt time units preceding t, where dt is kept constant, or from n last events before t, where n is kept constant, or from a time period during which the front advanced by a constant length dx. Four magnitude distribution estimation methods are supported: maximum likelihood using the unbounded Gutenberg-Richter relation based model, maximum likelihood using the upper- bounded Gutenberg-Richter relation based model, unbounded non-parametric kernel estimation, upper-bounded non-parametric kernel estimation. The upper limit of magnitude distribution is evaluated using the Kijko-Sellevol generic formula." ;
  		schema:contactPoint  <https://orcid.org/0000-0002-9824-7962/contactPoint> ;
		schema:mainEntityOfPage "https://tcs.ah-epos.eu/#app:TimeVaryingFullTDSH"^^xsd:anyURI ;
		schema:license "https://creativecommons.org/licenses/by/4.0/"^^xsd:anyURI ;
		schema:softwareVersion "1.0";
		schema:keywords "statistical analysis", "probabilistic seismic hazard analysis", "time-dependent hazard", "production-dependent hazard", "production - seismicity interaction";
		dcat:theme <epos:ProbabilisticSeismicHazardAnalysis>;
.

	<anthropogenic_hazards/software/StationaryTDSHFull> a schema:SoftwareApplication;
		schema:identifier "anthropogenic_hazards/software/StationaryTDSHFull" ;
		schema:identifier [ a schema:PropertyValue ;
			schema:propertyID  "DDSS-ID" ;
		  	schema:value "WP14-DDSS-A21" ;
		];
		schema:name "Time Dependent Hazard in Selected Area" ;
		schema:description "To estimate time-dependent values of seismic hazard parameters: the activity rate, the Gutenberg-Richter b-value, the return period and the exceedance probability for a prescribed area. The parameter values for the time moment t are estimated optionally either from events that occurred in dt time units preceding t, where dt is kept constant, or from n last events before t, where n is kept constant. Four magnitude distribution estimation methods are supported: maximum likelihood using the unbounded Gutenberg-Richter relation based model, maximum likelihood using the upper-bounded Gutenberg-Richter relation based model, unbounded non-parametric kernel estimation, upper-bounded non-parametric kernel estimation. The upper limit of magnitude distribution is evaluated using the Kijko-Sellevol generic formula." ;
  		schema:contactPoint  <https://orcid.org/0000-0002-9824-7962/contactPoint> ;
		schema:mainEntityOfPage "https://tcs.ah-epos.eu/#app:StationaryTDSHFull"^^xsd:anyURI ;
		schema:license "https://creativecommons.org/licenses/by/4.0/"^^xsd:anyURI ;
		schema:softwareVersion "1.0";
		schema:keywords "statistical analysis", "probabilistic seismic hazard analysis", "time-dependent hazard", "production-dependent hazard", "production - seismicity interaction";
		dcat:theme <epos:ProbabilisticSeismicHazardAnalysis>;
.

	<anthropogenic_hazards/software/ExcProbMag> a schema:SoftwareApplication;
		schema:identifier "anthropogenic_hazards/software/ExcProbMag" ;
		schema:identifier [ a schema:PropertyValue ;
			schema:propertyID  "DDSS-ID" ;
		  	schema:value "WP14-DDSS-A22" ;
		];
		schema:name "Stationary Hazard: Exceedance Probability" ;
		schema:description "This application uses the magnitude distribution and activity rate calculated from a seismic catalog to estimate the Exceedance Probability (EP). The EP of magnitude M in the time period of length T is the probability of an earthquake of magnitude M or greater to occur in T. The EP values are calculated optionally either for a fixed time period T and a series of magnitude values or for a fixed magnitude M and a series of period length values. Note: “Source size distribution functions/Stationary Hazard” application must be run before." ;
  		schema:contactPoint  <https://orcid.org/0000-0002-9824-7962/contactPoint> ;
		schema:mainEntityOfPage "https://tcs.ah-epos.eu/#app:ExcProbMag"^^xsd:anyURI ;
		schema:license "https://creativecommons.org/licenses/by/4.0/"^^xsd:anyURI ;
		schema:softwareVersion "1.0";
		schema:keywords "statistical analysis", "probabilistic seismic hazard analysis", "stationary hazard";
		dcat:theme <epos:ProbabilisticSeismicHazardAnalysis>;
.

	<anthropogenic_hazards/software/MaxCredMag> a schema:SoftwareApplication;
		schema:identifier "anthropogenic_hazards/software/MaxCredMag" ;
		schema:identifier [ a schema:PropertyValue ;
			schema:propertyID  "DDSS-ID" ;
		  	schema:value "WP14-DDSS-A23" ;
		];
		schema:name "Stationary Hazard: Maximum Credible Magnitude" ;
		schema:description "This application uses the magnitude distribution and activity rate from calculated a seismic catalog to estimate the Maximum Credible Magnitude (MCM). The MCM for the time period of length T is the magnitude value whose mean return period is T. The MCM values are calculated for a series of periods of length values. Note: “Source size distribution functions/Stationary Hazard” application must be run before." ;
  		schema:contactPoint  <https://orcid.org/0000-0002-9824-7962/contactPoint> ;
		schema:mainEntityOfPage "https://tcs.ah-epos.eu/#app:MaxCredMag"^^xsd:anyURI ;
		schema:license "https://creativecommons.org/licenses/by/4.0/"^^xsd:anyURI ;
		schema:softwareVersion "1.0";
		schema:keywords "statistical analysis", "probabilistic seismic hazard analysis", "stationary hazard";
		dcat:theme <epos:ProbabilisticSeismicHazardAnalysis>;
.

	<anthropogenic_hazards/software/MeanRetPeriod> a schema:SoftwareApplication;
		schema:identifier "anthropogenic_hazards/software/MeanRetPeriod" ;
		schema:identifier [ a schema:PropertyValue ;
			schema:propertyID  "DDSS-ID" ;
		  	schema:value "WP14-DDSS-A24" ;
		];
		schema:name "Stationary Hazard: Mean Return Period" ;
		schema:description "This application uses the magnitude distribution and activity rate calculated from a seismic catalog to estimate the Mean Return Period (MRP). The MRP of magnitude M is the average elapsed time between the consecutive earthquakes of magnitude M. The MRPs are calculated for a series of magnitude values. Note: “Source size distribution functions/Stationary Hazard” application must be run before." ;
  		schema:contactPoint  <https://orcid.org/0000-0002-9824-7962/contactPoint> ;
		schema:mainEntityOfPage "https://tcs.ah-epos.eu/#app:MeanRetPeriod"^^xsd:anyURI ;
		schema:license "https://creativecommons.org/licenses/by/4.0/"^^xsd:anyURI ;
		schema:softwareVersion "1.0";
		schema:keywords "statistical analysis", "probabilistic seismic hazard analysis", "stationary hazard";
		dcat:theme <epos:ProbabilisticSeismicHazardAnalysis>;
.

	<anthropogenic_hazards/software/BasicSSHApplication> a schema:SoftwareApplication;
		schema:identifier "anthropogenic_hazards/software/BasicSSHApplication" ;
		schema:identifier [ a schema:PropertyValue ;
			schema:propertyID  "DDSS-ID" ;
		  	schema:value "WP14-DDSS-A25" ;
		];
		schema:name "Source Size Distribution Functions / Stationary Hazard" ;
		schema:description "Estimates PDF and CDF of magnitudes assuming different models" ;
  		schema:contactPoint  <https://orcid.org/0000-0002-9824-7962/contactPoint> ;
		schema:mainEntityOfPage "https://tcs.ah-epos.eu/#app:BasicSSHApplication"^^xsd:anyURI ;
		schema:license "https://creativecommons.org/licenses/by/4.0/"^^xsd:anyURI ;
		schema:softwareVersion "1.0";
		schema:keywords "statistical analysis", "statistical properties of seismicity", "parameter probabilistic distribution", "stationary hazard";
		dcat:theme <epos:ProbabilisticSeismicHazardAnalysis>;
.

	<anthropogenic_hazards/software/SpectralAnalysis> a schema:SoftwareApplication;
		schema:identifier "anthropogenic_hazards/software/SpectralAnalysis" ;
		schema:identifier [ a schema:PropertyValue ;
			schema:propertyID  "DDSS-ID" ;
		  	schema:value "WP14-DDSS-A26" ;
		];
		schema:name "Spectral Analysis" ;
		schema:description "P and S waves spectral levels and corner frequencies using Snoke alghorithm." ;
  		schema:contactPoint  <https://orcid.org/0000-0002-9824-7962/contactPoint> ;
		schema:mainEntityOfPage "https://tcs.ah-epos.eu/#app:SpectralAnalysis"^^xsd:anyURI ;
		schema:license "https://creativecommons.org/licenses/by/4.0/"^^xsd:anyURI ;
		schema:softwareVersion "1.0";
		schema:keywords "source parameters", "earthquake spectra";
		dcat:theme <epos:SourceParameterEstimation>;
.

	<anthropogenic_hazards/software/FOCI_APP> a schema:SoftwareApplication;
		schema:identifier "anthropogenic_hazards/software/FOCI_APP" ;
		schema:identifier [ a schema:PropertyValue ;
			schema:propertyID  "DDSS-ID" ;
		  	schema:value "WP14-DDSS-A27" ;
		];
		schema:name "FOCI application" ;
		schema:description "This application makes use the P-wave first arrivals from the waveforms recorded by the seismic stations and resolves seismic moment tensors using various decomposition schemes. Three moment tensors are calculated: unconstrained (full) moment tensor solution, deviatoric moment tensor solution (no volumetric change in the source), and double-couple moment tensor solution (no volumetric change in the source, no linear dipole). In addition to the moment tensor components various source parameters are calculated as well (fault plane solutions, P/T/B axes orientation, scalar seismic moment etc)." ;
  		schema:contactPoint  <https://orcid.org/0000-0002-9824-7962/contactPoint> ;
		schema:mainEntityOfPage "https://tcs.ah-epos.eu/#app:FOCI_APP"^^xsd:anyURI ;
		schema:license "https://creativecommons.org/licenses/by/4.0/"^^xsd:anyURI ;
		schema:softwareVersion "1.0";
		schema:keywords "source parameters", "source mechanism", "moment tensor";
		dcat:theme <epos:SourceParameterEstimation>;
.

	<anthropogenic_hazards/software/Trmloc> a schema:SoftwareApplication;
		schema:identifier "anthropogenic_hazards/software/Trmloc" ;
		schema:identifier [ a schema:PropertyValue ;
			schema:propertyID  "DDSS-ID" ;
		  	schema:value "WP14-DDSS-A28" ;
		];
		schema:name "Localization" ;
		schema:description "Performs localization/re-localization of seismic events hypocenters" ;
  		schema:contactPoint  <https://orcid.org/0000-0002-9824-7962/contactPoint> ;
		schema:mainEntityOfPage "https://tcs.ah-epos.eu/#app:Trmloc"^^xsd:anyURI ;
		schema:license "https://creativecommons.org/licenses/by/4.0/"^^xsd:anyURI ;
		schema:softwareVersion "1.0";
		schema:keywords "source parameters", "source location";
		dcat:theme <epos:SourceParameterEstimation>;
.

	<anthropogenic_hazards/software/StressMaps> a schema:SoftwareApplication;
		schema:identifier "anthropogenic_hazards/software/StressMaps" ;
		schema:identifier [ a schema:PropertyValue ;
			schema:propertyID  "DDSS-ID" ;
		  	schema:value "WP14-DDSS-A29" ;
		];
		schema:name "Fracture Network Models – Mechanical Stresses" ;
		schema:description "Interactively plot stress patterns associated with the hydraulic fracturing of a shale gas well." ;
  		schema:contactPoint  <https://orcid.org/0000-0002-9824-7962/contactPoint> ;
		schema:mainEntityOfPage "https://tcs.ah-epos.eu/#app:StressMaps"^^xsd:anyURI ;
		schema:license "https://creativecommons.org/licenses/by-sa/4.0/"^^xsd:anyURI ;
		schema:softwareVersion "1.0";
		schema:keywords "stress modelling", "geo-resource production impact", "production - seismicity interaction";
		dcat:theme <epos:Visualizations>;
.

	<anthropogenic_hazards/software/MsatsiPlot> a schema:SoftwareApplication;
		schema:identifier "anthropogenic_hazards/software/MsatsiPlot" ;
		schema:identifier [ a schema:PropertyValue ;
			schema:propertyID  "DDSS-ID" ;
		  	schema:value "WP14-DDSS-A30" ;
		];
		schema:name "Stress Inversion" ;
		schema:description "Evaluates stress axis orientation and relative stress magnitude by inverting focal mechanisms" ;
  		schema:contactPoint  <https://orcid.org/0000-0002-9824-7962/contactPoint> ;
		schema:mainEntityOfPage "https://tcs.ah-epos.eu/#app:MsatsiPlot"^^xsd:anyURI ;
		schema:license "https://creativecommons.org/licenses/by/4.0/"^^xsd:anyURI ;
		schema:softwareVersion "1.0";
		schema:keywords "source mechanism", "moment tensor", "stress inversion";
		dcat:theme <epos:StressFieldModeling>;
.

	<anthropogenic_hazards/software/Autocorrelation> a schema:SoftwareApplication;
		schema:identifier "anthropogenic_hazards/software/Autocorrelation" ;
		schema:identifier [ a schema:PropertyValue ;
			schema:propertyID  "DDSS-ID" ;
		  	schema:value "WP14-DDSS-A31" ;
		];
		schema:name "Autocorrelation" ;
		schema:description "Autocorrelation of a time series" ;
  		schema:contactPoint  <https://orcid.org/0000-0002-9824-7962/contactPoint> ;
		schema:mainEntityOfPage "https://tcs.ah-epos.eu/#app:Autocorrelation"^^xsd:anyURI ;
		schema:license "https://creativecommons.org/licenses/by/4.0/"^^xsd:anyURI ;
		schema:softwareVersion "1.0";
		schema:keywords "statistical analysis", "statistical properties of seismicity";
		dcat:theme <epos:CorrelationAnalysis>;
.

	<anthropogenic_hazards/software/MatsumuraTest> a schema:SoftwareApplication;
		schema:identifier "anthropogenic_hazards/software/MatsumuraTest" ;
		schema:identifier [ a schema:PropertyValue ;
			schema:propertyID  "DDSS-ID" ;
		  	schema:value "WP14-DDSS-A32" ;
		];
		schema:name "Coefficient of Randomness" ;
		schema:description "A statistical test to express changes in seismicity patterns by means of an objective criterion. The Matsumura Test provides the parameter of Matsumura, value of the parameter in 5% and 95% percentile and the patterns classification as regular, completely random, and clustered." ;
  		schema:contactPoint  <https://orcid.org/0000-0002-9824-7962/contactPoint> ;
		schema:mainEntityOfPage "https://tcs.ah-epos.eu/#app:MatsumuraTest"^^xsd:anyURI ;
		schema:license "https://creativecommons.org/licenses/by/4.0/"^^xsd:anyURI ;
		schema:softwareVersion "1.0";
		schema:keywords "statistical analysis", "statistical properties of seismicity";
		dcat:theme <epos:CollectivePropertiesOfSeismicityAnalysis>;
.

	<anthropogenic_hazards/software/Crosscorrelation> a schema:SoftwareApplication;
		schema:identifier "anthropogenic_hazards/software/Crosscorrelation" ;
		schema:identifier [ a schema:PropertyValue ;
			schema:propertyID  "DDSS-ID" ;
		  	schema:value "WP14-DDSS-A33" ;
		];
		schema:name "Cross Correlation" ;
		schema:description "Cross-correlation of two time series" ;
  		schema:contactPoint  <https://orcid.org/0000-0002-9824-7962/contactPoint> ;
		schema:mainEntityOfPage "https://tcs.ah-epos.eu/#app:Crosscorrelation"^^xsd:anyURI ;
		schema:license "https://creativecommons.org/licenses/by/4.0/"^^xsd:anyURI ;
		schema:softwareVersion "1.0";
		schema:keywords "statistical analysis", "statistical properties of seismicity", "geo-resource production impact", "production – seismicity interaction";
		dcat:theme <epos:CorrelationAnalysis>;
.

	<anthropogenic_hazards/software/PSRTest> a schema:SoftwareApplication;
		schema:identifier "anthropogenic_hazards/software/PSRTest" ;
		schema:identifier [ a schema:PropertyValue ;
			schema:propertyID  "DDSS-ID" ;
		  	schema:value "WP14-DDSS-A34" ;
		];
		schema:name "Priestley-Subba Rao (PRS) Test" ;
		schema:description "Test for a time series stationarity testing" ;
  		schema:contactPoint  <https://orcid.org/0000-0002-9824-7962/contactPoint> ;
		schema:mainEntityOfPage "https://tcs.ah-epos.eu/#app:PSRTest"^^xsd:anyURI ;
		schema:license "https://creativecommons.org/licenses/by/4.0/"^^xsd:anyURI ;
		schema:softwareVersion "1.0";
		schema:keywords "statistical analysis", "statistical properties of seismicity";
		dcat:theme <epos:CollectivePropertiesOfSeismicityAnalysis>;
.

	<anthropogenic_hazards/software/CsvToCatalog> a schema:SoftwareApplication;
		schema:identifier "anthropogenic_hazards/software/CsvToCatalog" ;
		schema:identifier [ a schema:PropertyValue ;
			schema:propertyID  "DDSS-ID" ;
		  	schema:value "WP14-DDSS-A35" ;
		];
		schema:name "CSV to Catalog converter" ;
		schema:description "Tool for conversion of a CSV file into a Catalog in IS-EPOS Platform format. The csv file should use ';' as delimiter, and should include header line with names of the columns." ;
  		schema:contactPoint  <https://orcid.org/0000-0002-9824-7962/contactPoint> ;
		schema:mainEntityOfPage "https://tcs.ah-epos.eu/#app:CsvToCatalog"^^xsd:anyURI ;
		schema:license "https://creativecommons.org/licenses/by/4.0/"^^xsd:anyURI ;
		schema:softwareVersion "1.0";
		schema:keywords "converter";
		dcat:theme <epos:Converters>;
.

	<anthropogenic_hazards/software/EffDropApp> a schema:SoftwareApplication;
		schema:identifier "anthropogenic_hazards/software/EffDropApp" ;
		schema:identifier [ a schema:PropertyValue ;
			schema:propertyID  "DDSS-ID" ;
		  	schema:value "WP14-DDSS-A36" ;
		];
		schema:name "Effective Stress Drop Estimate" ;
		schema:description "Estimate of the scaling between total seismic moment and areal extent of earthquake cluster, which depends on the average stress drop released during the seismic sequence." ;
  		schema:contactPoint  <https://orcid.org/0000-0002-9824-7962/contactPoint> ;
		schema:mainEntityOfPage "https://tcs.ah-epos.eu/#app:EffDropApp"^^xsd:anyURI ;
		schema:license "https://creativecommons.org/licenses/by/4.0/"^^xsd:anyURI ;
		schema:softwareVersion "1.0";
		schema:keywords "source parameters", "statistical properties of seismicity";
		dcat:theme <epos:SourceParameterEstimation>;
.

	<anthropogenic_hazards/software/BasicVectorOperations> a schema:SoftwareApplication;
		schema:identifier "anthropogenic_hazards/software/BasicVectorOperations" ;
		schema:identifier [ a schema:PropertyValue ;
			schema:propertyID  "DDSS-ID" ;
		  	schema:value "WP14-DDSS-A37" ;
		];
		schema:name "Basic Vector Operations" ;
		schema:description "Tool for performing simple predefined operations on a given double vector" ;
  		schema:contactPoint  <https://orcid.org/0000-0002-9824-7962/contactPoint> ;
		schema:mainEntityOfPage "https://tcs.ah-epos.eu/#app:BasicVectorOperations"^^xsd:anyURI ;
		schema:license "https://creativecommons.org/licenses/by/4.0/"^^xsd:anyURI ;
		schema:softwareVersion "1.0";
		schema:keywords "vector operations";
		dcat:theme <epos:Dataprocessingapplications>;
.

	<anthropogenic_hazards/software/MmaxEstimate> a schema:SoftwareApplication;
		schema:identifier "anthropogenic_hazards/software/MmaxEstimate" ;
		schema:identifier [ a schema:PropertyValue ;
			schema:propertyID  "DDSS-ID" ;
		  	schema:value "WP14-DDSS-A38" ;
		];
		schema:name "Estimate of Maximum Possible Magnitude from Induced Deformation" ;
		schema:description "This application estimates an occurrence probability for an event of a given maximum magnitude over a period of time. It also estimates maximum possible magnitude from the size of the geo-resource reservoir, represented by the reservoir length (Grasso et al.2018), using M(Lr) relationship for earthquake (e.g. Wells Coppersmith 1994)." ;
  		schema:contactPoint  <https://orcid.org/0000-0002-9824-7962/contactPoint> ;
		schema:mainEntityOfPage "https://tcs.ah-epos.eu/#app:MmaxEstimate"^^xsd:anyURI ;
		schema:license "https://creativecommons.org/licenses/by/4.0/"^^xsd:anyURI ;
		schema:softwareVersion "1.0";
		schema:keywords "probabilistic seismic hazard analysis", "stationary hazard", "time-dependent hazard", "production-dependent hazard", "hazard analysis";
		dcat:theme <epos:Visualizations>;
.

	<anthropogenic_hazards/software/GMPEEqsCalc> a schema:SoftwareApplication;
		schema:identifier "anthropogenic_hazards/software/GMPEEqsCalc" ;
		schema:identifier [ a schema:PropertyValue ;
			schema:propertyID  "DDSS-ID" ;
		  	schema:value "WP14-DDSS-A39" ;
		];
		schema:name "Ground Motion Prediction Equations: GMPE calculation" ;
		schema:description "To estimate ground motion prediction equation (GMPE). The GMPE relates ground motion parameters, usually amplitude parameters, to sets of independent variables representing the cause of the motion. The following independent variables could be taken into account: characteristic of the path, source and site. Moreover, the non-linearity of ground vibration propagation on short distances from the epicenter is supported by using 'h' as the common/fix depth so that the standard error of estimation is minimised. The final model is estimated using ordinary one-stage regression method in three steps, including the statistical and physical consistency of the model, estimation of the fixed depth (if it's chosen as a parameter) and residuals analysis." ;
  		schema:contactPoint  <https://orcid.org/0000-0002-9824-7962/contactPoint> ;
		schema:mainEntityOfPage "https://tcs.ah-epos.eu/#app:GMPEEqsCalc"^^xsd:anyURI ;
		schema:license "https://creativecommons.org/licenses/by/4.0/"^^xsd:anyURI ;
		schema:softwareVersion "1.0";
		schema:keywords "ground motion prediction equations";
		dcat:theme <epos:ProbabilisticSeismicHazardAnalysis>;
.

	<anthropogenic_hazards/software/GMPEResidualsAnalysis> a schema:SoftwareApplication;
		schema:identifier "anthropogenic_hazards/software/GMPEResidualsAnalysis" ;
		schema:identifier [ a schema:PropertyValue ;
			schema:propertyID  "DDSS-ID" ;
		  	schema:value "WP14-DDSS-A49" ;
		];
		schema:name "Ground Motion Prediction Equations: Residuals analysis" ;
		schema:description "This step analyzes the residuals of the model (observed minus estimated values). Normality of residuals are investigated and suitable plots are shown. The outliers were shown and chosen one can be removed." ;
  		schema:contactPoint  <https://orcid.org/0000-0002-9824-7962/contactPoint> ;
		schema:mainEntityOfPage "https://tcs.ah-epos.eu/#app:GMPEResidualsAnalysis"^^xsd:anyURI ;
		schema:license "https://creativecommons.org/licenses/by/4.0/"^^xsd:anyURI ;
		schema:softwareVersion "1.0";
		schema:keywords "ground motion prediction equations";
		dcat:theme <epos:ProbabilisticSeismicHazardAnalysis>;
.

	<anthropogenic_hazards/software/GMPEFinalModel> a schema:SoftwareApplication;
		schema:identifier "anthropogenic_hazards/software/GMPEFinalModel" ;
		schema:identifier [ a schema:PropertyValue ;
			schema:propertyID  "DDSS-ID" ;
		  	schema:value "WP14-DDSS-A13" ;
		];
		schema:name "Ground Motion Prediction Equations: Final model analysis" ;
		schema:description "The final Model of the Ground Motion Prediction Equation is summarized with additional plots." ;
  		schema:contactPoint  <https://orcid.org/0000-0002-9824-7962/contactPoint> ;
		schema:mainEntityOfPage "https://tcs.ah-epos.eu/#app:GMPEFinalModel"^^xsd:anyURI ;
		schema:license "https://creativecommons.org/licenses/by/4.0/"^^xsd:anyURI ;
		schema:softwareVersion "1.0";
		schema:keywords "ground motion prediction equations";
		dcat:theme <epos:ProbabilisticSeismicHazardAnalysis>;
.

	<anthropogenic_hazards/software/BackProjection> a schema:SoftwareApplication;
		schema:identifier "anthropogenic_hazards/software/BackProjection" ;
		schema:identifier [ a schema:PropertyValue ;
			schema:propertyID  "DDSS-ID" ;
		  	schema:value "WP14-DDSS-A40" ;
		];
		schema:name "Waveform-based seismic event location" ;
		schema:description "This application implements a location procedure which allows imaging the distribution of seismic sources in both time and space. First, a characteristic function (CF; in this case, the STA/LTA ratio) is calculated at all the vertical-component seismograms from the selected stations. The user then define a volume likely containing the source(s), and a number of grid nodes along the two horizontal (NS-EW) and vertical coordinates for discretising this volume. For each grid node located at the arbitrary location (x,y,z), the predicted arrival times are calculated at all the stations, and the different CFs are time-shifted consequently. By stacking these time-shifted CFs one obtains a time-dependent Brightness function associated with that particular grid node. The procedure is iterated over all the grid nodes of the source volume; at the end of the process, the maximum (maxima) of the Brightness function will provide an estimate of the source location and origin time. The main advantage of this procedure is that it exploits waveform information (both arrival times and relative amplitudes) without the need of pre-assembled phase-picking data. The method, therefore, is particularly well-suited for emergent signals and/or for real-time applications. The technique has been largely inspired by the previous works from Kao and Shan (2004), Grigoli et al. (2013, 2014), Langet et al., (2014), to which the reader is referred for a more comprehensive description of the methodology." ;
  		schema:contactPoint  <https://orcid.org/0000-0002-9824-7962/contactPoint> ;
		schema:mainEntityOfPage "https://tcs.ah-epos.eu/#app:BackProjection"^^xsd:anyURI ;
		schema:license "https://creativecommons.org/licenses/by/4.0/"^^xsd:anyURI ;
		schema:softwareVersion "1.0";
		schema:keywords "source location", "hypocenter location";
		dcat:theme <epos:SourceParameterEstimation>;
.

	<anthropogenic_hazards/software/Merger> a schema:SoftwareApplication;
		schema:identifier "anthropogenic_hazards/software/Merger" ;
		schema:identifier [ a schema:PropertyValue ;
			schema:propertyID  "DDSS-ID" ;
		  	schema:value "WP14-DDSS-A41" ;
		];
		schema:name "MERGER: Dynamic risk analysis using a bow-tie approach" ;
		schema:description "MERGER, a simulator for multi-hazard risk assessment in ExploRation/exploitation of GeoResources, is a tool for performing dynamic risk analyses using a bow-tie approach. The tool has been designed for solving fault trees (FT) and event trees (ET) linked in a bow-tie structure and using a Monte Carlo approach." ;
  		schema:contactPoint  <https://orcid.org/0000-0002-9824-7962/contactPoint> ;
		schema:mainEntityOfPage "https://tcs.ah-epos.eu/#app:Merger"^^xsd:anyURI ;
		schema:license "https://creativecommons.org/licenses/by/4.0/"^^xsd:anyURI ;
		schema:softwareVersion "1.0";
		schema:keywords "dynamic bow-tie analysis", "fault-tree", "event-tree", "statistical analysis", "multi-hazard risk assessment", "Monte Carlo simulations", "Geo-resource production impact";
		dcat:theme <epos:ProbabilisticSeismicHazardAnalysis>;
.

	<anthropogenic_hazards/software/GeoresourceLengthAnalysisApp> a schema:SoftwareApplication;
		schema:identifier "anthropogenic_hazards/software/GeoresourceLengthAnalysisApp" ;
		schema:identifier [ a schema:PropertyValue ;
			schema:propertyID  "DDSS-ID" ;
		  	schema:value "WP14-DDSS-A42" ;
		];
		schema:name "Earthquake interactions: Georesource scale" ;
		schema:description "Anthropogenic seismicity rate and magnitude are analyzed using superposed epoch to extract mean field patterns that are more robust than a single serie. This application analyse aftershocks sequence in the 1-3L near field distances from the “reservoir”. L is a proxy for georesource dimension, being mine gallery width, reservoir length , etc... Input data are time series from seismicity catalogue. This application is important to quantify the mean field pattern of several aftershocks to be compared with regional tectonic patterns" ;
  		schema:contactPoint  <https://orcid.org/0000-0002-9824-7962/contactPoint> ;
		schema:mainEntityOfPage "https://tcs.ah-epos.eu/#app:GeoresourceLengthAnalysisApp"^^xsd:anyURI ;
		schema:license "https://creativecommons.org/licenses/by/4.0/"^^xsd:anyURI ;
		schema:softwareVersion "1.0";
		schema:keywords "geo-resource production impact", "statistical properties of seismicity", "mainshock", "aftershock";
		dcat:theme <epos:EarthquakeInteractionsAnalysis>;
.

	<anthropogenic_hazards/software/MagnitudinalLengthAnalysisApp> a schema:SoftwareApplication;
		schema:identifier "anthropogenic_hazards/software/MagnitudinalLengthAnalysisApp" ;
		schema:identifier [ a schema:PropertyValue ;
			schema:propertyID  "DDSS-ID" ;
		  	schema:value "WP14-DDSS-A43" ;
		];
		schema:name "Earthquake interactions: Mainshock scale" ;
		schema:description "Anthropogenic seismicity rate and magnitude are analyzed using superposed epochs to extract mean field patterns that are more robust than a single serie. This application analyse aftershocks sequence in the 1-3L near field distances, L being the Fault length for the earthquake mainshocks. Input data are time series from seismicity catalogue. This application is important to quantify the mean field pattern of aftershock production to be compared with regional tectonic patterns" ;
  		schema:contactPoint  <https://orcid.org/0000-0002-9824-7962/contactPoint> ;
		schema:mainEntityOfPage "https://tcs.ah-epos.eu/#app:MagnitudinalLengthAnalysisApp"^^xsd:anyURI ;
		schema:license "https://creativecommons.org/licenses/by/4.0/"^^xsd:anyURI ;
		schema:softwareVersion "1.0";
		schema:keywords "geo-resource production impact", "statistical properties of seismicity", "mainshock", "aftershock";
		dcat:theme <epos:EarthquakeInteractionsAnalysis>;
.

	<anthropogenic_hazards/software/EarthquakeReshufflingAnalysisApp> a schema:SoftwareApplication;
		schema:identifier "anthropogenic_hazards/software/EarthquakeReshufflingAnalysisApp" ;
		schema:identifier [ a schema:PropertyValue ;
			schema:propertyID  "DDSS-ID" ;
		  	schema:value "WP14-DDSS-A44" ;
		];
		schema:name "Earthquake interactions: Earthquake swarm / reshuffling analysis" ;
		schema:description "Anthropogenic seismicity rate and magnitude are tested against non correlated series with the same number of data. It is achieved by 'reshuffling' the data. It is a robust way to check how significant is the variability over time of anthropogenic seismicity. Input data are time series from seismicity catalogue. This application is important to quantify the robustness of observed seismicity pattern against random fluctuations of the same size system Outputs are observed and reshuffled time series.";
  		schema:contactPoint  <https://orcid.org/0000-0002-9824-7962/contactPoint> ;
		schema:mainEntityOfPage "https://tcs.ah-epos.eu/#app:EarthquakeReshufflingAnalysisApp"^^xsd:anyURI ;
		schema:license "https://creativecommons.org/licenses/by/4.0/"^^xsd:anyURI ;
		schema:softwareVersion "1.0";
		schema:keywords "geo-resource production impact", "statistical properties of seismicity", "earthquake swarm";
		dcat:theme <epos:EarthquakeInteractionsAnalysis>;
.

	<anthropogenic_hazards/software/SeasonalTrendApp> a schema:SoftwareApplication;
		schema:identifier "anthropogenic_hazards/software/SeasonalTrendApp" ;
		schema:identifier [ a schema:PropertyValue ;
			schema:propertyID  "DDSS-ID" ;
		  	schema:value "WP14-DDSS-A46" ;
		];
		schema:name "Earthquake interactions: Time correlated earthquakes (Seasonal trends)" ;
		schema:description "Test of of Number, space, and Magnitude pattern against reshuffled distribution in time e.g daily patterns for mine induced seismicity or monthly pattern for reservoir induced seismicity. The test aims to quantify how “seasonal” patterns remain uniform over time and to accept or to reject the uniform pattern under a given confidence level. Allows to capture anthropogenic trends in time pattern that correspond to geo-resource production type. It allows to extract time relationship to production patterns and departure from uniform tectonic seismicity background. Input data are time series from seismicity catalogue. Outputs are time series tested against reshuffled series .";
  		schema:contactPoint  <https://orcid.org/0000-0002-9824-7962/contactPoint> ;
		schema:mainEntityOfPage "https://tcs.ah-epos.eu/#app:SeasonalTrendApp"^^xsd:anyURI ;
		schema:license "https://creativecommons.org/licenses/by/4.0/"^^xsd:anyURI ;
		schema:softwareVersion "1.0";
		schema:keywords "geo-resource production impact", "statistical properties of seismicity", "seasonal trend";
		dcat:theme <epos:EarthquakeInteractionsAnalysis>;
.

	<anthropogenic_hazards/software/DoubleCoupleMomentTensorInversion> a schema:SoftwareApplication;
		schema:identifier "anthropogenic_hazards/software/DoubleCoupleMomentTensorInversion" ;
		schema:identifier [ a schema:PropertyValue ;
			schema:propertyID  "DDSS-ID" ;
		  	schema:value "WP14-DDSS-A45" ;
		];
		schema:name "Mechanism: Shear slip" ;
		schema:description "The program performs inversion of amplitudes of longitudinal (P) and transversal (S) seismic waves as 3-component vectors into the mechanism of the seismic source in the description of a double couple using a grid search across the full or a priori specified range of the fault-plane solution angles.";
  		schema:contactPoint  <https://orcid.org/0000-0002-9824-7962/contactPoint> ;
		schema:mainEntityOfPage "https://tcs.ah-epos.eu/#app:DoubleCoupleMomentTensorInversion"^^xsd:anyURI ;
		schema:license "https://creativecommons.org/licenses/by/4.0/"^^xsd:anyURI ;
		schema:softwareVersion "1.0";
		schema:keywords "seismic event mechanism", "shear slip along a fault", "inversion of P an/or S amplitudes", "grid search";
		dcat:theme <epos:SourceParameterEstimation>;
.

	<anthropogenic_hazards/software/MomentTensorInversion> a schema:SoftwareApplication;
		schema:identifier "anthropogenic_hazards/software/MomentTensorInversion" ;
		schema:identifier [ a schema:PropertyValue ;
			schema:propertyID  "DDSS-ID" ;
		  	schema:value "WP14-DDSS-A51" ;
		];
		schema:name "Mechanism: Full Moment Tensor" ;
		schema:description "The program performs inversion of amplitudes of longitudinal (P) and transversal (S) seismic waves as 3-component vectors into the mechanism of the seismic source in the description of unconstrained moment tensor (MT). As such, it allows describe general dipole sources including isotropic components: e.g., it is suitable to retrieve the parameters of both a shear dislocation common at foci of tectonic earthquakes (described as a double-couple, DC) and volumetric sources as tensile cracks or cavity implosions. It provides the MT error estimate: evaluates the data covariance matrix based on standard deviations of individual components of P and S motion. The application is designed preferentially for processing of seismic events induced by industrial activity (mining, hydro-fracture test in geothermal and oil wells etc.).";
  		schema:contactPoint  <https://orcid.org/0000-0002-9824-7962/contactPoint> ;
		schema:mainEntityOfPage "https://tcs.ah-epos.eu/#app:MomentTensorInversion"^^xsd:anyURI ;
		schema:license "https://creativecommons.org/licenses/by/4.0/"^^xsd:anyURI ;
		schema:softwareVersion "1.0";
		schema:keywords "seismic event mechanism", "linear inversion of P an/or S amplitudes", "full moment tensor", "decomposition into elementary components";
		dcat:theme <epos:SourceParameterEstimation>;
.

	<anthropogenic_hazards/software/ShearTensileCrackInversion> a schema:SoftwareApplication;
		schema:identifier "anthropogenic_hazards/software/ShearTensileCrackInversion" ;
		schema:identifier [ a schema:PropertyValue ;
			schema:propertyID  "DDSS-ID" ;
		  	schema:value "WP14-DDSS-A52" ;
		];
		schema:name "Mechanism: Shear-Tensile crack" ;
		schema:description "The program performs inversion of amplitudes of longitudinal (P) and transversal (S) seismic waves as 3-component vectors into the mechanism of the seismic source in the description of shear-tensile crack (STC).";
  		schema:contactPoint  <https://orcid.org/0000-0002-9824-7962/contactPoint> ;
		schema:mainEntityOfPage "https://tcs.ah-epos.eu/#app:ShearTensileCrackInversion"^^xsd:anyURI ;
		schema:license "https://creativecommons.org/licenses/by/4.0/"^^xsd:anyURI ;
		schema:softwareVersion "1.0";
		schema:keywords "seismic event mechanism", "crack source model", "shear-slip and crack opening/closing", "inversion of P an/or S amplitudes", "grid search";
		dcat:theme <epos:SourceParameterEstimation>;
.

	<anthropogenic_hazards/software/StressChanges> a schema:SoftwareApplication;
		schema:identifier "anthropogenic_hazards/software/StressChanges" ;
		schema:identifier [ a schema:PropertyValue ;
			schema:propertyID  "DDSS-ID" ;
		  	schema:value "WP14-DDSS-A47" ;
		];
		schema:name "Stress and strain changes induced by fluid injection and temperature change driven by geothermal injection" ;
		schema:description "Prediction of the temperature and Coulomb stress changes in a deep reservoir with hydro-thermal circulation and thermo-poro-elastic effects. Methodology: 2D THM model (code_Aster, open source), gmsh, gnuplot, python.";
  		schema:contactPoint  <https://orcid.org/0000-0002-9824-7962/contactPoint> ;
		schema:mainEntityOfPage "https://tcs.ah-epos.eu/#app:StressChanges"^^xsd:anyURI ;
		schema:license "https://creativecommons.org/licenses/by/4.0/"^^xsd:anyURI ;
		schema:softwareVersion "1.0";
		schema:keywords "Coulomb stress changes";
		dcat:theme <epos:CollectivePropertiesOfSeismicityAnalysis>;
.

	<anthropogenic_hazards/software/MultipletIdentification> a schema:SoftwareApplication;
		schema:identifier "anthropogenic_hazards/software/MultipletIdentification" ;
		schema:identifier [ a schema:PropertyValue ;
			schema:propertyID  "DDSS-ID" ;
		  	schema:value "WP14-DDSS-A48" ;
		];
		schema:name "Template-matching based detection algorithm" ;
		schema:description "Detection of events by template matching. Template datasets (picked events) are correlated with the continuous seismic records to identify new events.";
  		schema:contactPoint  <https://orcid.org/0000-0002-9824-7962/contactPoint> ;
		schema:mainEntityOfPage "https://tcs.ah-epos.eu/#app:MultipletIdentification"^^xsd:anyURI ;
		schema:license "https://creativecommons.org/licenses/by/4.0/"^^xsd:anyURI ;
		schema:softwareVersion "1.0";
		schema:keywords "aftershocks", "earthquake swarm", "data selection";
		dcat:theme <epos:EventDetectionAlgorithms>;
.

	<anthropogenic_hazards/software/CatalogToAscii> a schema:SoftwareApplication;
		schema:identifier "anthropogenic_hazards/software/CatalogToAscii" ;
		schema:identifier [ a schema:PropertyValue ;
			schema:propertyID  "DDSS-ID" ;
		  	schema:value "WP14-DDSS-A50" ;
		];
		schema:name "Catalog to ASCII converter" ;
		schema:description "Application that transforms a seismic or ground motion catalog to ASCII format";
  		schema:contactPoint  <https://orcid.org/0000-0002-9824-7962/contactPoint> ;
		schema:mainEntityOfPage "https://tcs.ah-epos.eu/#app:CatalogToAscii"^^xsd:anyURI ;
		schema:license "https://creativecommons.org/licenses/by/4.0/"^^xsd:anyURI ;
		schema:softwareVersion "1.0";
		schema:keywords "format conversion, data download, data export";
		dcat:theme <epos:Converters>;
.

	<http://orcid.org/0000-0002-4801-4888/contactPoint> a schema:ContactPoint;
		schema:email "lizurek@igf.edu.pl";
		schema:availableLanguage "en" ;
		schema:contactType "contactPoint" ;
. 
	<mailto:m.sterzel@cyfronet.pl/contactPoint> a schema:ContactPoint;
		schema:email "m.sterzel@cyfronet.pl";
		schema:availableLanguage "en" ;
		schema:contactType "contactPoint" ;
. 
	<https://orcid.org/0000-0002-9824-7962/contactPoint> a schema:ContactPoint;
		schema:email "j.kocot@cyfronet.pl";
		schema:availableLanguage "en" ;
		schema:contactType "contactPoint" ;
. 
	<mailto:a_blanke@gfz-potsdam.de/contactPoint> a schema:ContactPoint;
		schema:email "a_blanke@gfz-potsdam.de";
		schema:availableLanguage "en" ;
		schema:contactType "contactPoint" ;
. 
	<http://orcid.org/0000-0003-1076-615X/contactPoint> a schema:ContactPoint;
		schema:email "kwiatek@gfz-potsdam.de";
		schema:availableLanguage "en" ;
		schema:contactType "contactPoint" ;
. 
	<mailto:giangnv@igp-vast.vn/contactPoint> a schema:ContactPoint;
		schema:email "giangnv@igp-vast.vn";
		schema:availableLanguage "en" ;
		schema:contactType "contactPoint" ;
. 
	<http://orcid.org/0000-0001-8181-0758/contactPoint> a schema:ContactPoint;
		schema:email "gmutke@gig.eu";
		schema:availableLanguage "en" ;
		schema:contactType "contactPoint" ;
. 
	<mailto:jannes-l.kinscher@ineris.fr/contactPoint> a schema:ContactPoint;
		schema:email "jannes-l.kinscher@ineris.fr";
		schema:availableLanguage "en" ;
		schema:contactType "contactPoint" ;
. 
	<mailto:jouni.nevalainen@oulu.fi/contactPoint> a schema:ContactPoint;
		schema:email "jouni.nevalainen@oulu.fi";
		schema:availableLanguage "en" ;
		schema:contactType "contactPoint" ;
. 
	<http://orcid.org/0000-0003-2915-1446/contactPoint> a schema:ContactPoint;
		schema:email "gilberto.saccorotti@ingv.it";
		schema:availableLanguage "en" ;
		schema:contactType "contactPoint" ;
. 
	<http://orcid.org/0000-0003-3844-5059/contactPoint> a schema:ContactPoint;
		schema:email "pamela.roselli@ingv.it";
		schema:availableLanguage "en" ;
		schema:contactType "contactPoint" ;
.
	<http://orcid.org/0000-0001-9196-8452/contactPoint> a schema:ContactPoint;
		schema:email "alexander.garcia@ingv.it";
		schema:availableLanguage "en" ;
		schema:contactType "contactPoint" ;
.
	<http://orcid.org/0000-0002-0769-5277/contactPoint> a schema:ContactPoint;
		schema:email "g.m.jones@keele.ac.uk";
		schema:availableLanguage "en" ;
		schema:contactType "contactPoint" ;
.
	<http://orcid.org/0000-0002-9580-7864/contactPoint> a schema:ContactPoint;
		schema:email "jean-robert.grasso@univ-grenoble-alpes.fr";
		schema:availableLanguage "en" ;
		schema:contactType "contactPoint" ;
.
	<mailto:abror.karimov@univ-grenoble-alpes.fr/contactPoint> a schema:ContactPoint;
		schema:email "abror.karimov@univ-grenoble-alpes.fr";
		schema:availableLanguage "en" ;
		schema:contactType "contactPoint" ;
.
	<https://orcid.org/0000-0001-8078-9416/contactPoint> a schema:ContactPoint;
		schema:email "matteo.picozzi@unina.it";
		schema:availableLanguage "en" ;
		schema:contactType "contactPoint" ;
.
	<http://orcid.org/0000-0001-7153-5115/contactPoint> a schema:ContactPoint;
		schema:email "E.N.Ruigrok@uu.nl";
		schema:availableLanguage "en" ;
		schema:contactType "contactPoint" ;
.
	<https://orcid.org/0000-0003-2989-1663/contactPoint> a schema:ContactPoint;
		schema:email "sandra.osk.snaebjornsdottir@or.is";
		schema:availableLanguage "en" ;
		schema:contactType "contactPoint" ;
.
	<mailto:thomas.bloch@sgsw.ch/contactPoint> a schema:ContactPoint;
		schema:email "thomas.bloch@sgsw.ch";
		schema:availableLanguage "en" ;
		schema:contactType "contactPoint" ;
.
	<http://orcid.org/0000-0003-4017-4673/contactPoint> a schema:ContactPoint;
		schema:email "Marc.Schaming@unistra.fr";
		schema:availableLanguage "en" ;
		schema:contactType "contactPoint" ;
.
	<mailto:Egill.Arni.Gudnason@isor.is/contactPoint> a schema:ContactPoint;
        schema:email "Egill.Arni.Gudnason@isor.is";
        schema:availableLanguage "en" ;
        schema:contactType "contactPoint" ;
.
