@prefix adms: <http://www.w3.org/ns/adms#> .
@prefix rdf: <http://www.w3.org/1999/02/22-rdf-syntax-ns#> .
@prefix epos: <https://www.epos-eu.org/epos-dcat-ap#> .
@prefix dc: <http://purl.org/dc/elements/1.1/> .
@prefix dct: <http://purl.org/dc/terms/> .
@prefix vcard: <http://www.w3.org/2006/vcard/ns#> .
@prefix hydra: <http://www.w3.org/ns/hydra/core#> .
@prefix xsd: <http://www.w3.org/2001/XMLSchema#> .
@prefix schema: <http://schema.org/> .
@prefix dcat: <http://www.w3.org/ns/dcat#> .
@prefix cnt: <http://www.w3.org/2011/content#> .
@prefix locn: <http://www.w3.org/ns/locn#> .
@prefix skos: <http://www.w3.org/2004/02/skos/core#> .
@prefix rdfs: <http://www.w3.org/2000/01/rdf-schema#> .
@prefix http: <http://www.w3.org/2006/http#> .
@prefix owl: <http://www.w3.org/2002/07/owl#> .
@prefix gsp: <http://www.opengis.net/ont/geosparql#> .


<PIC:999472675> a schema:Organization;
	schema:identifier [ a schema:PropertyValue;
		schema:propertyID "PIC";
		schema:value "999472675";
	];
	schema:legalName "Instituto Nazionale di Geofisica e Vulcanologia";
	schema:address [ a schema:PostalAddress;
		schema:streetAddress "Via di Vigna Murata 605";
		schema:addressLocality "Rome";
		schema:postalCode "00143";
		schema:addressCountry "italy";
	];
	schema:logo "https://data.ingv.it/images/logos/logo_ingv_vertical_two_lines.png"^^xsd:anyURI;
	schema:url "http://www.ingv.it"^^xsd:anyURI;
	schema:email "ufficiogestionedati@ingv.it";
	schema:contactPoint <http://orcid.org/0000-0002-1213-0828/scientificContact>;
	schema:contactPoint <http://orcid.org/0000-0002-8651-6387/legalContact>;
	schema:contactPoint <http://orcid.org/0000-0003-1208-9412/contactPoint>;
.

<http://orcid.org/0000-0002-8651-6387> a schema:Person;
	schema:identifier [ a schema:PropertyValue;
		schema:propertyID "orcid";
		schema:value "http://orcid.org/0000-0002-8651-6387";
	];
	schema:familyName "Doglioni";
	schema:givenName "Carlo";
	schema:address [ a schema:PostalAddress;
		schema:streetAddress "Via di Vigna Murata 605";
		schema:addressLocality "Rome";
		schema:postalCode "00143";
		schema:addressCountry "Italy";
	];
	schema:email "segreteria.presidenza@ingv.it";
	schema:qualifications "Professor";
	schema:affiliation <PIC:999472675>;
	schema:contactPoint <http://orcid.org/0000-0002-8651-6387/legalContact>;
.

<http://orcid.org/0000-0002-1213-0828> a schema:Person;
	schema:identifier [ a schema:PropertyValue;
		schema:propertyID "orcid";
		schema:value "http://orcid.org/0000-0002-1213-0828";
	];
	schema:familyName "Basili";
	schema:givenName "Roberto";
	schema:address [ a schema:PostalAddress;
		schema:streetAddress "Via di Vigna Murata 605";
		schema:addressLocality "Rome";
		schema:postalCode "00143";
		schema:addressCountry "Italy";
	];
	schema:email "roberto.basili@ingv.it";
	schema:qualifications "Senior researcher";
	schema:affiliation <PIC:999472675>;
	schema:contactPoint <http://orcid.org/0000-0002-1213-0828/scientificContact>;
.

<http://orcid.org/0000-0003-1208-9412> a schema:Person;
	schema:identifier [ a schema:PropertyValue;
		schema:propertyID "orcid";
		schema:value "http://orcid.org/0000-0003-1208-9412";
	];
	schema:familyName "Vallone";
	schema:givenName "Roberto";
	schema:address [ a schema:PostalAddress;
		schema:streetAddress "Via di Vigna Murata 605";
		schema:addressLocality "Rome";
		schema:postalCode "00143";
		schema:addressCountry "Italy";
	];
	schema:email "roberto.vallone@ingv.it";
	schema:qualifications "Technologist";
	schema:affiliation <PIC:999472675>;
	schema:contactPoint <http://orcid.org/0000-0003-1208-9412/contactPoint>;
.

	<http://services.seismofaults.eu/geoserver/EDSF> a dcat:Dataset;
		dct:title "Seismology/EDSF";
		dct:identifier "http://services.seismofaults.eu/geoserver/EDSF";
		adms:identifier [ a adms:Identifier;
			adms:schemaAgency "DDSS-ID";
			skos:notation "WP08-DDSS-038";
		];
		dct:description "The European Database of Seismogenic Faults (EDSF) was compiled in the framework of the EU Project SHARE, Work Package 3, Task 3.2. EDSF includes only faults that are deemed to be capable of generating earthquakes of magnitude equal to or larger than 5.5 and aims at ensuring a homogeneous input for use in ground-shaking hazard assessment in the Euro-Mediterranean area. Several research institutions participated in this effort with the contribution of many scientists (see the Database section for a full list). The EDSF database and website are hosted and maintained by INGV.";
		dct:created "2013-05-31"^^xsd:date;
		dct:modified "2013-05-31"^^xsd:date;
		dct:issued "2013-05-31"^^xsd:date;
	  dct:temporal [ a dct:PeriodOfTime;
			schema:startDate "2013-05-31T00:00:00Z"^^xsd:dateTime;
			#schema:endDate "YYYY-MM-DDThh:mm:ssZ"^^xsd:dateTime;
		];
		dct:spatial [ a dct:Location;
				locn:geometry "POLYGON((-12.39 30.3,-12.39 49.0,45.28 49,45.28 30.3,-12.39 30.3))"^^gsp:wktLiteral;
		];
		dcat:theme <#Activefaults>;
		dcat:keyword "active fault", "seismogenic fault", "seismogenic source", "seismogenic zone", "earthquake", "subduction", "slab", "hazard", "earthquakes", "magnitude", "slip rate", "crustal fault sources", "subduction fault sources", "hazard model", "faults", "seismology", "geology", "geohazard", "seismic hazard";
		dcat:contactPoint <http://orcid.org/0000-0003-1208-9412/contactPoint>;
		dct:publisher <PIC:999472675>;
		dcat:distribution <Seismology/EDSF/Distribution/WMS>;
		dcat:distribution <Seismology/EDSF/Distribution/WFS_CrustalFaults>;
		dcat:distribution <Seismology/EDSF/Distribution/WFS_Subductions>;
		owl:versionInfo "2013";
		dct:accrualPeriodicity "http://purl.org/cld/freq/irregular"^^xsd:anyURI ;
		dct:type "http://purl.org/dc/dcmitype/Dataset"^^xsd:anyURI ;
.

<Seismology/EDSF/Distribution/WMS> a dcat:Distribution;
	dct:identifier "Seismology/EDSF/Distribution/WMS";
	dct:title "European Database of Seismogenic Faults";
	dct:description "The European Database of Seismogenic Faults (EDSF) was compiled in the framework of the EU Project SHARE, Work Package 3, Task 3.2. EDSF includes only faults that are deemed to be capable of generating earthquakes of magnitude equal to or larger than 5.5 and aims at ensuring a homogeneous input for use in ground-shaking hazard assessment in the Euro-Mediterranean area. Several research institutions participated in this effort with the contribution of many scientists (see the Database section for a full list). The EDSF database and website are hosted and maintained by INGV.";
	dct:issued "2013-05-31"^^xsd:date;
	dct:modified "2013-05-31"^^xsd:date;
	dct:type "http://publications.europa.eu/resource/authority/distribution-type/WEB_SERVICE"^^xsd:anyURI;
	dct:conformsTo <Seismology/EDSF>;
	dcat:accessURL <Seismology/EDSF/Operation/WMS>;
	dct:license "https://creativecommons.org/licenses/by-sa/4.0/"^^xsd:anyURI ;
	dct:format "http://publications.europa.eu/resource/authority/file-type/PNG"^^xsd:anyURI;
.
<Seismology/EDSF/Distribution/WFS_CrustalFaults> a dcat:Distribution;
	dct:identifier "Seismology/EDSF/Distribution/WFS_CrustalFaults";
	dct:title "European Database of Seismogenic Faults - WFS - Crustal Faults";
	dct:description "The European Database of Seismogenic Faults (EDSF) was compiled in the framework of the EU Project SHARE, Work Package 3, Task 3.2. EDSF includes only faults that are deemed to be capable of generating earthquakes of magnitude equal to or larger than 5.5 and aims at ensuring a homogeneous input for use in ground-shaking hazard assessment in the Euro-Mediterranean area. Several research institutions participated in this effort with the contribution of many scientists (see the Database section for a full list). The EDSF database and website are hosted and maintained by INGV.";
	dct:issued "2017-01-01"^^xsd:date;
	dct:modified "2017-01-01"^^xsd:date;
	dct:type "http://publications.europa.eu/resource/authority/distribution-type/WEB_SERVICE"^^xsd:anyURI;
	dct:conformsTo <Seismology/EDSF>;
	dcat:accessURL <Seismology/EDSF/WFS-CrustalFaults>;
	dct:license "https://creativecommons.org/licenses/by-sa/4.0/"^^xsd:anyURI ;
	dct:format "http://publications.europa.eu/resource/authority/file-type/XML"^^xsd:anyURI;
.
<Seismology/EDSF/Distribution/WFS_Subductions> a dcat:Distribution;
	dct:identifier "Seismology/EDSF/Distribution/WFS_Subductions";
	dct:title "European Database of Seismogenic Faults - WFS - Subductions";
	dct:description "The European Database of Seismogenic Faults (EDSF) was compiled in the framework of the EU Project SHARE, Work Package 3, Task 3.2. EDSF includes only faults that are deemed to be capable of generating earthquakes of magnitude equal to or larger than 5.5 and aims at ensuring a homogeneous input for use in ground-shaking hazard assessment in the Euro-Mediterranean area. Several research institutions participated in this effort with the contribution of many scientists (see the Database section for a full list). The EDSF database and website are hosted and maintained by INGV.";
	dct:issued "2017-01-01"^^xsd:date;
	dct:modified "2017-01-01"^^xsd:date;
	dct:type "http://publications.europa.eu/resource/authority/distribution-type/WEB_SERVICE"^^xsd:anyURI;
	dct:conformsTo <Seismology/EDSF>;
	dcat:accessURL <Seismology/EDSF/WFS-Subductions>;
	dct:license "https://creativecommons.org/licenses/by-sa/4.0/"^^xsd:anyURI ;
	dct:format "http://publications.europa.eu/resource/authority/file-type/XML"^^xsd:anyURI;
.

<Seismology/EDSF> a epos:WebService;
	schema:identifier "Seismology/EDSF";

	schema:description "The European Database of Seismogenic Faults (EDSF) was compiled in the framework of the EU Project SHARE, Work Package 3, Task 3.2. EDSF includes only faults that are deemed to be capable of generating earthquakes of magnitude equal to or larger than 5.5 and aims at ensuring a homogeneous input for use in ground-shaking hazard assessment in the Euro-Mediterranean area. Several research institutions participated in this effort with the contribution of many scientists (see the Database section for a full list). This layer includes subduction zones. The EDSF database and website are hosted and maintained by INGV.";
	dcat:theme <#Activefaults>;
	schema:name "European Database of Seismogenic Faults";
	schema:provider <PIC:999472675>;
	schema:datePublished "2017-01-01"^^xsd:date;
	schema:dateModified "2017-01-01"^^xsd:date;
	dct:spatial [ a dct:Location;
		locn:geometry "POLYGON((-12.39 30.3,-12.39 49.0,45.28 49,45.28 30.3,-12.39 30.3))"^^gsp:wktLiteral;
	];
	hydra:supportedOperation <Seismology/EDSF/Operation/WMS>;
	hydra:supportedOperation <Seismology/EDSF/WFS-CrustalFaults>;
	hydra:supportedOperation <Seismology/EDSF/WFS-Subductions>;
	schema:keywords "active fault"," seismogenic fault"," seismogenic source"," seismogenic zone"," earthquake"," subduction"," slab"," hazard"," earthquakes"," magnitude"," slip rate"," crustal fault sources"," subduction fault sources"," hazard model"," faults"," seismology"," geology"," geohazard"," seismic hazard";
	dct:license "https://creativecommons.org/licenses/by-sa/4.0/"^^xsd:anyURI;
	dct:temporal [ a dct:PeriodOfTime;
		schema:startDate "2017-01-01T00:00:00Z"^^xsd:dateTime;
		#schema:endDate "YYYY-MM-DDThh:mm:ssZ"^^xsd:dateTime;
	];
	dcat:contactPoint <http://orcid.org/0000-0003-1208-9412/contactPoint>;
.
	<Seismology/EDSF/Operation/WMS> a hydra:Operation;
		hydra:method "GET"^^xsd:string;
		hydra:returns "image/png";
		hydra:property[ a hydra:IriTemplate;
			hydra:template "http://services.seismofaults.eu/geoserver/EDSF/ows{?service, version, request, layers, width, height, crs, format}&bbox={minlatitude, minlongitude, maxlatitude, maxlongitude}"^^xsd:string;
				hydra:mapping[ a hydra:IriTemplateMapping;
					hydra:variable "service"^^xsd:string;
					rdfs:range "xsd:string";
					rdfs:label "Service type";
					schema:defaultValue "WMS";
					http:paramValue "WMS";
					hydra:required "true"^^xsd:boolean;
				];
				hydra:mapping[ a hydra:IriTemplateMapping;
					hydra:variable "version"^^xsd:string;
					rdfs:range "xsd:string";
					rdfs:label "Service version";
					schema:defaultValue "1.3.0";
					http:paramValue "1.3.0";
					#commented out because of axis ordering difference between the two versions
					#http:paramValue "1.1.0";
					hydra:required "true"^^xsd:boolean;
				];
				hydra:mapping[ a hydra:IriTemplateMapping;
					hydra:variable "request"^^xsd:string;
					rdfs:range "xsd:string";
					rdfs:label "Request type";
					schema:defaultValue "GetMap";
					http:paramValue "GetMap";
					hydra:required "true"^^xsd:boolean;
				];
				hydra:mapping[ a hydra:IriTemplateMapping;
					hydra:variable "layers"^^xsd:string;
					rdfs:range "xsd:string";
					rdfs:label "Layer to load";
					schema:defaultValue "EDSF:EDSF";
					http:paramValue "EDSF:EDSF";
					http:paramValue "EDSF:EDSF.Crustal_Fault_Sources";
					http:paramValue "EDSF:EDSF.Subduction_Zones";
					http:paramValue "EDSF:crustal_fault_sources_top";
					http:paramValue "EDSF:crustal_fault_sources_pln";
					http:paramValue "EDSF:subduction_zones";
					http:paramValue "EDSF:subduction_contours";
					hydra:required "true"^^xsd:boolean;
				];
				
				#hydra:mapping[ a hydra:IriTemplateMapping;
				#	hydra:variable "bbox"^^xsd:string;
				#	rdfs:range "xsd:string";
				#	rdfs:label "Bounding box";
				#	schema:defaultValue "-12.3925075531006,30.303092956543,45.2800407409668,49.0013656616211";
				#	#http:paramValue "-12.3925075531006,30.303092956543,45.2800407409668,49.0013656616211";
				#	hydra:required "true"^^xsd:boolean;
				
				hydra:mapping[ a hydra:IriTemplateMapping;
					hydra:variable "minlatitude"^^xsd:string;
					hydra:property "epos:southernmostLatitude";
					rdfs:range "xsd:float";
					rdfs:label "Minimum Latitude";
					schema:minValue "-90.0";
					schema:maxValue "90.0";
					hydra:required "true"^^xsd:boolean;
					schema:defaultValue "30.303092956543" ;
				];
				hydra:mapping[ a hydra:IriTemplateMapping;
					hydra:variable "maxlatitude"^^xsd:string;
					hydra:property "epos:northernmostLatitude";
					rdfs:range "xsd:float";
					rdfs:label "Maximum Latitude";
					schema:minValue "-90.0";
					schema:maxValue "90.0";
					hydra:required "true"^^xsd:boolean;
					schema:defaultValue "49.0013656616211" ;
				];
				hydra:mapping[ a hydra:IriTemplateMapping;
					hydra:variable "minlongitude"^^xsd:string;
					hydra:property "epos:westernmostLongitude";
					rdfs:range "xsd:float";
					rdfs:label "Minimum Longitude";
					schema:minValue "-180.0";
					schema:maxValue "180.0";
					hydra:required "true"^^xsd:boolean;
					schema:defaultValue "-12.3925075531006" ;
				];
				hydra:mapping[ a hydra:IriTemplateMapping;
					hydra:variable "maxlongitude"^^xsd:string;
					hydra:property "epos:easternmostLongitude";
					rdfs:range "xsd:float";
					rdfs:label "Maximum Longitude";
					schema:minValue "-180.0";
					schema:maxValue "180.0";
					hydra:required "true"^^xsd:boolean;
					schema:defaultValue "45.2800407409668" ;
				];
				hydra:mapping[ a hydra:IriTemplateMapping;
					hydra:variable "width"^^xsd:string;
					rdfs:range "xsd:integer";
					rdfs:label "Image width";
					schema:defaultValue "768";
					http:paramValue "768";
					hydra:required "true"^^xsd:boolean;
				];
				hydra:mapping[ a hydra:IriTemplateMapping;
					hydra:variable "height"^^xsd:string;
					rdfs:range "xsd:integer";
					rdfs:label "Image height";
					schema:defaultValue "330";
					http:paramValue "330";
					hydra:required "true"^^xsd:boolean;
				];
				hydra:mapping[ a hydra:IriTemplateMapping;
					hydra:variable "crs"^^xsd:string;
					rdfs:range "xsd:string";
					rdfs:label "Coordinate (Spatial) Reference System";
					schema:defaultValue "EPSG:4326";
					http:paramValue "EPSG:4326";
					http:paramValue "EPSG:5837";
					http:paramValue "EPSG:32628";
					http:paramValue "EPSG:32629";
					http:paramValue "EPSG:32630";
					http:paramValue "EPSG:32631";
					http:paramValue "EPSG:32632";
					http:paramValue "EPSG:32633";
					http:paramValue "EPSG:32634";
					http:paramValue "EPSG:32635";
					http:paramValue "EPSG:32636";
					http:paramValue "EPSG:32637";
					http:paramValue "EPSG:32638";
					http:paramValue "EPSG:32639";
					http:paramValue "EPSG:32640";
					hydra:required "true"^^xsd:boolean;
				];
				hydra:mapping[ a hydra:IriTemplateMapping;
					hydra:variable "format"^^xsd:string;
					rdfs:range "xsd:string";
					rdfs:label "Output format";
					schema:defaultValue "image/png";
					http:paramValue "image/png";
					http:paramValue "image/jpg";
					http:paramValue "image/tiff";
					http:paramValue "image/gif";
					http:paramValue "application/vnd.google-earth.kmz";
					http:paramValue "application/vnd.google-earth.kml+xml";
					http:paramValue "application/pdf";
					hydra:required "true"^^xsd:boolean;
				];
		] ;
.

	<Seismology/EDSF/WFS-CrustalFaults> a hydra:Operation;
		hydra:method "GET"^^xsd:string;
		hydra:returns "application/gml+xml";
		hydra:property[ a hydra:IriTemplate;
			hydra:template "http://services.seismofaults.eu/geoserver/EDSF/ows{?service, version, request, typeNames, outputFormat, count, srsName}&bbox={minlatitude, minlongitude, maxlatitude, maxlongitude}"^^xsd:string;
			#CQL_FILTER GeoServer vendor parameter management is postponed to forthcoming version since some issues have to be solved in its management together with bbox
			#hydra:template "http://services.seismofaults.eu/geoserver/EDSF/ows{?service, version, request, typeNames, outputFormat, count, srsName}&bbox={minlatitude, minlongitude, maxlatitude, maxlongitude}&CQL_FILTER={mindepth, maxdepth, strikemin, strikemax, dipmin, dipmax, rakemin, rakemax, srmin, srmax, maxmag}"^^xsd:string;
				hydra:mapping[ a hydra:IriTemplateMapping;
					hydra:variable "service"^^xsd:string;
					rdfs:range "xsd:string";
					rdfs:label "Service";
					schema:defaultValue "WFS";
					http:paramValue "WFS";
					hydra:required "true"^^xsd:boolean;
				];
				hydra:mapping[ a hydra:IriTemplateMapping;
					hydra:variable "version"^^xsd:string;
					rdfs:range "xsd:string";
					rdfs:label "Service version";
					schema:defaultValue "2.0.0";
					# commented out for axis ordering difference between it and later versions
					#http:paramValue "1.0.0";
					http:paramValue "1.1.0";
					http:paramValue "2.0.0";
					hydra:required "true"^^xsd:boolean;
				];
				hydra:mapping[ a hydra:IriTemplateMapping;
					hydra:variable "request"^^xsd:string;
					rdfs:range "xsd:string";
					rdfs:label "Request type";
					schema:defaultValue "GetFeature";
					http:paramValue "GetFeature";
					hydra:required "true"^^xsd:boolean;
				];
				hydra:mapping[ a hydra:IriTemplateMapping;
					hydra:variable "typeNames"^^xsd:string;
					rdfs:range "xsd:string";
					rdfs:label "Feature layer to load";
					schema:defaultValue "EDSF:crustal_fault_sources_top";
					http:paramValue "EDSF:crustal_fault_sources_top";
					http:paramValue "EDSF:crustal_fault_sources_pln";
					hydra:required "true"^^xsd:boolean;
				];
				hydra:mapping[ a hydra:IriTemplateMapping;
					hydra:variable "count"^^xsd:string;
					rdfs:range "xsd:string";
					rdfs:label "Maximum number of features to retrieve";
					hydra:required "false"^^xsd:boolean;
				];
				hydra:mapping[ a hydra:IriTemplateMapping;
					hydra:variable "minlatitude"^^xsd:string;
					hydra:property "epos:southernmostLatitude";
					rdfs:range "xsd:float";
					rdfs:label "Minimum Latitude";
					schema:minValue "-90.0";
					schema:maxValue "90.0";
					hydra:required "false"^^xsd:boolean;
					schema:defaultValue "30.303092956543" ;
				];
				hydra:mapping[ a hydra:IriTemplateMapping;
					hydra:variable "maxlatitude"^^xsd:string;
					hydra:property "epos:northernmostLatitude";
					rdfs:range "xsd:float";
					rdfs:label "Maximum Latitude";
					schema:minValue "-90.0";
					schema:maxValue "90.0";
					hydra:required "false"^^xsd:boolean;
					schema:defaultValue "49.0013656616211" ;
				];
				hydra:mapping[ a hydra:IriTemplateMapping;
					hydra:variable "minlongitude"^^xsd:string;
					hydra:property "epos:westernmostLongitude";
					rdfs:range "xsd:float";
					rdfs:label "Minimum Longitude";
					schema:minValue "-180.0";
					schema:maxValue "180.0";
					hydra:required "false"^^xsd:boolean;
					schema:defaultValue "-12.3925075531006" ;
				];
				hydra:mapping[ a hydra:IriTemplateMapping;
					hydra:variable "maxlongitude"^^xsd:string;
					hydra:property "epos:easternmostLongitude";
					rdfs:range "xsd:float";
					rdfs:label "Maximum Longitude";
					schema:minValue "-180.0";
					schema:maxValue "180.0";
					hydra:required "false"^^xsd:boolean;
					schema:defaultValue "45.2800407409668" ;
				];
				hydra:mapping[ a hydra:IriTemplateMapping;
					hydra:variable "srsName";
					rdfs:range "xsd:string";
					rdfs:label "SRS to use";
					schema:defaultValue "EPSG:4326";
					http:paramValue "EPSG:4326";
					http:paramValue "EPSG:5837";
					http:paramValue "EPSG:32628";
					http:paramValue "EPSG:32629";
					http:paramValue "EPSG:32630";
					http:paramValue "EPSG:32631";
					http:paramValue "EPSG:32632";
					http:paramValue "EPSG:32633";
					http:paramValue "EPSG:32634";
					http:paramValue "EPSG:32635";
					http:paramValue "EPSG:32636";
					http:paramValue "EPSG:32637";
					http:paramValue "EPSG:32638";
					http:paramValue "EPSG:32639";
					http:paramValue "EPSG:32640";
					hydra:required "true"^^xsd:boolean;
				];
				#hydra:mapping[ a hydra:IriTemplateMapping;
				#	hydra:variable "bbox"^^xsd:string;
				#	rdfs:range "xsd:string";
				#	rdfs:label "Bounding Box";
				#	hydra:required "false"^^xsd:boolean;
				#];
				hydra:mapping[ a hydra:IriTemplateMapping;
					hydra:variable "outputFormat"^^xsd:string;
					rdfs:range "xsd:string";
					rdfs:label "Output format";
					schema:defaultValue "text/xml; subtype=gml/2.1.2 ";
					http:paramValue "text/xml; subtype=gml/2.1.2 ";
					http:paramValue "gml3";
					http:paramValue "application/json";
					http:paramValue "application/kml";
					http:paramValue "csv";
					http:paramValue "SHAPE-ZIP";
					hydra:required "true"^^xsd:boolean;
				];
				hydra:mapping[ a hydra:IriTemplateMapping;
					hydra:variable "CQL_FILTER=mindepth";
					rdfs:range "xsd:float";
					rdfs:label "Minimum fault depth";
					hydra:required "false"^^xsd:boolean;
				];
				hydra:mapping[ a hydra:IriTemplateMapping;
					hydra:variable "CQL_FILTER=maxdepth";
					rdfs:range "xsd:float";
					rdfs:label "Maximum fault depth";
					hydra:required "false"^^xsd:boolean;
				];
				hydra:mapping[ a hydra:IriTemplateMapping;
					hydra:variable "CQL_FILTER=strikemin";
					rdfs:range "xsd:integer";
					rdfs:label "Minimum strike base 60";
					hydra:required "false"^^xsd:boolean;
				];
				hydra:mapping[ a hydra:IriTemplateMapping;
					hydra:variable "CQL_FILTER=strikemax";
					rdfs:range "xsd:integer";
					rdfs:label "Maximum strike base 60";
					hydra:required "false"^^xsd:boolean;
				];
				hydra:mapping[ a hydra:IriTemplateMapping;
					hydra:variable "CQL_FILTER=dipmin";
					rdfs:range "xsd:integer";
					rdfs:label "Minimum dip base 60";
					hydra:required "false"^^xsd:boolean;
				];
				hydra:mapping[ a hydra:IriTemplateMapping;
					hydra:variable "CQL_FILTER=dipmax";
					rdfs:range "xsd:integer";
					rdfs:label "Maximum dip base 60";
					hydra:required "false"^^xsd:boolean;
				];
				hydra:mapping[ a hydra:IriTemplateMapping;
					hydra:variable "CQL_FILTER=rakemin";
					rdfs:range "xsd:integer";
					rdfs:label "Minimum rake base 60";
					hydra:required "false"^^xsd:boolean;
				];
				hydra:mapping[ a hydra:IriTemplateMapping;
					hydra:variable "CQL_FILTER=rakemax";
					rdfs:range "xsd:integer";
					rdfs:label "Maximum rake base 60";
					hydra:required "false"^^xsd:boolean;
				];
				hydra:mapping[ a hydra:IriTemplateMapping;
					hydra:variable "CQL_FILTER=srmin";
					rdfs:range "xsd:float";
					rdfs:label "Minimum slip rate (mm/yr)";
					hydra:required "false"^^xsd:boolean;
				];
				hydra:mapping[ a hydra:IriTemplateMapping;
					hydra:variable "CQL_FILTER=srmax";
					rdfs:range "xsd:float";
					rdfs:label "Maximum slip rate (mm/yr)";
					hydra:required "false"^^xsd:boolean;
				];
				hydra:mapping[ a hydra:IriTemplateMapping;
					hydra:variable "CQL_FILTER=maxmag";
					rdfs:range "xsd:float";
					rdfs:label "Maximum magnitude";
					hydra:required "false"^^xsd:boolean;
				];
		] ;
.
	<Seismology/EDSF/WFS-Subductions> a hydra:Operation;
		hydra:method "GET"^^xsd:string;
		hydra:returns "application/gml+xml";
		hydra:property[ a hydra:IriTemplate;
			hydra:template "http://services.seismofaults.eu/geoserver/EDSF/ows{?service, version, request, typeNames, outputFormat, count, srsName}&bbox={minlatitude, minlongitude, maxlatitude, maxlongitude}"^^xsd:string;
			#hydra:template "http://services.seismofaults.eu/geoserver/EDSF/ows{?service, version, request, typeNames, outputFormat, count, srsName}&bbox={minlatitude, maxlatitude, minlongitude, maxlongitude}&CQL_FILTER={}"^^xsd:string;
				hydra:mapping[ a hydra:IriTemplateMapping;
					hydra:variable "service"^^xsd:string;
					rdfs:range "xsd:string";
					rdfs:label "Service";
					schema:defaultValue "WFS";
					http:paramValue "WFS";
					hydra:required "true"^^xsd:boolean;
				];
				hydra:mapping[ a hydra:IriTemplateMapping;
					hydra:variable "version"^^xsd:string;
					rdfs:range "xsd:string";
					rdfs:label "Service version";
					schema:defaultValue "2.0.0";
					# commented out for axis ordering difference between it and later versions	
					#http:paramValue "1.0.0";
					http:paramValue "1.1.0";
					http:paramValue "2.0.0";
					hydra:required "true"^^xsd:boolean;
				];
				hydra:mapping[ a hydra:IriTemplateMapping;
					hydra:variable "request"^^xsd:string;
					rdfs:range "xsd:string";
					rdfs:label "Request type";
					schema:defaultValue "GetFeature";
					http:paramValue "GetFeature";
					hydra:required "true"^^xsd:boolean;
				];
				hydra:mapping[ a hydra:IriTemplateMapping;
					hydra:variable "typeNames"^^xsd:string;
					rdfs:range "xsd:string";
					rdfs:label "Feature layer to load";
					schema:defaultValue "EDSF:subduction_contours";
					http:paramValue "EDSF:subduction_zones";
					http:paramValue "EDSF:subduction_contours";
					hydra:required "true"^^xsd:boolean;
				];
				hydra:mapping[ a hydra:IriTemplateMapping;
					hydra:variable "count"^^xsd:string;
					rdfs:range "xsd:string";
					rdfs:label "Maximum number of features to retrieve";
					hydra:required "false"^^xsd:boolean;
				];
				#hydra:mapping[ a hydra:IriTemplateMapping;
				#	hydra:variable "bbox"^^xsd:string;
				#	rdfs:range "xsd:string";
				#	rdfs:label "Bounding Box";
				#	hydra:required "false"^^xsd:boolean;
				#];
				hydra:mapping[ a hydra:IriTemplateMapping;
					hydra:variable "minlatitude"^^xsd:string;
					hydra:property "epos:southernmostLatitude";
					rdfs:range "xsd:float";
					rdfs:label "Minimum Latitude";
					schema:minValue "-90.0";
					schema:maxValue "90.0";
					hydra:required "false"^^xsd:boolean;
					schema:defaultValue "32.278719" ;
				];
				hydra:mapping[ a hydra:IriTemplateMapping;
					hydra:variable "maxlatitude"^^xsd:string;
					hydra:property "epos:northernmostLatitude";
					rdfs:range "xsd:float";
					rdfs:label "Maximum Latitude";
					schema:minValue "-90.0";
					schema:maxValue "90.0";
					hydra:required "false"^^xsd:boolean;
					schema:defaultValue "42.456003" ;
				];
				hydra:mapping[ a hydra:IriTemplateMapping;
					hydra:variable "minlongitude"^^xsd:string;
					hydra:property "epos:westernmostLongitude";
					rdfs:range "xsd:float";
					rdfs:label "Minimum Longitude";
					schema:minValue "-180.0";
					schema:maxValue "180.0";
					hydra:required "false"^^xsd:boolean;
					schema:defaultValue "13.204229" ;
				];
				hydra:mapping[ a hydra:IriTemplateMapping;
					hydra:variable "maxlongitude"^^xsd:string;
					hydra:property "epos:easternmostLongitude";
					rdfs:range "xsd:float";
					rdfs:label "Maximum Longitude";
					schema:minValue "-180.0";
					schema:maxValue "180.0";
					hydra:required "false"^^xsd:boolean;
					schema:defaultValue "35.2695846557617" ;
				];
				hydra:mapping[ a hydra:IriTemplateMapping;
					hydra:variable "outputFormat"^^xsd:string;
					rdfs:range "xsd:string";
					rdfs:label "Output format";
					schema:defaultValue "text/xml; subtype=gml/2.1.2 ";
					http:paramValue "text/xml; subtype=gml/2.1.2 ";
					http:paramValue "gml3";
					http:paramValue "application/json";
					http:paramValue "application/kml";
					http:paramValue "csv";
					http:paramValue "SHAPE-ZIP";
					hydra:required "true"^^xsd:boolean;
				];
				#DB parameter for subductions are not yet implemented since attributes between subduction_countour and subduction_zones layers are different each other
		] ;
.

	<http://orcid.org/0000-0003-1208-9412/contactPoint> a schema:ContactPoint;
		schema:email "roberto.vallone@ingv.it";
		schema:availableLanguage "en" ;
.
	<http://orcid.org/0000-0002-1213-0828/scientificContact> a schema:ContactPoint;
		schema:email "roberto.basili@ingv.it";
		schema:availableLanguage "en" ;
		schema:contactType "scientificContact" ;
.
	<http://orcid.org/0000-0002-8651-6387/legalContact> a schema:ContactPoint;
		schema:email "segreteria.presidenza@ingv.it";
		schema:availableLanguage "en" ;
		schema:contactType "legalContact" ;
.
	<http://orcid.org/0000-0003-1208-9412/contactPoint> a schema:ContactPoint;
		schema:email "roberto.vallone@ingv.it";
		schema:availableLanguage "en" ;
		#schema:contactType "contactPoint" ;
.

<#Seismology> a skos:ConceptScheme;
	dct:title "Seismology";
	dct:description "It contains the concepts of Seismology";
.
<#Activefaults> a skos:Concept;
	skos:definition "Faults that are deemed to be capable to generate earthquakes of magnitude greater or equal to 5.5";
	skos:inScheme <#Seismology>;
	skos:prefLabel "Active faults";
.
